@prefix : <https://w3id.org/sdp/core#> .
@prefix cc: <https://creativecommons.org/ns/> .
@prefix dc: <http://purl.org/dc/elements/1.1/> .
@prefix gn: <http://www.geonames.org/ontology#> .
@prefix dct: <http://purl.org/dc/terms/> .
@prefix owl: <http://www.w3.org/2002/07/owl#> .
@prefix rdf: <http://www.w3.org/1999/02/22-rdf-syntax-ns#> .
@prefix xml: <http://www.w3.org/XML/1998/namespace> .
@prefix xsd: <http://www.w3.org/2001/XMLSchema#> .
@prefix cspa: <http://rdf.unece.org/models/cspa#> .
@prefix dcat: <http://www.w3.org/TR/vocab-dcat/> .
@prefix foaf: <http://xmlns.com/foaf/0.1/> .
@prefix gsim: <http://rdf.unece.org/models/gsim#> .
@prefix obda: <https://w3id.org/obda/vocabulary#> .
@prefix prov: <http://www.w3.org/ns/prov#> .
@prefix rdfs: <http://www.w3.org/2000/01/rdf-schema#> .
@prefix skos: <http://www.w3.org/2004/02/skos/core#> .
@prefix xkos: <http://rdf-vocabulary.ddialliance.org/xkos#> .
@prefix gamso: <http://rdf.unece.org/models/gamso#> .
@prefix gsbpm: <http://rdf.unece.org/models/gsbpm#> .
@prefix id-ps: <https://www.bps.go.id/survey/population-census#> .
@prefix igsbpm: <http://id.unece.org/models/gsbpm/> .
@prefix kshrts: <https://www.ksh.hu/survey/retail-trade-statistics#> .
@prefix gsim-sum: <https://w3id.org/italia/onto/gsim-sum#> .
@base <https://w3id.org/sdp/core#> .

<https://w3id.org/sdp/core#> rdf:type owl:Ontology ;
                              owl:versionIRI <https://w3id.org/sdp/1.0> ;
                              dc:creator """Sulthoni Ashiddiiqi - Institut Teknologi Bandung, Bandung, Indonesia
Fajar J. Ekaputra - DPKM - WU Vienna, Austria
Muhammad Zuhri Catur Candra - Institut Teknologi Bandung, Bandung, Indonesia""" ;
                              dc:description "An Ontology that describes processes and metadata for the statistical data production."@en ;
                              dc:title "Statistical Data Production (SDP) Ontology"@en ;
                              dct:issued "2024-09-02"^^xsd:date ;
                              dct:license <https://creativecommons.org/licenses/by/4.0/> ;
                              owl:versionInfo "Version 1.0"@en .

#################################################################
#    Annotation properties
#################################################################

###  http://purl.org/dc/elements/1.1/creator
dc:creator rdf:type owl:AnnotationProperty .


###  http://purl.org/dc/elements/1.1/description
dc:description rdf:type owl:AnnotationProperty .


###  http://purl.org/dc/elements/1.1/title
dc:title rdf:type owl:AnnotationProperty .


###  http://purl.org/dc/terms/issued
dct:issued rdf:type owl:AnnotationProperty .


###  http://purl.org/dc/terms/license
dct:license rdf:type owl:AnnotationProperty .


###  http://rdf.unece.org/models/cspa#label
cspa:label rdf:type owl:AnnotationProperty ;
           rdfs:subPropertyOf rdfs:label ;
           rdfs:range xsd:string .


###  http://www.w3.org/2004/02/skos/core#broader
skos:broader rdf:type owl:AnnotationProperty .


###  http://www.w3.org/2004/02/skos/core#definition
skos:definition rdf:type owl:AnnotationProperty .


###  http://www.w3.org/2004/02/skos/core#hasTopConcept
skos:hasTopConcept rdf:type owl:AnnotationProperty .


###  http://www.w3.org/2004/02/skos/core#inScheme
skos:inScheme rdf:type owl:AnnotationProperty .


###  http://www.w3.org/2004/02/skos/core#narrower
skos:narrower rdf:type owl:AnnotationProperty .


###  http://www.w3.org/2004/02/skos/core#notation
skos:notation rdf:type owl:AnnotationProperty .


###  http://www.w3.org/2004/02/skos/core#prefLabel
skos:prefLabel rdf:type owl:AnnotationProperty .


###  http://www.w3.org/2004/02/skos/core#topConceptOf
skos:topConceptOf rdf:type owl:AnnotationProperty .


###  http://xmlns.com/foaf/0.1/homepage
foaf:homepage rdf:type owl:AnnotationProperty .


#################################################################
#    Datatypes
#################################################################

###  http://www.w3.org/2001/XMLSchema#date
xsd:date rdf:type rdfs:Datatype .


#################################################################
#    Object Properties
#################################################################

###  http://rdf.unece.org/models/cspa#aimsAt
cspa:aimsAt rdf:type owl:ObjectProperty ;
            rdfs:domain cspa:ServiceDefinition ;
            rdfs:range cspa:BusinessFunction ;
            rdfs:label "Link between a description level and Business function" .


###  http://rdf.unece.org/models/cspa#assemblerOrganization
cspa:assemblerOrganization rdf:type owl:ObjectProperty ;
                           rdfs:subPropertyOf cspa:genericOrganization ;
                           rdfs:label "Assembler organization" .


###  http://rdf.unece.org/models/cspa#builderOrganization
cspa:builderOrganization rdf:type owl:ObjectProperty ;
                         rdfs:subPropertyOf cspa:genericOrganization ;
                         rdfs:label "Builder organization" .


###  http://rdf.unece.org/models/cspa#comesFrom
cspa:comesFrom rdf:type owl:ObjectProperty ;
               rdfs:domain cspa:DescriptionLevel ;
               rdfs:range cspa:Provenance ;
               rdfs:label "Link between a description level and a Provenance" .


###  http://rdf.unece.org/models/cspa#configurerOrganization
cspa:configurerOrganization rdf:type owl:ObjectProperty ;
                            rdfs:subPropertyOf cspa:genericOrganization ;
                            rdfs:label "Configurer organization" .


###  http://rdf.unece.org/models/cspa#definitionDependsOn
cspa:definitionDependsOn rdf:type owl:ObjectProperty ;
                         rdfs:domain cspa:ServiceDefinition ;
                         rdfs:range cspa:DefinitionDependency ;
                         rdfs:label "Link between a service definition description level and a Dependency" .


###  http://rdf.unece.org/models/cspa#definitionHasInput
cspa:definitionHasInput rdf:type owl:ObjectProperty ;
                        rdfs:domain cspa:FunctionDefinition ;
                        rdfs:range cspa:DefinitionInput ;
                        rdfs:label "Link between a service definition description level and an Input" .


###  http://rdf.unece.org/models/cspa#definitionHasOuput
cspa:definitionHasOuput rdf:type owl:ObjectProperty ;
                        rdfs:domain cspa:FunctionDefinition ;
                        rdfs:range cspa:DefinitionOutput ;
                        rdfs:label "Link between a service definition description level and an Output" .


###  http://rdf.unece.org/models/cspa#definitionIsInvokedBy
cspa:definitionIsInvokedBy rdf:type owl:ObjectProperty ;
                           rdfs:domain cspa:ServiceDefinition ;
                           rdfs:range cspa:DefinitionInterface ;
                           rdfs:label "Link between a service definition description level and an Interface" .


###  http://rdf.unece.org/models/cspa#designerOrganization
cspa:designerOrganization rdf:type owl:ObjectProperty ;
                          rdfs:subPropertyOf cspa:genericOrganization ;
                          rdfs:label "Designer organization" .


###  http://rdf.unece.org/models/cspa#environmentProviderOrganization
cspa:environmentProviderOrganization rdf:type owl:ObjectProperty ;
                                     rdfs:subPropertyOf cspa:genericOrganization ;
                                     rdfs:label "Environment provider organization" .


###  http://rdf.unece.org/models/cspa#genericOrganization
cspa:genericOrganization rdf:type owl:ObjectProperty ;
                         rdfs:subPropertyOf owl:topObjectProperty ;
                         rdfs:domain cspa:Provenance ;
                         rdfs:range cspa:Organization ;
                         rdfs:label "Generic Organization" .


###  http://rdf.unece.org/models/cspa#gsbpmSubProcess
cspa:gsbpmSubProcess rdf:type owl:ObjectProperty ;
                     rdfs:domain cspa:BusinessFunction ;
                     rdfs:range gsbpm:SubProcess ;
                     rdfs:comment "See GSBPM documentation" ;
                     rdfs:label "GSBPM sub-process" .


###  http://rdf.unece.org/models/cspa#gsimInput
cspa:gsimInput rdf:type owl:ObjectProperty ;
               rdfs:domain cspa:DefinitionInput ;
               rdfs:range gsim-sum:IdentifiableArtefact ;
               rdfs:label "GSIM Input" .


###  http://rdf.unece.org/models/cspa#gsimOutput
cspa:gsimOutput rdf:type owl:ObjectProperty ;
                rdfs:domain cspa:DefinitionOutput ;
                rdfs:range gsim-sum:IdentifiableArtefact ;
                rdfs:label "GSIM Output" .


###  http://rdf.unece.org/models/cspa#hasDependencyIdentifier
cspa:hasDependencyIdentifier rdf:type owl:ObjectProperty ;
                             rdfs:domain cspa:Dependency ;
                             rdfs:range cspa:DependencyIdentifier ;
                             rdfs:label "Link between a dependency and its identifier" .


###  http://rdf.unece.org/models/cspa#hasFunctionDefinition
cspa:hasFunctionDefinition rdf:type owl:ObjectProperty ;
                           rdfs:domain cspa:Function ;
                           rdfs:range cspa:FunctionDefinition ;
                           rdfs:comment "Link between a CSPA function and its definition" ;
                           rdfs:label "Definition of a CSPA function" .


###  http://rdf.unece.org/models/cspa#hasFunctionImplementation
cspa:hasFunctionImplementation rdf:type owl:ObjectProperty ;
                               rdfs:domain cspa:Function ;
                               rdfs:range cspa:FunctionImplementation ;
                               rdfs:comment "Link between a CSPA function and its implementation description" ;
                               rdfs:label "Implementation description of a CSPA function" .


###  http://rdf.unece.org/models/cspa#hasFunctionSpecification
cspa:hasFunctionSpecification rdf:type owl:ObjectProperty ;
                              rdfs:domain cspa:Function ;
                              rdfs:range cspa:FunctionSpecification ;
                              rdfs:comment "Link between a CSPA function and its specification" ;
                              rdfs:label "Specification of a CSPA function" .


###  http://rdf.unece.org/models/cspa#hasInputIdentifier
cspa:hasInputIdentifier rdf:type owl:ObjectProperty ;
                        rdfs:domain cspa:Input ;
                        rdfs:range cspa:InputIdentifier ;
                        rdfs:label "Link between an input and its identifier" .


###  http://rdf.unece.org/models/cspa#hasInterfaceIdentifier
cspa:hasInterfaceIdentifier rdf:type owl:ObjectProperty ;
                            rdfs:domain cspa:Interface ;
                            rdfs:range cspa:InterfaceIdentifier ;
                            rdfs:label "Link between an interface and its identifier" .


###  http://rdf.unece.org/models/cspa#hasOutputIdentifier
cspa:hasOutputIdentifier rdf:type owl:ObjectProperty ;
                         rdfs:domain cspa:Output ;
                         rdfs:range cspa:OutputIdentifier ;
                         rdfs:label "Link between an output and its identifier" .


###  http://rdf.unece.org/models/cspa#hasPackage
cspa:hasPackage rdf:type owl:ObjectProperty ;
                rdfs:domain cspa:PackageOrFunction ;
                rdfs:range cspa:Package ;
                rdfs:comment "A CSPA package or a CSPA function may be a member of a CSPA package." ;
                rdfs:label "CSPA package or CSPA function is a member of a CSPA package" .


###  http://rdf.unece.org/models/cspa#hasPackageDefinition
cspa:hasPackageDefinition rdf:type owl:ObjectProperty ;
                          rdfs:domain cspa:Package ;
                          rdfs:range cspa:PackageDefinition ;
                          rdfs:comment "Link between a CSPA package and its definition." ;
                          rdfs:label "Definition of a CSPA package" .


###  http://rdf.unece.org/models/cspa#hasPackageImplementation
cspa:hasPackageImplementation rdf:type owl:ObjectProperty ;
                              rdfs:domain cspa:Package ;
                              rdfs:range cspa:PackageImplementation ;
                              rdfs:comment "Link between a CSPA package and its implementation" ;
                              rdfs:label "Implementation of a CSPA package" .


###  http://rdf.unece.org/models/cspa#hasPackageSpecification
cspa:hasPackageSpecification rdf:type owl:ObjectProperty ;
                             rdfs:domain cspa:Package ;
                             rdfs:range cspa:PackageSpecification ;
                             rdfs:comment "Link between a CSPA package and its specification" ;
                             rdfs:label "Specification of a CSPA package" .


###  http://rdf.unece.org/models/cspa#homepage
cspa:homepage rdf:type owl:ObjectProperty ;
              rdfs:subPropertyOf owl:topObjectProperty ;
              rdfs:domain cspa:Documentation ;
              rdfs:range cspa:Document ;
              rdfs:comment "Homepage of the service; a web page containing information about the service." ;
              rdfs:label "Homepage" .


###  http://rdf.unece.org/models/cspa#implementationDependsOn
cspa:implementationDependsOn rdf:type owl:ObjectProperty ;
                             rdfs:domain cspa:ImplementationInterface ,
                                         cspa:ServiceImplementation ;
                             rdfs:range cspa:ImplementationDependency ;
                             rdfs:label "Link between a implementation description level and a Dependency" .


###  http://rdf.unece.org/models/cspa#implementationHasInput
cspa:implementationHasInput rdf:type owl:ObjectProperty ;
                            rdfs:domain cspa:FunctionImplementation ;
                            rdfs:range cspa:ImplementationInput ;
                            rdfs:label "Link between a implementation description level and an Input" .


###  http://rdf.unece.org/models/cspa#implementationHasOutput
cspa:implementationHasOutput rdf:type owl:ObjectProperty ;
                             rdfs:domain cspa:FunctionImplementation ;
                             rdfs:range cspa:ImplementationOutput ;
                             rdfs:label "Link between a implementation description level and an Output" .


###  http://rdf.unece.org/models/cspa#implementationIsInvokedBy
cspa:implementationIsInvokedBy rdf:type owl:ObjectProperty ;
                               rdfs:domain cspa:ServiceImplementation ;
                               rdfs:range cspa:ImplementationInterface ;
                               rdfs:label "Link between a implementation description level and an Interface" .


###  http://rdf.unece.org/models/cspa#installationGuide
cspa:installationGuide rdf:type owl:ObjectProperty ;
                       rdfs:domain cspa:Documentation ;
                       rdfs:range cspa:Document ;
                       rdfs:comment "Document explaining how to install the service." ;
                       rdfs:label "Installation guide" .


###  http://rdf.unece.org/models/cspa#investorOrganization
cspa:investorOrganization rdf:type owl:ObjectProperty ;
                          rdfs:subPropertyOf cspa:genericOrganization ;
                          rdfs:label "Investor organization" .


###  http://rdf.unece.org/models/cspa#isDocumentedBy
cspa:isDocumentedBy rdf:type owl:ObjectProperty ;
                    rdfs:domain cspa:DescriptionLevel ;
                    rdfs:range cspa:Documentation ;
                    rdfs:label "Link between a description level and a Documentation" .


###  http://rdf.unece.org/models/cspa#limObject
cspa:limObject rdf:type owl:ObjectProperty ;
               rdfs:domain cspa:SpecificationInput ,
                           cspa:SpecificationOutput ;
               rdfs:range cspa:LIMClass ;
               rdfs:label "CSPA LIM object" .


###  http://rdf.unece.org/models/cspa#serviceProviderOrganization
cspa:serviceProviderOrganization rdf:type owl:ObjectProperty ;
                                 rdfs:subPropertyOf cspa:genericOrganization ;
                                 rdfs:label "Service provider organization" .


###  http://rdf.unece.org/models/cspa#specificationDependsOn
cspa:specificationDependsOn rdf:type owl:ObjectProperty ;
                            rdfs:domain cspa:ServiceSpecification ;
                            rdfs:range cspa:SpecificationDependency ;
                            rdfs:label "Link between a specification description level and a Dependency" .


###  http://rdf.unece.org/models/cspa#specificationHasInput
cspa:specificationHasInput rdf:type owl:ObjectProperty ;
                           rdfs:domain cspa:FunctionSpecification ;
                           rdfs:range cspa:SpecificationInput ;
                           rdfs:label "Link between a specification description level and an Input" .


###  http://rdf.unece.org/models/cspa#specificationHasOuput
cspa:specificationHasOuput rdf:type owl:ObjectProperty ;
                           rdfs:domain cspa:FunctionSpecification ;
                           rdfs:range cspa:SpecificationOutput ;
                           rdfs:label "Link between a specification description level and Output" .


###  http://rdf.unece.org/models/cspa#specificationIsInvokedBy
cspa:specificationIsInvokedBy rdf:type owl:ObjectProperty ;
                              rdfs:domain cspa:ServiceSpecification ;
                              rdfs:range cspa:SpecificationInterface ;
                              rdfs:label "Link between a specification description level and an Interface" .


###  http://rdf.unece.org/models/cspa#userOrganization
cspa:userOrganization rdf:type owl:ObjectProperty ;
                      rdfs:subPropertyOf cspa:genericOrganization ;
                      rdfs:label "User organization" .


###  https://w3id.org/italia/onto/gsim-sum#measuresV-C
gsim-sum:measuresV-C rdf:type owl:ObjectProperty ;
                     rdfs:domain gsim-sum:Variable ;
                     rdfs:range gsim-sum:Concept .


###  https://w3id.org/italia/onto/gsim-sum#measuresV-UT
gsim-sum:measuresV-UT rdf:type owl:ObjectProperty ;
                      rdfs:domain gsim-sum:Variable ;
                      rdfs:range gsim-sum:UnitType .


###  https://w3id.org/sdp/core#classifiedAs
:classifiedAs rdf:type owl:ObjectProperty ;
              rdfs:domain :ProcessDesign ;
              rdfs:range gsbpm:SubProcess .


###  https://w3id.org/sdp/core#classifiedAs-GAMSO
:classifiedAs-GAMSO rdf:type owl:ObjectProperty ;
                    rdfs:domain :ProcessSupportInput ;
                    rdfs:range gamso:StatisticalSupportingActivity .


###  https://w3id.org/sdp/core#correspondsToPI-PIS
:correspondsToPI-PIS rdf:type owl:ObjectProperty ;
                     rdfs:domain :ProcessInput ;
                     rdfs:range :ProcessInputSpecification .


###  https://w3id.org/sdp/core#correspondsToPO-POS
:correspondsToPO-POS rdf:type owl:ObjectProperty ;
                     rdfs:domain :ProcessOutput ;
                     rdfs:range :ProcessOutputSpecification .


###  https://w3id.org/sdp/core#createsPS-PO
:createsPS-PO rdf:type owl:ObjectProperty ;
              rdfs:domain :ProcessStep ;
              rdfs:range :ProcessOutput .


###  https://w3id.org/sdp/core#hasBP-PS
:hasBP-PS rdf:type owl:ObjectProperty ;
          rdfs:domain :BusinessProcess ;
          rdfs:range :ProcessStep .


###  https://w3id.org/sdp/core#hasPCD-R
:hasPCD-R rdf:type owl:ObjectProperty ;
          rdfs:domain :ProcessControlDesign ;
          rdfs:range :Rule .


###  https://w3id.org/sdp/core#hasPD-PCD
:hasPD-PCD rdf:type owl:ObjectProperty ;
           rdfs:domain :ProcessDesign ;
           rdfs:range :ProcessControlDesign .


###  https://w3id.org/sdp/core#hasPD-PIS
:hasPD-PIS rdf:type owl:ObjectProperty ;
           rdfs:domain :ProcessDesign ;
           rdfs:range :ProcessInputSpecification .


###  https://w3id.org/sdp/core#hasPD-POS
:hasPD-POS rdf:type owl:ObjectProperty ;
           rdfs:domain :ProcessDesign ;
           rdfs:range :ProcessOutputSpecification .


###  https://w3id.org/sdp/core#hasPM-R
:hasPM-R rdf:type owl:ObjectProperty ;
         rdfs:domain :ProcessMethod ;
         rdfs:range :Rule .


###  https://w3id.org/sdp/core#hasPS-PI
:hasPS-PI rdf:type owl:ObjectProperty ;
          rdfs:domain :ProcessStep ;
          rdfs:range :ProcessInput .


###  https://w3id.org/sdp/core#hasSP-SPC
:hasSP-SPC rdf:type owl:ObjectProperty ;
           rdfs:domain :StatisticalProgram ;
           rdfs:range :StatisticalProgramCycle .


###  https://w3id.org/sdp/core#implementsPD-PM
:implementsPD-PM rdf:type owl:ObjectProperty ;
                 rdfs:domain :ProcessDesign ;
                 rdfs:range :ProcessMethod .


###  https://w3id.org/sdp/core#includesSPC-BP
:includesSPC-BP rdf:type owl:ObjectProperty ;
                rdfs:domain :StatisticalProgramCycle ;
                rdfs:range :BusinessProcess .


###  https://w3id.org/sdp/core#performsSPC-SPD
:performsSPC-SPD rdf:type owl:ObjectProperty ;
                 rdfs:domain :StatisticalProgramCycle ;
                 rdfs:range :StatisticalProgramDesign .


###  https://w3id.org/sdp/core#refersToCI-IA
:refersToCI-IA rdf:type owl:ObjectProperty ;
               rdfs:domain :CoreInput ;
               rdfs:range gsim-sum:IdentifiableArtefact .


###  https://w3id.org/sdp/core#refersToCO-IA
:refersToCO-IA rdf:type owl:ObjectProperty ;
               rdfs:domain :CoreOutput ;
               rdfs:range gsim-sum:IdentifiableArtefact .


###  https://w3id.org/sdp/core#refersToPSI-IA
:refersToPSI-IA rdf:type owl:ObjectProperty ;
                rdfs:domain :ProcessSupportInput ;
                rdfs:range gsim-sum:IdentifiableArtefact .


###  https://w3id.org/sdp/core#specifiesPD-PS
:specifiesPD-PS rdf:type owl:ObjectProperty ;
                rdfs:domain :ProcessDesign ;
                rdfs:range :ProcessStep .


###  https://w3id.org/sdp/core#usesSP-SPD
:usesSP-SPD rdf:type owl:ObjectProperty ;
            rdfs:domain :StatisticalProgram ;
            rdfs:range :StatisticalProgramDesign .


###  https://w3id.org/sdp/core#usesSPD-PD
:usesSPD-PD rdf:type owl:ObjectProperty ;
            rdfs:domain :StatisticalProgramDesign ;
            rdfs:range :ProcessDesign .


#################################################################
#    Data properties
#################################################################

###  http://rdf.unece.org/models/cspa#additionalInformation
cspa:additionalInformation rdf:type owl:DatatypeProperty ;
                           rdfs:domain cspa:Documentation ;
                           rdfs:range xsd:string ;
                           rdfs:comment "Information which does not fit elsewhere." ;
                           rdfs:label "Additional information" .


###  http://rdf.unece.org/models/cspa#dataByReferenceProtocol
cspa:dataByReferenceProtocol rdf:type owl:DatatypeProperty ;
                             rdfs:domain cspa:ImplementationInput ;
                             rdfs:range xsd:string ;
                             rdfs:label "Data by reference Protocol" .


###  http://rdf.unece.org/models/cspa#description
cspa:description rdf:type owl:DatatypeProperty ;
                 rdfs:domain cspa:DescriptionLevel ,
                             cspa:PackageOrFunction ,
                             cspa:PropertyTopic ;
                 rdfs:range xsd:string ;
                 rdfs:label "Description" .


###  http://rdf.unece.org/models/cspa#label
cspa:label rdf:type owl:DatatypeProperty ;
           rdfs:domain cspa:Dependency ,
                       cspa:DescriptionLevel ,
                       cspa:Identifier ,
                       cspa:Input ,
                       cspa:Interface ,
                       cspa:Output ,
                       cspa:PackageOrFunction .


###  http://rdf.unece.org/models/cspa#methods
cspa:methods rdf:type owl:DatatypeProperty ;
             rdfs:domain cspa:Documentation ;
             rdfs:range xsd:string ;
             rdfs:comment "Any method used by the service to achieve its goal." ;
             rdfs:label "Methods" .


###  http://rdf.unece.org/models/cspa#organizationName
cspa:organizationName rdf:type owl:DatatypeProperty ;
                      rdfs:subPropertyOf owl:topDataProperty ;
                      rdfs:domain cspa:Organization ;
                      rdfs:range xsd:string ;
                      rdfs:label "Organization name" .


###  http://rdf.unece.org/models/cspa#outcomes
cspa:outcomes rdf:type owl:DatatypeProperty ;
              rdfs:domain cspa:BusinessFunction ;
              rdfs:range xsd:string ;
              rdfs:comment "Outcomes of the service." ;
              rdfs:label "Outcomes" .


###  http://rdf.unece.org/models/cspa#restrictions
cspa:restrictions rdf:type owl:DatatypeProperty ;
                  rdfs:domain cspa:BusinessFunction ;
                  rdfs:range xsd:string ;
                  rdfs:comment "Restrictions of the service." ;
                  rdfs:label "Restrisctions" .


###  http://rdf.unece.org/models/cspa#version
cspa:version rdf:type owl:DatatypeProperty ;
             rdfs:domain cspa:DescriptionLevel ,
                         cspa:PackageOrFunction ;
             rdfs:range xsd:string ;
             rdfs:label "Version" .


###  https://w3id.org/italia/onto/gsim-sum#hasAlgorithm-R
gsim-sum:hasAlgorithm-R rdf:type owl:DatatypeProperty ,
                                 owl:FunctionalProperty ;
                        rdfs:domain gsim-sum:Rule ;
                        rdfs:range xsd:string ;
                        rdfs:comment "The rule expressed as an algorithm"@en .


###  https://w3id.org/italia/onto/gsim-sum#hasBudget-SP
gsim-sum:hasBudget-SP rdf:type owl:DatatypeProperty ;
                      rdfs:domain gsim-sum:StatisticalProgram ;
                      rdfs:range xsd:integer .


###  https://w3id.org/italia/onto/gsim-sum#hasChangeOrigin-EC
gsim-sum:hasChangeOrigin-EC rdf:type owl:DatatypeProperty ;
                            rdfs:domain gsim-sum:EnvironmentChange ;
                            rdfs:range xsd:string .


###  https://w3id.org/italia/onto/gsim-sum#hasConceptualFramework-SPD
gsim-sum:hasConceptualFramework-SPD rdf:type owl:DatatypeProperty ,
                                             owl:FunctionalProperty ;
                                    rdfs:domain gsim-sum:StatisticalProgramDesign ;
                                    rdfs:range xsd:string ;
                                    rdfs:comment "Describe the conceptual framework for the Statistical Program (e.g. SNA)"@en .


###  https://w3id.org/italia/onto/gsim-sum#hasDateEnded-BP
gsim-sum:hasDateEnded-BP rdf:type owl:DatatypeProperty ,
                                  owl:FunctionalProperty ;
                         rdfs:domain gsim-sum:BusinessProcess ;
                         rdfs:range xsd:dateTime .


###  https://w3id.org/italia/onto/gsim-sum#hasDateEnded-SP
gsim-sum:hasDateEnded-SP rdf:type owl:DatatypeProperty ,
                                  owl:FunctionalProperty ;
                         rdfs:domain gsim-sum:StatisticalProgram ;
                         rdfs:range xsd:dateTime .


###  https://w3id.org/italia/onto/gsim-sum#hasDateEnded-SPD
gsim-sum:hasDateEnded-SPD rdf:type owl:DatatypeProperty ,
                                   owl:FunctionalProperty ;
                          rdfs:domain gsim-sum:StatisticalProgramDesign ;
                          rdfs:range xsd:dateTime ;
                          rdfs:comment "Last date of validity"@en .


###  https://w3id.org/italia/onto/gsim-sum#hasDateInitiated-BP
gsim-sum:hasDateInitiated-BP rdf:type owl:DatatypeProperty ,
                                      owl:FunctionalProperty ;
                             rdfs:domain gsim-sum:BusinessProcess ;
                             rdfs:range xsd:dateTime .


###  https://w3id.org/italia/onto/gsim-sum#hasDateInitiated-SP
gsim-sum:hasDateInitiated-SP rdf:type owl:DatatypeProperty ,
                                      owl:FunctionalProperty ;
                             rdfs:domain gsim-sum:StatisticalProgram ;
                             rdfs:range xsd:dateTime .


###  https://w3id.org/italia/onto/gsim-sum#hasDateInitiated-SPD
gsim-sum:hasDateInitiated-SPD rdf:type owl:DatatypeProperty ,
                                       owl:FunctionalProperty ;
                              rdfs:domain gsim-sum:StatisticalProgramDesign ;
                              rdfs:range xsd:dateTime ;
                              rdfs:comment "First date of validity"@en .


###  https://w3id.org/italia/onto/gsim-sum#hasDescription-IA
gsim-sum:hasDescription-IA rdf:type owl:DatatypeProperty ,
                                    owl:FunctionalProperty ;
                           rdfs:domain gsim-sum:IdentifiableArtefact ;
                           rdfs:range xsd:string ;
                           rdfs:comment "The general description of the scope, function, and goals"@en .


###  https://w3id.org/italia/onto/gsim-sum#hasExecutionLog
gsim-sum:hasExecutionLog rdf:type owl:DatatypeProperty ;
                         rdfs:domain gsim:ProcessExecutionLog ;
                         rdfs:range xsd:string .


###  https://w3id.org/italia/onto/gsim-sum#hasHistory-SP
gsim-sum:hasHistory-SP rdf:type owl:DatatypeProperty ,
                                owl:FunctionalProperty ;
                       rdfs:domain gsim-sum:StatisticalProgram ;
                       rdfs:range xsd:string ;
                       rdfs:comment "A description of the precursors of the program within the organization"@en .


###  https://w3id.org/italia/onto/gsim-sum#hasId-IA
gsim-sum:hasId-IA rdf:type owl:DatatypeProperty ;
                  rdfs:domain gsim-sum:IdentifiableArtefact ;
                  rdfs:range xsd:string .


###  https://w3id.org/italia/onto/gsim-sum#hasInformationRequest-IR
gsim-sum:hasInformationRequest-IR rdf:type owl:DatatypeProperty ;
                                  rdfs:domain gsim-sum:InformationRequest ;
                                  rdfs:range xsd:string .


###  https://w3id.org/italia/onto/gsim-sum#hasIssues-Ass
gsim-sum:hasIssues-Ass rdf:type owl:DatatypeProperty ;
                       rdfs:domain gsim-sum:Assessment ;
                       rdfs:range xsd:string .


###  https://w3id.org/italia/onto/gsim-sum#hasLegalFramework-SP
gsim-sum:hasLegalFramework-SP rdf:type owl:DatatypeProperty ,
                                       owl:FunctionalProperty ;
                              rdfs:domain gsim-sum:StatisticalProgram ;
                              rdfs:range xsd:string .


###  https://w3id.org/italia/onto/gsim-sum#hasLegislativeReference-SN
gsim-sum:hasLegislativeReference-SN rdf:type owl:DatatypeProperty ,
                                             owl:FunctionalProperty ;
                                    rdfs:domain gsim-sum:StatisticalProgram ;
                                    rdfs:range xsd:string .


###  https://w3id.org/italia/onto/gsim-sum#hasName-IA
gsim-sum:hasName-IA rdf:type owl:DatatypeProperty ;
                    rdfs:domain gsim-sum:IdentifiableArtefact ;
                    rdfs:range xsd:string .


###  https://w3id.org/italia/onto/gsim-sum#hasOutputs-BC
gsim-sum:hasOutputs-BC rdf:type owl:DatatypeProperty ;
                       rdfs:domain gsim-sum:BusinessCase ;
                       rdfs:range xsd:string .


###  https://w3id.org/italia/onto/gsim-sum#hasReferencePeriodEnd-SPC
gsim-sum:hasReferencePeriodEnd-SPC rdf:type owl:DatatypeProperty ,
                                            owl:FunctionalProperty ;
                                   rdfs:domain gsim-sum:StatisticalProgramCycle ;
                                   rdfs:range xsd:dateTime .


###  https://w3id.org/italia/onto/gsim-sum#hasReferencePeriodStart-SPC
gsim-sum:hasReferencePeriodStart-SPC rdf:type owl:DatatypeProperty ,
                                              owl:FunctionalProperty ;
                                     rdfs:domain gsim-sum:StatisticalProgramCycle ;
                                     rdfs:range xsd:dateTime .


###  https://w3id.org/italia/onto/gsim-sum#hasSourceOfFunding-SP
gsim-sum:hasSourceOfFunding-SP rdf:type owl:DatatypeProperty ,
                                        owl:FunctionalProperty ;
                               rdfs:domain gsim-sum:StatisticalProgram ;
                               rdfs:range xsd:string .


###  https://w3id.org/italia/onto/gsim-sum#hasStatus-BP
gsim-sum:hasStatus-BP rdf:type owl:DatatypeProperty ,
                               owl:FunctionalProperty ;
                      rdfs:domain gsim-sum:BusinessProcess ;
                      rdfs:range xsd:string .


###  https://w3id.org/italia/onto/gsim-sum#hasStatus-SN
gsim-sum:hasStatus-SN rdf:type owl:DatatypeProperty ;
                      rdfs:domain gsim-sum:StatisticalNeed ;
                      rdfs:range xsd:string .


###  https://w3id.org/italia/onto/gsim-sum#hasStatus-SP
gsim-sum:hasStatus-SP rdf:type owl:DatatypeProperty ,
                               owl:FunctionalProperty ;
                      rdfs:domain gsim-sum:StatisticalProgram ;
                      rdfs:range xsd:string ;
                      rdfs:comment "The current condition of the program. e.g. New Proposal, New-Under Development, Current, Completed, Cancelled, Transferred to Another Organization"@en .


###  https://w3id.org/italia/onto/gsim-sum#hasStatus-SPD
gsim-sum:hasStatus-SPD rdf:type owl:DatatypeProperty ,
                                owl:FunctionalProperty ;
                       rdfs:domain gsim-sum:StatisticalProgramDesign ;
                       rdfs:range xsd:string .


###  https://w3id.org/italia/onto/gsim-sum#hasSubjectMatterDomain-SP
gsim-sum:hasSubjectMatterDomain-SP rdf:type owl:DatatypeProperty ,
                                            owl:FunctionalProperty ;
                                   rdfs:domain gsim-sum:StatisticalProgram ;
                                   rdfs:range xsd:string .


###  https://w3id.org/italia/onto/gsim-sum#hasSystemExectableIndicator-R
gsim-sum:hasSystemExectableIndicator-R rdf:type owl:DatatypeProperty ,
                                                owl:FunctionalProperty ;
                                       rdfs:domain gsim-sum:Rule ;
                                       rdfs:range xsd:boolean ;
                                       rdfs:comment "Whether the rule is formatted to be executed by a system, or is only documentary"@en .


###  https://w3id.org/italia/onto/gsim-sum#hasType-PI
gsim-sum:hasType-PI rdf:type owl:DatatypeProperty ,
                             owl:FunctionalProperty ;
                    rdfs:domain gsim-sum:ProcessInput ;
                    rdfs:range xsd:string ;
                    rdfs:comment "e.g. Parameter Input, Process Support Input, Transformable Input"@en .


###  https://w3id.org/italia/onto/gsim-sum#hasType-PO
gsim-sum:hasType-PO rdf:type owl:DatatypeProperty ,
                             owl:FunctionalProperty ;
                    rdfs:domain gsim-sum:ProcessOutput ;
                    rdfs:range xsd:string ;
                    rdfs:comment "e.g. Transformed Output or Process Metric"@en .


###  https://w3id.org/italia/onto/gsim-sum#hasType-R
gsim-sum:hasType-R rdf:type owl:DatatypeProperty ,
                            owl:FunctionalProperty ;
                   rdfs:domain gsim-sum:Rule ;
                   rdfs:range xsd:string ;
                   rdfs:comment "A type taken from a controlled vocabulary."@en .


###  https://w3id.org/italia/onto/gsim-sum#hasValue-IA
gsim-sum:hasValue-IA rdf:type owl:DatatypeProperty ;
                     rdfs:domain gsim-sum:IdentifiableArtefact ;
                     rdfs:range xsd:string .


###  https://w3id.org/sdp/core#coreInputType
:coreInputType rdf:type owl:DatatypeProperty ;
               rdfs:domain :ProcessInputSpecification ;
               rdfs:range xsd:string .


###  https://w3id.org/sdp/core#coreOutputType
:coreOutputType rdf:type owl:DatatypeProperty ;
                rdfs:domain :ProcessOutputSpecification ;
                rdfs:range xsd:string .


###  https://w3id.org/sdp/core#gsbpmProcessType
:gsbpmProcessType rdf:type owl:DatatypeProperty ;
                  rdfs:domain :ProcessStep ;
                  rdfs:range xsd:string .


###  https://w3id.org/sdp/core#hasEndTime-PS
:hasEndTime-PS rdf:type owl:DatatypeProperty ;
               rdfs:domain :ProcessStep ;
               rdfs:range xsd:dateTime .


###  https://w3id.org/sdp/core#hasExecutionLog
:hasExecutionLog rdf:type owl:DatatypeProperty ;
                 rdfs:domain :ProcessExecutionLog ;
                 rdfs:range xsd:string .


###  https://w3id.org/sdp/core#hasStartTime-PS
:hasStartTime-PS rdf:type owl:DatatypeProperty ;
                 rdfs:domain :ProcessStep ;
                 rdfs:range xsd:dateTime .


###  https://w3id.org/sdp/core#parameterInputType
:parameterInputType rdf:type owl:DatatypeProperty ;
                    rdfs:domain :ProcessInputSpecification ;
                    rdfs:range xsd:string .


###  https://w3id.org/sdp/core#processExecutionLogType
:processExecutionLogType rdf:type owl:DatatypeProperty ;
                         rdfs:domain :ProcessOutputSpecification ;
                         rdfs:range xsd:string .


###  https://w3id.org/sdp/core#processMetricType
:processMetricType rdf:type owl:DatatypeProperty ;
                   rdfs:domain :ProcessOutputSpecification ;
                   rdfs:range xsd:string .


###  https://w3id.org/sdp/core#processSupportInputType
:processSupportInputType rdf:type owl:DatatypeProperty ;
                         rdfs:domain :ProcessInputSpecification ;
                         rdfs:range xsd:string .


#################################################################
#    Classes
#################################################################

###  http://rdf.unece.org/models/cspa#BusinessFunction
cspa:BusinessFunction rdf:type owl:Class ;
                      rdfs:subClassOf cspa:PropertyTopic ,
                                      gsim-sum:BusinessFunction ;
                      rdfs:comment "Documents the intented goal of a CSPA service. Useful when someone scroll through many packages to find a relevant one." ;
                      rdfs:label "Business function of a CSPA service" .


###  http://rdf.unece.org/models/cspa#DefinitionDependency
cspa:DefinitionDependency rdf:type owl:Class ;
                          rdfs:subClassOf cspa:StatisticalProductionArchitecture ;
                          rdfs:label "Dependency at the definition description level" .


###  http://rdf.unece.org/models/cspa#DefinitionInput
cspa:DefinitionInput rdf:type owl:Class ;
                     rdfs:subClassOf cspa:StatisticalProductionArchitecture ;
                     rdfs:label "Input at the definition description level" .


###  http://rdf.unece.org/models/cspa#DefinitionInterface
cspa:DefinitionInterface rdf:type owl:Class ;
                         rdfs:subClassOf cspa:StatisticalProductionArchitecture ;
                         rdfs:label "Interface at the definition description level" .


###  http://rdf.unece.org/models/cspa#DefinitionOutput
cspa:DefinitionOutput rdf:type owl:Class ;
                      rdfs:subClassOf cspa:StatisticalProductionArchitecture ;
                      rdfs:label "Output at the definition description level" .


###  http://rdf.unece.org/models/cspa#Dependency
cspa:Dependency rdf:type owl:Class ;
                rdfs:subClassOf cspa:PropertyTopic ;
                owl:disjointUnionOf ( cspa:DefinitionDependency
                                      cspa:ImplementationDependency
                                      cspa:SpecificationDependency
                                    ) ;
                rdfs:comment "A dependency is something needed to run a CSPA service such as an operating system or a database. One instance of the class describe one dependency: there should be as many instances as different dependecies. It can be linked to a description level or to an interface." ;
                rdfs:label "Dependency of a CSPA service" .


###  http://rdf.unece.org/models/cspa#DependencyIdentifier
cspa:DependencyIdentifier rdf:type owl:Class ;
                          rdfs:subClassOf cspa:Identifier ;
                          rdfs:comment "Used to identify one dependency described multiple times at different description levels." ;
                          rdfs:label "Dependency identifier" .


###  http://rdf.unece.org/models/cspa#DescriptionLevel
cspa:DescriptionLevel rdf:type owl:Class ;
                      rdfs:subClassOf cspa:StatisticalProductionArchitecture ;
                      owl:disjointUnionOf ( cspa:ServiceDefinition
                                            cspa:ServiceImplementationDescription
                                            cspa:ServiceSpecification
                                          ) ;
                      rdfs:comment "CSPA offers 3 levels of description: service definition which is the most conceptual, service specification and service implementation description (which is the most physical description level)." ;
                      rdfs:label "CSPA 3 levels of description" .


###  http://rdf.unece.org/models/cspa#Document
cspa:Document rdf:type owl:Class ;
              rdfs:subClassOf cspa:StatisticalProductionArchitecture .


###  http://rdf.unece.org/models/cspa#Documentation
cspa:Documentation rdf:type owl:Class ;
                   rdfs:subClassOf cspa:PropertyTopic ;
                   rdfs:comment "Any kind of information which does not fit elsewhere can be put here." ;
                   rdfs:label "Documentation of a CSPA service" .


###  http://rdf.unece.org/models/cspa#Function
cspa:Function rdf:type owl:Class ;
              rdfs:subClassOf cspa:PackageOrFunction ;
              rdfs:comment "CSPA function or atomic service" ;
              rdfs:label "CSPA Function" .


###  http://rdf.unece.org/models/cspa#FunctionDefinition
cspa:FunctionDefinition rdf:type owl:Class ;
                        rdfs:subClassOf cspa:StatisticalProductionArchitecture ;
                        rdfs:comment "Function description at conceptual level." ;
                        rdfs:label "CSPA function definition" .


###  http://rdf.unece.org/models/cspa#FunctionImplementation
cspa:FunctionImplementation rdf:type owl:Class ;
                            rdfs:subClassOf cspa:StatisticalProductionArchitecture ;
                            rdfs:comment "Function description at physical implementation level." ;
                            rdfs:label "CSPA function implementation" .


###  http://rdf.unece.org/models/cspa#FunctionSpecification
cspa:FunctionSpecification rdf:type owl:Class ;
                           rdfs:subClassOf cspa:StatisticalProductionArchitecture ;
                           rdfs:comment "Function description at logical level." ;
                           rdfs:label "CSPA function specification" .


###  http://rdf.unece.org/models/cspa#Identifier
cspa:Identifier rdf:type owl:Class ;
                rdfs:subClassOf cspa:StatisticalProductionArchitecture ;
                rdfs:comment "Used to identify one object described multiple times at different description levels." ;
                rdfs:label "CSPA Identifier" .


###  http://rdf.unece.org/models/cspa#ImplementationDependency
cspa:ImplementationDependency rdf:type owl:Class ;
                              rdfs:subClassOf cspa:StatisticalProductionArchitecture ;
                              rdfs:label "Dependency at the implementation description level" .


###  http://rdf.unece.org/models/cspa#ImplementationInput
cspa:ImplementationInput rdf:type owl:Class ;
                         rdfs:subClassOf cspa:StatisticalProductionArchitecture ;
                         rdfs:label "Input at the implementation description level" .


###  http://rdf.unece.org/models/cspa#ImplementationInterface
cspa:ImplementationInterface rdf:type owl:Class ;
                             rdfs:subClassOf cspa:StatisticalProductionArchitecture ;
                             rdfs:label "Interface at the implementation description level" .


###  http://rdf.unece.org/models/cspa#ImplementationOutput
cspa:ImplementationOutput rdf:type owl:Class ;
                          rdfs:subClassOf cspa:StatisticalProductionArchitecture ;
                          rdfs:label "Output at the implementation description level" .


###  http://rdf.unece.org/models/cspa#Input
cspa:Input rdf:type owl:Class ;
           rdfs:subClassOf cspa:PropertyTopic ;
           owl:disjointUnionOf ( cspa:DefinitionInput
                                 cspa:ImplementationInput
                                 cspa:SpecificationInput
                               ) ;
           rdfs:comment "One instance of the classs describe one input: there should be as many instances as different inputs." ;
           rdfs:label "Input of a CSPA function" .


###  http://rdf.unece.org/models/cspa#InputIdentifier
cspa:InputIdentifier rdf:type owl:Class ;
                     rdfs:subClassOf cspa:Identifier ;
                     rdfs:comment "Used to identify one input described multiple times at different description levels." ;
                     rdfs:label "Input identifier" .


###  http://rdf.unece.org/models/cspa#Interface
cspa:Interface rdf:type owl:Class ;
               rdfs:subClassOf cspa:PropertyTopic ;
               owl:disjointUnionOf ( cspa:DefinitionInterface
                                     cspa:ImplementationInterface
                                     cspa:SpecificationInterface
                                   ) ;
               rdfs:comment "An interface is a way to call a CSPA service for instance a REST web API." ;
               rdfs:label "Interface of a CSPA service" .


###  http://rdf.unece.org/models/cspa#InterfaceIdentifier
cspa:InterfaceIdentifier rdf:type owl:Class ;
                         rdfs:subClassOf cspa:Identifier ;
                         rdfs:comment "Used to identify one interface described multiple times at different description levels." ;
                         rdfs:label "Interface identifier" .


###  http://rdf.unece.org/models/cspa#LIMClass
cspa:LIMClass rdf:type owl:Class ;
              rdfs:subClassOf cspa:StatisticalProductionArchitecture .


###  http://rdf.unece.org/models/cspa#Organization
cspa:Organization rdf:type owl:Class ;
                  rdfs:subClassOf cspa:StatisticalProductionArchitecture ,
                                  prov:Organization ;
                  rdfs:label "Organization" .


###  http://rdf.unece.org/models/cspa#Output
cspa:Output rdf:type owl:Class ;
            rdfs:subClassOf cspa:PropertyTopic ;
            owl:disjointUnionOf ( cspa:DefinitionOutput
                                  cspa:ImplementationOutput
                                  cspa:SpecificationOutput
                                ) ;
            rdfs:comment "One instance of the classs describe one input: there should be as many instances as different inputs." ;
            rdfs:label "Output of a CSPA function" .


###  http://rdf.unece.org/models/cspa#OutputIdentifier
cspa:OutputIdentifier rdf:type owl:Class ;
                      rdfs:subClassOf cspa:Identifier ;
                      rdfs:comment "Used to identify one output described multiple times at different description levels." ;
                      rdfs:label "Output identifier" .


###  http://rdf.unece.org/models/cspa#Package
cspa:Package rdf:type owl:Class ;
             rdfs:subClassOf cspa:PackageOrFunction ;
             rdfs:comment "CSPA bundle of functions or other packages" ;
             rdfs:label "CSPA Package" .


###  http://rdf.unece.org/models/cspa#PackageDefinition
cspa:PackageDefinition rdf:type owl:Class ;
                       rdfs:subClassOf cspa:StatisticalProductionArchitecture ;
                       rdfs:comment "Package description at conceptual level." ;
                       rdfs:label "CSPA package definition" .


###  http://rdf.unece.org/models/cspa#PackageImplementation
cspa:PackageImplementation rdf:type owl:Class ;
                           rdfs:subClassOf cspa:StatisticalProductionArchitecture ;
                           rdfs:comment "Package description at physical implementation level." ;
                           rdfs:label "CSPA package implementation" .


###  http://rdf.unece.org/models/cspa#PackageOrFunction
cspa:PackageOrFunction rdf:type owl:Class ;
                       rdfs:subClassOf cspa:StatisticalProductionArchitecture ;
                       owl:disjointUnionOf ( cspa:Function
                                             cspa:Package
                                           ) .


###  http://rdf.unece.org/models/cspa#PackageSpecification
cspa:PackageSpecification rdf:type owl:Class ;
                          rdfs:subClassOf cspa:StatisticalProductionArchitecture ;
                          rdfs:comment "Package description at logical level." ;
                          rdfs:label "CSPA package specification" .


###  http://rdf.unece.org/models/cspa#PropertyTopic
cspa:PropertyTopic rdf:type owl:Class ;
                   rdfs:subClassOf cspa:StatisticalProductionArchitecture ;
                   owl:disjointUnionOf ( cspa:BusinessFunction
                                         cspa:Dependency
                                         cspa:Documentation
                                         cspa:Input
                                         cspa:Interface
                                         cspa:Output
                                         cspa:Provenance
                                       ) ;
                   rdfs:comment "The properties used to describe CSPA function and packages are numerous and designed to be extended. To ease the finding of relevant information, properties are grouped by topics. One topic (such as Input or Output) can be sevaral time in a description level." ;
                   rdfs:label "Properties about CSPA function or package grouped by topic." .


###  http://rdf.unece.org/models/cspa#Provenance
cspa:Provenance rdf:type owl:Class ;
                rdfs:subClassOf cspa:PropertyTopic ,
                                prov:Entity ;
                rdfs:comment "The provenance of a CSPA service says who did what in the building of a CSPA package or function." ;
                rdfs:label "Provenance of a CSPA service" .


###  http://rdf.unece.org/models/cspa#ServiceDefinition
cspa:ServiceDefinition rdf:type owl:Class ;
                       rdfs:subClassOf cspa:DescriptionLevel ;
                       owl:disjointUnionOf ( cspa:FunctionDefinition
                                             cspa:PackageDefinition
                                           ) ;
                       rdfs:comment "Function or package description at conceptual level." ;
                       rdfs:label "CSPA package or function definition" .


###  http://rdf.unece.org/models/cspa#ServiceImplementation
cspa:ServiceImplementation rdf:type owl:Class ;
                           rdfs:subClassOf cspa:StatisticalProductionArchitecture .


###  http://rdf.unece.org/models/cspa#ServiceImplementationDescription
cspa:ServiceImplementationDescription rdf:type owl:Class ;
                                      rdfs:subClassOf cspa:DescriptionLevel ;
                                      owl:disjointUnionOf ( cspa:FunctionImplementation
                                                            cspa:PackageImplementation
                                                          ) ;
                                      rdfs:comment "Function or package description at physical level." ;
                                      rdfs:label "CSPA package or function implementation description" .


###  http://rdf.unece.org/models/cspa#ServiceSpecification
cspa:ServiceSpecification rdf:type owl:Class ;
                          rdfs:subClassOf cspa:DescriptionLevel ;
                          owl:disjointUnionOf ( cspa:FunctionSpecification
                                                cspa:PackageSpecification
                                              ) ;
                          rdfs:comment "Function or package description at logical level." ;
                          rdfs:label "CSPA package or function specification" .


###  http://rdf.unece.org/models/cspa#SpecificationDependency
cspa:SpecificationDependency rdf:type owl:Class ;
                             rdfs:subClassOf cspa:StatisticalProductionArchitecture ;
                             rdfs:label "Dependency at the specification description level" .


###  http://rdf.unece.org/models/cspa#SpecificationInput
cspa:SpecificationInput rdf:type owl:Class ;
                        rdfs:subClassOf cspa:StatisticalProductionArchitecture ;
                        rdfs:label "Input at the specification description level" .


###  http://rdf.unece.org/models/cspa#SpecificationInterface
cspa:SpecificationInterface rdf:type owl:Class ;
                            rdfs:subClassOf cspa:StatisticalProductionArchitecture ;
                            rdfs:label "Interface at the specification description level" .


###  http://rdf.unece.org/models/cspa#SpecificationOutput
cspa:SpecificationOutput rdf:type owl:Class ;
                         rdfs:subClassOf cspa:StatisticalProductionArchitecture ;
                         rdfs:label "Output at the specification description level" .


###  http://rdf.unece.org/models/cspa#StatisticalProductionArchitecture
cspa:StatisticalProductionArchitecture rdf:type owl:Class .


###  http://rdf.unece.org/models/gamso#CapabilityDevelopmentActivity
gamso:CapabilityDevelopmentActivity rdf:type owl:Class ;
                                    rdfs:subClassOf gamso:StatisticalSupportingActivity .


###  http://rdf.unece.org/models/gamso#CorporateSupportActivity
gamso:CorporateSupportActivity rdf:type owl:Class ;
                               rdfs:subClassOf gamso:StatisticalSupportingActivity .


###  http://rdf.unece.org/models/gamso#GenericActivityModelforStatisticalOrganisations
gamso:GenericActivityModelforStatisticalOrganisations rdf:type owl:Class ;
                                                      rdfs:subClassOf prov:Activity ;
                                                      rdfs:comment """The Generic Activity Model for Statistical Organisations (GAMSO) describes and defines the activities that take place within a typical organisation that produces official statistics. It extends and complements the Generic Statistical Business Process Model (GSBPM) by adding additional activities needed to support statistical production. The GAMSO describes activities – that is, what statistical organisations do – while the GSBPM describes the process – that is, how statistical organisations undertake the activity of statistical production.

Like the GSBPM, the GAMSO aims to provide a common vocabulary and framework to support international collaboration activities, particularly in the field of modernisation.  While individual collaboration typically focuses on modernising a particular aspect of production (as described by the GSBPM), statistical production occurs within a broader context of corporate strategies, capabilities and support. The GAMSO helps to place collaboration in the wider context."""@en .


###  http://rdf.unece.org/models/gamso#StatisticalSupportingActivity
gamso:StatisticalSupportingActivity rdf:type owl:Class ;
                                    rdfs:subClassOf gamso:GenericActivityModelforStatisticalOrganisations .


###  http://rdf.unece.org/models/gamso#StrategyAndLeadershipActivity
gamso:StrategyAndLeadershipActivity rdf:type owl:Class ;
                                    rdfs:subClassOf gamso:StatisticalSupportingActivity .


###  http://rdf.unece.org/models/gsbpm#Phase
gsbpm:Phase rdf:type owl:Class ;
            rdfs:subClassOf gsbpm:StatisticalProductionActivity ;
            rdfs:label "GSBPM phase" .


###  http://rdf.unece.org/models/gsbpm#StatisticalProductionActivity
gsbpm:StatisticalProductionActivity rdf:type owl:Class ;
                                    rdfs:subClassOf gamso:GenericActivityModelforStatisticalOrganisations ,
                                                    skos:Concept ;
                                    rdfs:isDefinedBy <http://rdf.unece.org/def/gsbpm#> ;
                                    rdfs:label "Activité de production statistique"@fr ,
                                               "Statistical production activity"@en .


###  http://rdf.unece.org/models/gsbpm#SubProcess
gsbpm:SubProcess rdf:type owl:Class ;
                 rdfs:subClassOf gsbpm:StatisticalProductionActivity ;
                 rdfs:label "GSBPM sub-process"@en .


###  http://rdf.unece.org/models/gsim#ChangeEvent
gsim:ChangeEvent rdf:type owl:Class ;
                 rdfs:subClassOf gsim-sum:StatisticalGenericInformationModel ;
                 rdfs:comment "A Change Event relates to the information class(es) that has(have) been affected. It can be applied to only one Identifiable Artefact and result in one or more Identifiable Artefact(s). On the other hand, a Change Event can be applied to more than one Identifiable Artefact and result in only one Identifiable Artefact."@en ;
                 rdfs:isDefinedBy "ndication of the occurrence of a change to an Identifiable Artefact"@en .


###  http://rdf.unece.org/models/gsim#Contact
gsim:Contact rdf:type owl:Class ;
             rdfs:subClassOf gsim:Role ;
             rdfs:isDefinedBy "Role in which Individual(s) is(are) responsible for providing additional information about an information class and/or its metadata, either directly or indirectly by linking to its source."@en .


###  http://rdf.unece.org/models/gsim#CoreInput
gsim:CoreInput rdf:type owl:Class ;
               rdfs:subClassOf gsim-sum:ProcessInput ;
               rdfs:comment "Core Input is a sub-type of Process Input. Producers of official statistics often conceptualise data (and sometimes metadata) flowing through the statistical Business Process, having statistical value added by each Process Step. The concept of Core Input allows this notional flow of information through the production process to be traced, without confusing these inputs with other inputs - such as Parameter Inputs and Process Support Inputs that are controlling or influencing a particular Process Step but do not flow through the Business Process in the same sense. Typical Core Inputs are Data Sets and structural metadata."@en ;
               rdfs:isDefinedBy "essential input for the Process Step Instance"@en .


###  http://rdf.unece.org/models/gsim#CoreOutput
gsim:CoreOutput rdf:type owl:Class ;
                rdfs:subClassOf gsim-sum:ProcessOutput ;
                rdfs:comment "A Core Output is a sub-type of Process Output. Typically a Core Output is either a Process Input to a subsequent Process Step or it represents the final product from a statistical Business Process. In many cases a Core Output may be readily identified as an updated (value added) version of one or more Core Inputs supplied to the Process Step Instance."@en ;
                rdfs:isDefinedBy "key output of the Process Step Instance"@en .


###  http://rdf.unece.org/models/gsim#DataHarvest
gsim:DataHarvest rdf:type owl:Class ;
                 rdfs:subClassOf gsim:ExchangeInstrumen ;
                 rdfs:comment "Examples of Data Harvest include web scraper, API (e.g., to acquire data from administrative sources), scanner, sensor, etc."@en ;
                 rdfs:isDefinedBy "Exchange Instrument to pass information between two sources, usually by a machine to machine mechanism"@en .


###  http://rdf.unece.org/models/gsim#DataRecord
gsim:DataRecord rdf:type owl:Class ;
                rdfs:subClassOf gsim-sum:Structures ;
                rdfs:comment "For example (1212123, 48, American, United Kingdom) specifies the age (48) in years, the current citizenship (American), and the country of birth (United Kingdom) for a person with social security number 1212123. For the case of unit data, it can be structured by Logical Record."@en ;
                rdfs:isDefinedBy "collection of Data Points related to a given Unit or Population"@en .


###  http://rdf.unece.org/models/gsim#DisseminationInstrument
gsim:DisseminationInstrument rdf:type owl:Class ;
                             rdfs:subClassOf gsim:ExchangeInstrumen ;
                             rdfs:comment "Examples include: API or web services for data dissemination"@en ;
                             rdfs:isDefinedBy "Exchange Instrument to disseminate information"@en .


###  http://rdf.unece.org/models/gsim#ExchangeInstrumen
gsim:ExchangeInstrumen rdf:type owl:Class ;
                       rdfs:subClassOf gsim-sum:Exchange ;
                       rdfs:comment "The Exchange Instrument is a tool to receive or send information and is used for external and internal purposes. Different Exchange Instruments are used for data acquisition and dissemination. An example of Exchange Instrument for receiving information is Questionnaire. An example of Exchange Instrument for sending information is Dissemination Instrument. Additional Exchange Instruments can be added to the model as needed by individual organisations."@en ;
                       rdfs:isDefinedBy "concrete and usable tool to exchange information"@en .


###  http://rdf.unece.org/models/gsim#ExchangeSpecification
gsim:ExchangeSpecification rdf:type owl:Class ;
                           rdfs:subClassOf gsim-sum:Exchange ;
                           rdfs:comment "GSBPM Phase 2 (Design) results in an Exchange Specification that specifies the design of the data acquisition or dissemination instruments (e.g., Questionnaire, web page). In GSBPM Phase 3 (Build), these instruments are built based on the tools."@en ;
                           rdfs:isDefinedBy "outline or description specifying the design of the Exchange Instrument"@en .


###  http://rdf.unece.org/models/gsim#Individual
gsim:Individual rdf:type owl:Class ;
                rdfs:subClassOf gsim-sum:Agent ;
                rdfs:isDefinedBy "person who acts, or is designated to act towards a specific purpose"@en .


###  http://rdf.unece.org/models/gsim#InformationCustomer
gsim:InformationCustomer rdf:type owl:Class ;
                         rdfs:subClassOf gsim-sum:Exchange ;
                         rdfs:comment "The Information Consumer accesses a set of information in a Product that is made available via a Dissemination Instrument. The Information Consumer subscribes to the Provision Agreement, which sets out conditions of access. The Information Consumer can be defined in a broad sense with a persona concept (group of Individuals) without specific details."@en ;
                         rdfs:isDefinedBy "Role that entails consuming data and information"@en .


###  http://rdf.unece.org/models/gsim#InformationProvider
gsim:InformationProvider rdf:type owl:Class ;
                         rdfs:subClassOf gsim-sum:Exchange ;
                         rdfs:comment "An Information Provider possesses sets of information (that it has acquired, for example by collecting or purchasing it) and is willing to supply that information (data or referential metadata) to the statistical organisation. The two parties use a Provision Agreement to agree on the Data Structure and Referential Metadata Structure of the data to be exchanged via an Exchange Instrument."@en ;
                         rdfs:isDefinedBy "Role that entails providing data and information"@en .


###  http://rdf.unece.org/models/gsim#InformationStructure
gsim:InformationStructure rdf:type owl:Class ;
                          rdfs:subClassOf gsim-sum:Structures ;
                          rdfs:isDefinedBy "describes the structure of an Information Set"@en .


###  http://rdf.unece.org/models/gsim#Maintainer
gsim:Maintainer rdf:type owl:Class ;
                rdfs:subClassOf gsim:Role ;
                rdfs:comment "A unit or group of persons with the role of Maintainer is responsible for all administrative and operational issues relating to one or a set of information classes and its metadata (e.g. adding, modifying or deleting metadata about an information class). It is answerable to all stakeholders for all issues related to the information classes under its responsibility. A Maintainer is not a decision-making body. Decisions are made collaboratively among the owners of the artefact."@en ;
                rdfs:isDefinedBy "Role in which a unit or group of persons within the Organisation is responsible for managing an information class and its metadata"@en .


###  http://rdf.unece.org/models/gsim#MeasurementType
gsim:MeasurementType rdf:type owl:Class ;
                     rdfs:subClassOf gsim-sum:Concepts ;
                     rdfs:comment "The Measurement Type groups all Measurement Units, which can be converted into each other. A Measurement Type can have a standard Measurement Unit, which can be used for conversion between different Measurement Units. There need not be any standard Measurement Unit for a given Measurement Type e.g. currency. Each Measurement Type has as a standard at most one Measurement Unit."@en ;
                     rdfs:isDefinedBy "defines the type of a measure e.g. mass or currency."@en .


###  http://rdf.unece.org/models/gsim#MeasurementUnit
gsim:MeasurementUnit rdf:type owl:Class ;
                     rdfs:subClassOf gsim-sum:Concepts ;
                     rdfs:comment "Measurement Unit is a definite magnitude of a quantity, defined and adopted by convention or by law, that is used as a standard for measurement of the same kind of quantity. Measurement Units can be based on different Measurement Types such as weight, height, currency, duration etc. Measurement Units can be transformed into one another (e.g. kilometres into metres) if they refer to the same Measurement Type (e.g. length). The conversion rule attribute can be used to include a multiplicative factor e.g. the non-standard Measurement Unit 1000 kg = 1000 x the standard Measurement Unit kg."@en ;
                     rdfs:isDefinedBy "metric for a measurement in terms of an official unit of measurement"@en .


###  http://rdf.unece.org/models/gsim#Organisations
gsim:Organisations rdf:type owl:Class ;
                   rdfs:subClassOf gsim-sum:Agent ;
                   rdfs:comment "Organisation represents a collection of people organised together, often with hierarchical structures. Examples of Organisation: national statistics office, international agency"@en ;
                   rdfs:isDefinedBy "unique framework of authority within which a person or persons act, or are designated to act, towards some purpose."@en .


###  http://rdf.unece.org/models/gsim#Owner
gsim:Owner rdf:type owl:Class ;
           rdfs:subClassOf gsim:Role ;
           rdfs:comment "Some information classes may have several Owners."@en ;
           rdfs:isDefinedBy "Role in which a statistical office, authority or other organisation is responsible for defining, specifying, creating and making decisions about the maintenance of a class and/or its metadata."@en .


###  http://rdf.unece.org/models/gsim#ParameterInput
gsim:ParameterInput rdf:type owl:Class ;
                    rdfs:subClassOf gsim-sum:ProcessInput ;
                    rdfs:comment "Parameter Inputs may be provided where Rules and/or Business Service interfaces associated with a particular Process Step have been designed to be configurable based on Process Input Specification. Parameter Inputs are passed into the Process Step Instance."@en ;
                    rdfs:isDefinedBy "Process Input that specifies the run-time configuration used in a parameterised Process Step Instance"@en .


###  http://rdf.unece.org/models/gsim#ProcessExecutionLog
gsim:ProcessExecutionLog rdf:type owl:Class ;
                         rdfs:subClassOf gsim-sum:ProcessOutput ;
                         rdfs:comment "It may include data that was recorded during the real-time execution of the Process Step."@en ;
                         rdfs:isDefinedBy "Process Output listing events generated by a Process Step Instance"@en .


###  http://rdf.unece.org/models/gsim#ProcessMetric
gsim:ProcessMetric rdf:type owl:Class ;
                   rdfs:subClassOf gsim-sum:ProcessOutput ;
                   rdfs:comment "A Process Metric is a sub-type of Process Output which records information about the execution of a Process Step. For example, how long it took to complete execution of the Process Step and what percentage of records in the Core Input was updated by the Process Step to produce the Core Output. One purpose for a Process Metric may be to provide a quality measure related to the Core Output. For example, a Process Step with the Business Function of imputing missing values is likely to result, as its Core Output, in a Data Set where values that were missing previously have been imputed. Statistical quality measures, captured as Process Metrics for that Process Step may include a measure of how many records were imputed, and a measure of how much difference, statistically, the imputed values make to the dataset overall which can be also used as a part of a quality report associated with the Data Set produced. Another purpose for a Process Metric may be to measure an aspect of the Process Step which is not directly related to the Core Output it produced. For example, a Process Metric may record the time taken to complete the Process Step or other forms of resource utilisation (for example, human and/or IT). Often these two kinds of Process Metrics will be used in combination when seeking to, for example, monitor and tune a statistical Business Process so its statistical outputs achieve the highest level of quality possible based on the time, staff and/or IT resources that are available."@en ;
                   rdfs:isDefinedBy "Process Output summarising some aspect or property of the execution"@en .


###  http://rdf.unece.org/models/gsim#ProcessSupportInput
gsim:ProcessSupportInput rdf:type owl:Class ;
                         rdfs:subClassOf gsim-sum:ProcessInput ;
                         rdfs:comment """Process Support Input is a sub-type of Process Input.
- Examples of Process Support Inputs could include: A technical or methodological handbook which can be used as a reference to assist the work performed (e.g. data editing, coding and classification)
- An auxiliary Data Set which will influence imputation for, or editing of, a primary Data Set which has been submitted to the Process Step as the Core Input
- A Provision Agreement which can be used as a supporting document
- A repository or inventory of Process Methods or software system / architecture that are approved in the Organisation that could be used as reference"""@en ;
                         rdfs:isDefinedBy "Process Input that influences the work performed by the Process Step Instance by providing additional information that affects the way Core Input is used"@en .


###  http://rdf.unece.org/models/gsim#Product
gsim:Product rdf:type owl:Class ;
             rdfs:subClassOf gsim-sum:Exchange ;
             rdfs:comment "A Product packages Information Sets for an Information Consumer. The Product is generated according to Output Specifications, which define how the information from the Information Sets are presented (via Presentations) to the Information Consumer. A Provision Agreement between the statistical organisation and the Information Consumer governs the use of a Product by the Information Consumer. The Provision Agreement, which may be explicitly or implicitly agreed, provides the legal or other bases by which the two parties agree to exchange data. In many cases, dissemination Provision Agreements are implicit in the terms of use published by the statistical organisation. For static Products (e.g. paper publications), specifications are predetermined. For dynamic Products, aspects of specification could be determined by the Information Consumer at run time. Both cases result in Output Specifications specifying Information Set data or referential metadata that will be included within the Product."@en ;
             rdfs:isDefinedBy "package of content that can be disseminated as a whole"@en .


###  http://rdf.unece.org/models/gsim#QuestionBlock
gsim:QuestionBlock rdf:type owl:Class ;
                   rdfs:subClassOf gsim-sum:Exchange ;
                   rdfs:comment """A Question Block should ideally be designed for reuse. The Question Block is a type of Questionnaire Component. A statistical organisation will often have a number of Question Blocks which they reuse in a number of Questionnaires. Examples of Question Blocks include:
- Household Question Block
- Income Question Block
- Employment Question Block"""@en ;
                   rdfs:isDefinedBy "set of Questions, Statements or instructions which are used together"@en .


###  http://rdf.unece.org/models/gsim#Questionnaire
gsim:Questionnaire rdf:type owl:Class ;
                   rdfs:subClassOf gsim:ExchangeInstrumen ;
                   rdfs:comment "This is an example of a way statistical organisations acquire information (an Exchange Instrument). Each collection mode (e.g. in-person, CAPI (Computer-assisted personal interviewing), online Questionnaire) should be interpreted as a new Questionnaire derived from the Questionnaire Specification. The Questionnaire is a tool in which data is obtained."@en ;
                   rdfs:isDefinedBy "Exchange Instrument to elicit information from observation Units"@en .


###  http://rdf.unece.org/models/gsim#ReferentialMetadataSet
gsim:ReferentialMetadataSet rdf:type owl:Class ;
                            rdfs:subClassOf gsim-sum:Structures ;
                            rdfs:comment "Each Referential Metadata Set uses a Referential Metadata Structure to define a structured list of Referential Metadata Attributes for a given Referential Metadata Subject Item."@en ;
                            rdfs:isDefinedBy "organised collection of referential metadata for a given Referential Metadata Subject Item"@en .


###  http://rdf.unece.org/models/gsim#Register
gsim:Register rdf:type owl:Class ;
              rdfs:subClassOf gsim-sum:Exchange ;
              rdfs:comment """In official statistics, statistical registers and adminisitrative registers (registers maintained by other organisations, usually administrative data owners) are usually distinguished. In GSIM, the information class Register is used to describe both types because the attributes are more or less the same so from the information management point of view, they can be handled as one GSIM class. There is usually a purpose or authority for maintaining the Register and each object in the Register is described using a pre-defined set of characteristics. Examples include business and population registers as used by statistical organisations. Therefore, from statistical perspective, the Register can be interpreted as a set of objects for a given Population, updated on a regular basis, containing information on identification, accessibility of Units and other attributes. The Register contains the current and historical statuses of the Population and the causes, effects and sources of alterations in the Population. In order to better understand how the Register is used in GSIM, the use cases for the different scenarios are explained. These scenarios are:
- Register _as Information Set_ maintained and regularly updated by the statistical organisation.
- Register _as Information Set_ for survey frames/sample frames.
- Register _as Information Set_ for statistical Products.
- Register _as Information Set_ used as direct or auxiliary information for the production of statistics.
- Register _as Information Set_ as a source of administrative information obtained usually from external organisations."""@en ;
              rdfs:isDefinedBy "written and complete record containing regular entries of items and details on particular sets of objects"@en .


###  http://rdf.unece.org/models/gsim#Role
gsim:Role rdf:type owl:Class ;
          rdfs:subClassOf gsim-sum:Base ;
          rdfs:comment "Part played by an Individual, an Organisation (or part of it) or a Software Agent in a particular situation. Examples: Contact, data steward, scheduler. Role can be maintained by a controlled vocabulary (e.g. RASCI)."@en ;
          rdfs:isDefinedBy "function assumed by an Agent"@en .


###  http://rdf.unece.org/models/gsim#SentinelValueDomain
gsim:SentinelValueDomain rdf:type owl:Class ;
                         rdfs:subClassOf gsim-sum:ValueDomain ;
                         rdfs:comment "A sentinel value is one used for processing and with no subject matter content, such as missing or refused. Sentinel Value Domains can be enumerated (listed) or described. A Value Domain expressed as a list of Categories _for sentinel values or a description thereof. The scope and the meaning of the possible values are defined within the frame of the Conceptual Domain_ that the Sentinel Value Domain is associated with. Separating the sentinel values from the substantive ones allows a large reduction in the number of Value Domains, and thus Represented Variables and Instance Variables, that need to be maintained. Use of generic codes is recommended for Concepts which appear in many, if not, all Code Lists, e.g. <S_X, Unspecified>, <S_Z, Not applicable>, < S_R, Refusal>, <S_U, Unknown>"@en ;
                         rdfs:isDefinedBy "Value Domain containing sentinel values, i.e. processing-related special values"@en .


###  http://rdf.unece.org/models/gsim#SoftwareAgent
gsim:SoftwareAgent rdf:type owl:Class ;
                   rdfs:subClassOf gsim-sum:Agent ;
                   rdfs:comment "Examples: google bot"@en ;
                   rdfs:isDefinedBy "software that carries out Process Step based on Process Control"@en .


###  http://rdf.unece.org/models/gsim#SubstantiveValueDomain
gsim:SubstantiveValueDomain rdf:type owl:Class ;
                            rdfs:subClassOf gsim-sum:ValueDomain ;
                            rdfs:comment "A substantive value is one representing subject matter content, such as <f, female> in a gender classification. The scope and the meaning of the possible values are defined within the frame of the Conceptual Domain that the Substantive Value Domain is associated with. Example: <0, Pre-primary>, <1, Primary>, <2, Lower secondary>, < 3, Upper secondary>, <4, Post-secondary non-tertiary>, <5, First stage of tertiary education>, <6, Second stage of tertiary education> where the scope and meaning of the values are defined within Categories for levels of education."@en ;
                            rdfs:isDefinedBy "Value Domain containing substantive values, where a substantive value is subject matter related"@en .


###  http://rdf.unece.org/models/gsim#Universe
gsim:Universe rdf:type owl:Class ;
              rdfs:subClassOf gsim-sum:Concept ;
              rdfs:comment "The description statement of a Universe is generally stated in inclusive terms such as All persons with a university degree. Occasionally a Universe is defined by what it excludes, i.e., All persons except those with a university degree. In both cases, adding the condition of the university degree specializes persons, which is a Unit Type."@en ;
              rdfs:isDefinedBy "specialized Unit Type, but not by time or geography"@en .


###  http://www.w3.org/2004/02/skos/core#Concept
skos:Concept rdf:type owl:Class .


###  http://www.w3.org/2004/02/skos/core#ConceptScheme
skos:ConceptScheme rdf:type owl:Class .


###  http://www.w3.org/ns/prov#Activity
prov:Activity rdf:type owl:Class .


###  http://www.w3.org/ns/prov#Entity
prov:Entity rdf:type owl:Class .


###  http://www.w3.org/ns/prov#Organization
prov:Organization rdf:type owl:Class .


###  https://w3id.org/italia/onto/gsim-sum#AdministrativeDetails
gsim-sum:AdministrativeDetails rdf:type owl:Class ;
                               rdfs:subClassOf gsim-sum:StatisticalGenericInformationModel ;
                               rdfs:comment "The Administrative Details object is designed to act as a 'placeholder' to allow for future extensions to the existing model. It allows for further information to be added about the administrative details required to maintain the other objects outlined by GSIM."@en ;
                               rdfs:isDefinedBy "A placeholder for extensions to the model based on an organization’s administrative needs."@en .


###  https://w3id.org/italia/onto/gsim-sum#Agent
gsim-sum:Agent rdf:type owl:Class ;
               rdfs:subClassOf gsim-sum:Base ;
               rdfs:comment "An Agent may be an Individual, an Organisation (or part of it) or a Software Agent that affects in some way an instance of a GSIM class. For example, an Agent can play a role in the execution of a Business Processes or in the way a Statistical Classification (or a Concept) changes over time."@en ;
               rdfs:isDefinedBy "someone or something that plays an active role in the lifecycle of an Identifiable Artefact"@en .


###  https://w3id.org/italia/onto/gsim-sum#AgentInRole
gsim-sum:AgentInRole rdf:type owl:Class ;
                     rdfs:subClassOf gsim-sum:StatisticalGenericInformationModel ;
                     rdfs:comment "In the Organization Ontology from W3C Agent In Role is called a Post."@en ;
                     rdfs:isDefinedBy "an Agent acting in a specific Role"@en .


###  https://w3id.org/italia/onto/gsim-sum#Assessment
gsim-sum:Assessment rdf:type owl:Class ;
                    rdfs:subClassOf gsim-sum:Business ;
                    rdfs:comment """An Assessment can be of a variety of types. One example may include a gap analysis, where a current state is determined along with what is needed to reach its target state. Alternately, an Assessment may compare current processes against a set of requirements, for example a new Statistical Need or change in the operating environment.
An Assessment can use various information objects as inputs, whether they are the main objects that the Assessment is about or auxiliary information objects that help accomplish the Assessment."""@en ;
                    rdfs:isDefinedBy "The result of the analysis of the quality and effectiveness of any activity undertaken by a statistical organization and recommendations on how these can be improved."@en .


###  https://w3id.org/italia/onto/gsim-sum#AttributeComponent
gsim-sum:AttributeComponent rdf:type owl:Class ;
                            rdfs:subClassOf gsim-sum:DataStructureComponent ;
                            rdfs:comment "For example the publication status of an observation (e.g. provisional, final, revised)."@en ;
                            rdfs:isDefinedBy "The role given to a Represented Variable in the context of a Data Structure, which supplies information other than identification or measures."@en .


###  https://w3id.org/italia/onto/gsim-sum#Base
gsim-sum:Base rdf:type owl:Class ;
              rdfs:subClassOf gsim-sum:IdentifiableArtefact ;
              rdfs:comment "Base Group provides features that are reusable by other classes to support functionality such as identity and versioning."@en .


###  https://w3id.org/italia/onto/gsim-sum#Business
gsim-sum:Business rdf:type owl:Class ;
                  rdfs:subClassOf gsim-sum:IdentifiableArtefact ;
                  rdfs:comment "Business Group is used to capture the designs and plans of statistical programmes, and the processes undertaken to deliver those programmes."@en .


###  https://w3id.org/italia/onto/gsim-sum#BusinessCase
gsim-sum:BusinessCase rdf:type owl:Class ;
                      rdfs:subClassOf gsim-sum:Business ;
                      rdfs:comment "A Business Case is produced as a result of a detailed consideration of a Change Definition. It sets out a plan for how the change described by the Change Definition can be achieved. A Business Case usually comprises various evaluations. The Business Case will specify the stakeholders that are impacted by the Statistical Need or by the different solutions that are required to implement it."@en ;
                      rdfs:isDefinedBy "A proposal for a body of work that will deliver outputs designed to achieve outcomes. A Business Case will provide the reasoning for undertaking a Statistical Support Program to initiate a new Statistical Program Design for an existing Statistical Program, or an entirely new Statistical Program, as well as the details of the change proposed."@en .


###  https://w3id.org/italia/onto/gsim-sum#BusinessFunction
gsim-sum:BusinessFunction rdf:type owl:Class ;
                          rdfs:subClassOf gsim-sum:Business ;
                          rdfs:comment """A Business Function delivers added value from a business point of view. It is delivered by bringing together people, processes and technology (resources), for a specific business purpose. Business Functions answer in a generic sense \"What business purpose does this Business Service or Process Step serve?\" Through identifying the Business Function associated with each Business Service or Process Step it increases the documentation of the use of the associated Business Services and Process Steps, to enable future reuse.
A Business Function may be defined directly with descriptive text and/or through reference to an existing catalogue of Business Functions. The phases and sub processes defined within GSBPM can be used as an internationally agreed basis for cataloguing high level Business Functions. A catalogue might also include Business Functions defined at a lower level than \"sub process\". For example, \"Identify and address outliers\" might be catalogued as a lower level Business Function with the \"Review, validate and edit\" function (5.3) defined within GSBPM."""@en ;
                          rdfs:isDefinedBy "Something an enterprise does, or needs to do, in order to achieve its objectives."@en .


###  https://w3id.org/italia/onto/gsim-sum#BusinessProcess
gsim-sum:BusinessProcess rdf:type owl:Class ;
                         rdfs:subClassOf gsim-sum:Business ;
                         rdfs:comment "For example, a particular Statistical Program Cycle might include several data collection activities, the corresponding editing activities for each collection and the production and dissemination of final outputs. Each of these may be considered separate Business Processes for the Statistical Program Cycle."@en ;
                         rdfs:isDefinedBy "The set of Process Steps to perform one of more Business Functions to deliver a Statistical Program Cycle or Statistical Support Program." .


###  https://w3id.org/italia/onto/gsim-sum#BusinessService
gsim-sum:BusinessService rdf:type owl:Class ;
                         rdfs:subClassOf gsim-sum:Business ;
                         rdfs:comment """A Business Service may provide one means of accessing a particular Business Function. The operation of a Business Service will perform one or more Business Processes. The explicitly defined interface of a Business Service can be seen as representing a \"service contract\". If particular inputs are provided then the service will deliver particular outputs in compliance within specific parameters (for example, within a particular period of time). Note: The interface of a Business Service is not necessarily IT based. For example, a typical postal service will have a number of service interfaces:
- Public letter box for posting letters
- Counter at post office for interacting with postal workers."""@en ;
                         rdfs:isDefinedBy "A means of performing a Business Function (an ability that an organization possesses, typically expressed in general and high level terms and requiring a combination of organization, people, processes and technology to achieve)."@en .


###  https://w3id.org/italia/onto/gsim-sum#Category
gsim-sum:Category rdf:type owl:Class ;
                  rdfs:subClassOf gsim-sum:Concept ;
                  rdfs:comment "Categories for the Concept of sex include: Male, Female Note: An extensional definition is a description of a Concept by enumerating all of its sub ordinate Concepts under one criterion or sub division. For example - the Noble Gases (in the periodic table) is extensionally defined by the set of elements including Helium, Neon, Argon, Krypton, Xenon, Radon. (ISO 1087-1)."@en ;
                  rdfs:isDefinedBy "A Concept whose role is to extensionally define and measure a characteristic."@en .


###  https://w3id.org/italia/onto/gsim-sum#CategoryItem
gsim-sum:CategoryItem rdf:type owl:Class ;
                      rdfs:subClassOf gsim-sum:Node ;
                      rdfs:comment "A type of Node particular to a Category Set type of Node Set. A Category Item contains the meaning of a Category without any associated representation."@en ;
                      rdfs:isDefinedBy "An element of a Category Set."@en .


###  https://w3id.org/italia/onto/gsim-sum#CategorySet
gsim-sum:CategorySet rdf:type owl:Class ;
                     rdfs:subClassOf gsim-sum:NodeSet ;
                     rdfs:comment "A Category Set is a type of Node Set which groups Categories through the use of Category Items. The Categories in a Category Set typically have no assigned Designations (Codes). For example: Male, Female."@en ;
                     rdfs:isDefinedBy "A list of Categories."@en .


###  https://w3id.org/italia/onto/gsim-sum#ChangeDefinition
gsim-sum:ChangeDefinition rdf:type owl:Class ;
                          rdfs:subClassOf gsim-sum:Business ;
                          rdfs:comment "A related object - the Statistical Need - is a change expression as it has been received by an organization.A Statistical Need is a raw expression of a proposed change, and is not necessarily well-defined. A Change Definition is created when a Statistical Need is analyzed by an organization, and expresses the raw need in well-defined, structured terms. A Change Definition does not assess the feasibility of the change or propose solutions to deliver the change - this role is satisfied by the Business Case object. The precise structure or organization of a Change Definition can be further specified by rules or standards local to a given organization. It also includes the specific Concepts to be measured and the Population that is under consideration. Once a Statistical Need has been received, the first step is to do the conceptual work to establish what it is we are trying to measure. The final output of this conceptual work is the Change Definition. The next step is to assess how we are going to make the measurements - to design a solution and put forward a proposal for a body of work that will deliver on the requirements of the original Statistical Need. "@en ;
                          rdfs:isDefinedBy "A structured, well-defined specification for a proposed change."@en .


###  https://w3id.org/italia/onto/gsim-sum#ClassificationFamily
gsim-sum:ClassificationFamily rdf:type owl:Class ;
                              rdfs:subClassOf gsim-sum:Concepts ;
                              rdfs:comment "Different classification databases may use different types of Classification Families and have different names for the families, as no standard has been agreed upon."@en ;
                              rdfs:isDefinedBy "A Classification Family is a group of Classification Series related from a particular point of view. The Classification Family is related by being based on a common Concept (e.g. economic activity)."@en .


###  https://w3id.org/italia/onto/gsim-sum#ClassificationIndex
gsim-sum:ClassificationIndex rdf:type owl:Class ;
                             rdfs:subClassOf gsim-sum:Concepts ;
                             rdfs:comment """A Classification Index shows the relationship between text found in statistical data sources (responses to survey questionnaires, administrative records) and one or more Statistical Classifications. A Classification Index may be used to assign the codes for Classification Items to observations in statistical collections.
A Statistical Classification is a subtype of Node Set. The relationship between Statistical Classification and Classification Index can also be extended to include the other Node Set types - Code List and Category Set."""@en ;
                             rdfs:isDefinedBy "A Classification Index is an ordered list (alphabetical, in code order etc.) of Classification Index Entries. A Classification Index can relate to one particular or to several Statistical Classifications."@en .


###  https://w3id.org/italia/onto/gsim-sum#ClassificationIndexEntry
gsim-sum:ClassificationIndexEntry rdf:type owl:Class ;
                                  rdfs:subClassOf gsim-sum:Concepts ;
                                  rdfs:comment "A Classification Item is a subtype of Node. The relationship between Classification Item and Classification Index Entry can also be extended to include the other Node types - Code Item and Category Item."@en ;
                                  rdfs:isDefinedBy "A Classification Index Entry is a word or a short text (e.g. the name of a locality, an economic activity or an occupational title) describing a type of object/unit or object property to which a Classification Item applies, together with the code of the corresponding Classification Item. Each Classification Index Entry typically refers to one item of the Statistical Classification. Although a Classification Index Entry may be associated with a Classification Item at any Level of a Statistical Classification, Classification Index Entries are normally associated with items at the lowest Level."@en .


###  https://w3id.org/italia/onto/gsim-sum#ClassificationItem
gsim-sum:ClassificationItem rdf:type owl:Class ;
                            rdfs:subClassOf gsim-sum:Node ;
                            rdfs:isDefinedBy "A Classification Item represents a Category at a certain Level within a Statistical Classification. It defines the content and the borders of the Category. A Unit can be classified to one and only one item at each Level of a Statistical Classification."@en .


###  https://w3id.org/italia/onto/gsim-sum#ClassificationSeries
gsim-sum:ClassificationSeries rdf:type owl:Class ;
                              rdfs:subClassOf gsim-sum:Concept ;
                              rdfs:isDefinedBy "A Classification Series is an ensemble of one or more Statistical Classifications, based on the same concept, and related to each other as versions or updates. Typically, these Statistical Classifications have the same name (for example, ISIC or ISCO)."@en .


###  https://w3id.org/italia/onto/gsim-sum#Code
gsim-sum:Code rdf:type owl:Class ;
              rdfs:subClassOf gsim-sum:Designation ;
              rdfs:comment "Codes are unique within their Code List. Example: M (Male), F (Female). "@en ;
              rdfs:isDefinedBy "A Designation for a Category."@en .


###  https://w3id.org/italia/onto/gsim-sum#CodeItem
gsim-sum:CodeItem rdf:type owl:Class ;
                  rdfs:subClassOf gsim-sum:Node ;
                  rdfs:comment "A type of Node particular to a Code List type of Node Set. A Code Item combines the meaning of the included Category with a Code representation."@en ;
                  rdfs:isDefinedBy "An element of a Code List."@en .


###  https://w3id.org/italia/onto/gsim-sum#CodeList
gsim-sum:CodeList rdf:type owl:Class ;
                  rdfs:subClassOf gsim-sum:NodeSet ;
                  rdfs:comment "A kind of Node Set for which the Category contained in each Node has a Code assigned as a Designation. For example: 1 - Male 2 - Female"@en ;
                  rdfs:isDefinedBy "A list of Categories where each Category has a predefined Code assigned to it."@en .


###  https://w3id.org/italia/onto/gsim-sum#Concept
gsim-sum:Concept rdf:type owl:Class ;
                 rdfs:subClassOf gsim-sum:Concepts ;
                 rdfs:isDefinedBy "Unit of thought differentiated by characteristics"@en .


###  https://w3id.org/italia/onto/gsim-sum#ConceptSystem
gsim-sum:ConceptSystem rdf:type owl:Class ;
                       rdfs:subClassOf gsim-sum:Concepts ;
                       rdfs:comment "Here are 2 examples 1) Concept of Sex: Male, Female, Other 2) ISIC (the list is too long to write down)."@en ;
                       rdfs:isDefinedBy "Set of Concepts structured by the relations among them."@en .


###  https://w3id.org/italia/onto/gsim-sum#Concepts
gsim-sum:Concepts rdf:type owl:Class ;
                  rdfs:subClassOf gsim-sum:IdentifiableArtefact .


###  https://w3id.org/italia/onto/gsim-sum#ConceptualDomain
gsim-sum:ConceptualDomain rdf:type owl:Class ;
                          rdfs:subClassOf gsim-sum:Concepts ;
                          rdfs:comment "The Concepts can be described by either enumeration or by an expression."@en ;
                          rdfs:isDefinedBy "Set of valid Concepts."@en .


###  https://w3id.org/italia/onto/gsim-sum#CorrespondenceTable
gsim-sum:CorrespondenceTable rdf:type owl:Class ;
                             rdfs:subClassOf gsim-sum:Concepts ;
                             rdfs:comment "A Statistical Classification is a subtype of Node Set. The relationship between Statistical Classification and Correspondence Table can also be extended to include the other Node Sets - Code List and Category Set."@en ;
                             rdfs:isDefinedBy "A Correspondence Table expresses the relationship between two Statistical Classifications. These are typically: two versions from the same Classification Series; Statistical Classifications from different Classification Series; a variant and the version on which it is based; or, different versions of a variant. In the first and last examples, the Correspondence Table facilitates comparability over time. Correspondence relationships are shown in both directions"@en .


###  https://w3id.org/italia/onto/gsim-sum#DataPoint
gsim-sum:DataPoint rdf:type owl:Class ;
                   rdfs:subClassOf gsim-sum:Structures ;
                   rdfs:comment "Field in a Data Structure which corresponds to a cell in a table. The Data Point is structural and distinct from the value (the Datum) that it holds."@en ;
                   rdfs:isDefinedBy "A placeholder (or cell) for the value of an Instance Variable."@en .


###  https://w3id.org/italia/onto/gsim-sum#DataResource
gsim-sum:DataResource rdf:type owl:Class ;
                      rdfs:subClassOf gsim-sum:InformationResource ;
                      rdfs:comment "Data Resources are collections of data that are used by a statistical activity to produce information. Data Resource is a specialization of an Information Resource."@en ;
                      rdfs:isDefinedBy "An organized collection of stored information made of one or more Data Sets."@en .


###  https://w3id.org/italia/onto/gsim-sum#DataSet
gsim-sum:DataSet rdf:type owl:Class ;
                 rdfs:subClassOf gsim-sum:InformationSet ;
                 rdfs:comment "Examples of Data Sets could be observation registers, time series, longitudinal data, survey data, rectangular data sets, event-history data, tables, data tables, cubes, registers, hypercubes, and matrixes. A broader term for Data Set could be data. A narrower term for Data Set could be data element, data record, cell, field."@en ;
                 rdfs:isDefinedBy "An organized collection of data."@en .


###  https://w3id.org/italia/onto/gsim-sum#DataStructure
gsim-sum:DataStructure rdf:type owl:Class ;
                       rdfs:subClassOf gsim-sum:Structures ;
                       rdfs:comment "The structure is described using Data Structure Components that can be either Attribute Components, Identifier Components or Measure Components. Examples for unit data include social security number, country of residence, age, citizenship, country of birth, where the social security number and the country of residence are both identifying components and the others are measured variables obtained directly or indirectly from the person (Unit)."@en ;
                       rdfs:isDefinedBy "Defines the structure of an organized collection of data (Data Set)."@en .


###  https://w3id.org/italia/onto/gsim-sum#DataStructureComponent
gsim-sum:DataStructureComponent rdf:type owl:Class ;
                                rdfs:subClassOf gsim-sum:Structures ;
                                rdfs:comment "A Data Structure Component can be an Attribute Component, Measure Component or an Identifier Component. Example of Attribute Component: The publication status of an observation such as provisional, revised. Example of Measure Component: age and height of a person in a Unit Data Set or number of citizens and number of households in a country in a Data Set for multiple countries (Dimensional Data Set). Example of Identifier Component: The personal identification number of a Swedish citizen for unit data or the name of a country in the European Union for dimensional data."@en ;
                                rdfs:isDefinedBy "The role of the Represented Variable in the context of a Data Structure."@en .


###  https://w3id.org/italia/onto/gsim-sum#Datum
gsim-sum:Datum rdf:type owl:Class ;
               rdfs:subClassOf gsim-sum:StatisticalGenericInformationModel ;
               rdfs:comment "A Datum is the actual instance of data that was collected or derived. It is the value which populates a Data Point. A Datum is the value found in a cell of a table."@en ;
               rdfs:isDefinedBy "A value."@en .


###  https://w3id.org/italia/onto/gsim-sum#DescribedConceptualDomain
gsim-sum:DescribedConceptualDomain rdf:type owl:Class ;
                                   rdfs:subClassOf gsim-sum:ConceptualDomain ;
                                   rdfs:comment "For example: All real numbers between 0 and 1."@en ;
                                   rdfs:isDefinedBy "A Conceptual Domain defined by an expression." .


###  https://w3id.org/italia/onto/gsim-sum#DescribedValueDomain
gsim-sum:DescribedValueDomain rdf:type owl:Class ;
                              rdfs:subClassOf gsim-sum:ValueDomain ;
                              rdfs:comment "For example: All real decimal numbers between 0 and 1."@en ;
                              rdfs:isDefinedBy "A Value Domain defined by an expression."@en .


###  https://w3id.org/italia/onto/gsim-sum#Designation
gsim-sum:Designation rdf:type owl:Class ;
                     rdfs:subClassOf gsim-sum:Concepts ;
                     rdfs:comment "The association of a Concept with a Sign that denotes it."@en ;
                     rdfs:isDefinedBy "The name given to an object for identification." .


###  https://w3id.org/italia/onto/gsim-sum#DimensionalDataStructure
gsim-sum:DimensionalDataStructure rdf:type owl:Class ;
                                  rdfs:subClassOf gsim-sum:DataStructure ;
                                  rdfs:comment "For example (city, average income, total population) where the city is the Identifier Component and the others are measured variables."@en ;
                                  rdfs:isDefinedBy "Describes the structure of a Dimensional Data Set."@en .


###  https://w3id.org/italia/onto/gsim-sum#EnumeratedConceptualDomain
gsim-sum:EnumeratedConceptualDomain rdf:type owl:Class ;
                                    rdfs:subClassOf gsim-sum:ConceptualDomain ;
                                    rdfs:comment "For instance the Sex Categories: 'Male' and 'Female'."@en ;
                                    rdfs:isDefinedBy "A Conceptual Domain expressed as a list of Categories."@en .


###  https://w3id.org/italia/onto/gsim-sum#EnumeratedValueDomain
gsim-sum:EnumeratedValueDomain rdf:type owl:Class ;
                               rdfs:subClassOf gsim-sum:ValueDomain ;
                               rdfs:comment "Example -  Sex Codes: <m, male>, <f, female>, <o, others>."@en ;
                               rdfs:isDefinedBy "A Value Domain expressed as a list of Categories and associated Codes."@en .


###  https://w3id.org/italia/onto/gsim-sum#EnvironmentChange
gsim-sum:EnvironmentChange rdf:type owl:Class ;
                           rdfs:subClassOf gsim-sum:StatisticalNeed ;
                           rdfs:comment "An Environment Change reflects change in the context in which a statistical organization operates. Environment Changes can be of different origins and also take different forms. They can result from a precise event (budget cut, new legislation enforced) or from a progressive process (technical or methodological progress, application or tool obsolescence). Other examples of Environment Changes include the availability of a new Information Resource, the opportunity for new collaboration between organizations, etc."@en ;
                           rdfs:isDefinedBy "A requirement for change that originates from a change in the operating environment of the statistical organization."@en .


###  https://w3id.org/italia/onto/gsim-sum#Exchange
gsim-sum:Exchange rdf:type owl:Class ;
                  rdfs:subClassOf gsim-sum:IdentifiableArtefact .


###  https://w3id.org/italia/onto/gsim-sum#IdentifiableArtefact
gsim-sum:IdentifiableArtefact rdf:type owl:Class ;
                              rdfs:subClassOf gsim-sum:StatisticalGenericInformationModel ;
                              rdfs:comment "An instance of any GSIM information object is an Identifiable Artefact."@en ;
                              rdfs:isDefinedBy "An abstract class that comprises the basic attributes and associations needed for identification, naming and other documentation."@en .


###  https://w3id.org/italia/onto/gsim-sum#IdentifierComponent
gsim-sum:IdentifierComponent rdf:type owl:Class ;
                             rdfs:subClassOf gsim-sum:DataStructureComponent ;
                             rdfs:comment "An Identifier Component is a sub-type of a data structure Component. The personal identification number of a Swedish citizen for unit data or the name of a country in the European Union for dimensional data."@en ;
                             rdfs:isDefinedBy "The role given to a Represented Variable in the context of a Data Structure to identify the unit in an organized collection of data."@en .


###  https://w3id.org/italia/onto/gsim-sum#InformationRequest
gsim-sum:InformationRequest rdf:type owl:Class ;
                            rdfs:subClassOf gsim-sum:StatisticalNeed ;
                            rdfs:comment "An Information Request is a special case of Statistical Need that may come in an organized form, for example by specifying on which Subject Field the information is required. It may also be a more general request and require refinement by the statistical agency and formalized in a Change Definition."@en ;
                            rdfs:isDefinedBy "An outline of a need for new information required for a particular purpose."@en .


###  https://w3id.org/italia/onto/gsim-sum#InformationResource
gsim-sum:InformationResource rdf:type owl:Class ;
                             rdfs:subClassOf gsim-sum:Structures ;
                             rdfs:comment "There currently are only two concrete sub classes: Data Resource and Referential Metadata Resource. The Information Resource allows the model to be extended to other types of resource."@en ;
                             rdfs:isDefinedBy "An abstract notion that is any organized collection of information."@en .


###  https://w3id.org/italia/onto/gsim-sum#InformationSet
gsim-sum:InformationSet rdf:type owl:Class ;
                        rdfs:subClassOf gsim-sum:Structures ;
                        rdfs:comment "Statistical organizations collect, process, analyze and disseminate Information Sets, which contain data (Data Sets), referential metadata (Referential Metadata Sets), or potentially other types of statistical content, which could be included in addition types of Information Set."@en ;
                        rdfs:isDefinedBy "Organized collections of statistical content."@en .


###  https://w3id.org/italia/onto/gsim-sum#InstanceQuestion
gsim-sum:InstanceQuestion rdf:type owl:Class ;
                          rdfs:subClassOf gsim-sum:Exchange ;
                          rdfs:comment "The Instance Question is the use of a Question in a particular Questionnaire Component. This also includes the use of the Question in a Question Block, which is a particular type of Questionnaire Component."@en ;
                          rdfs:isDefinedBy "The use of a Question in a particular Questionnaire."@en .


###  https://w3id.org/italia/onto/gsim-sum#InstanceQuestionBlock
gsim-sum:InstanceQuestionBlock rdf:type owl:Class ;
                               rdfs:subClassOf gsim-sum:Exchange ;
                               rdfs:comment "The Instance Question Block is the use of a Question Block in a particular Questionnaire Component. This also includes the use of a Question Block in another Question Block, as it is a particular type of Questionnaire Component."@en ;
                               rdfs:isDefinedBy "The use of a Question Block in a particular Questionnaire. "@en .


###  https://w3id.org/italia/onto/gsim-sum#InstanceStatement
gsim-sum:InstanceStatement rdf:type owl:Class ;
                           rdfs:subClassOf gsim-sum:Exchange ;
                           rdfs:comment "The Instance Statement is the use of a Statement in a particular Questionnaire Component. This also includes the use of the Statement in a Question Block, which is a particular type of Questionnaire Component."@en ;
                           rdfs:isDefinedBy "The use of a Statement in a particular Questionnaire."@en .


###  https://w3id.org/italia/onto/gsim-sum#InstanceVariable
gsim-sum:InstanceVariable rdf:type owl:Class ;
                          rdfs:subClassOf gsim-sum:Concept ;
                          rdfs:comment "The Instance Variable is used to describe actual instances of data that have been collected. Here are three examples: 1- Gender: Dan Gillman has gender <m, male>, Arofan Gregory has gender<m, male>, etc.; 2- Number of employees: Microsoft has 90,000 employees; IBM has 433,000 employees, etc.; 3 -  Endowment: Johns Hopkins has endowment of <3, 1,000,000$ and above>, Yale has endowment of <3, 1,000,000$ and above>."@en ;
                          rdfs:isDefinedBy "The use of a Represented Variable within a Data Set. It may include information about the source of the data."@en .


###  https://w3id.org/italia/onto/gsim-sum#Level
gsim-sum:Level rdf:type owl:Class ;
               rdfs:subClassOf gsim-sum:Concepts ;
               rdfs:comment "A Statistical Classification is a subtype of Node Set. The relationship between Statistical Classification and Level can also be extended to include the other Node Set types - Code List and Category Set."@en ;
               rdfs:isDefinedBy "A Statistical Classification has a structure which is composed of one or several Levels. A Level often is associated with a Concept, which defines it. In a hierarchical classification the Classification Items of each Level but the highest are aggregated to the nearest higher Level. A linear classification has only one Level."@en .


###  https://w3id.org/italia/onto/gsim-sum#LogicalRecord
gsim-sum:LogicalRecord rdf:type owl:Class ;
                       rdfs:subClassOf gsim-sum:Structures ;
                       rdfs:comment "Examples: household, person or dwelling record."@en ;
                       rdfs:isDefinedBy "Describes a type of Unit Data Record for one Unit Type within a Unit Data Set."@en .


###  https://w3id.org/italia/onto/gsim-sum#Map
gsim-sum:Map rdf:type owl:Class ;
             rdfs:subClassOf gsim-sum:Concepts ;
             rdfs:comment "The use of Correspondence Tables and Maps can be extended to include all types of Node and Node Set. This means that a Correspondence Table could map between the items of Statistical Classifications, Code Lists or Category Sets."@en ;
             rdfs:isDefinedBy "A Map is an expression of the relation between a Classification Item in a source Statistical Classification and a corresponding Classification Item in the target Statistical Classification. The Map should specify whether the relationship between the two Classification Items is partial or complete. Depending on the relationship type of the Correspondence Table, there may be several Maps for a single source or target item."@en .


###  https://w3id.org/italia/onto/gsim-sum#MeasureComponent
gsim-sum:MeasureComponent rdf:type owl:Class ;
                          rdfs:subClassOf gsim-sum:DataStructureComponent ;
                          rdfs:comment "A Measure Component is a sub-type of Data Structure Component. For example age and height of a person in a Unit Data Set or number of citizens and number of households in a country in a Data Set for multiple countries (Dimensional Data Set)."@en ;
                          rdfs:isDefinedBy "The role given to a Represented Variable in the context of a Data Structure to hold the observed/derived values for a particular Unit in an organized collection of data."@en .


###  https://w3id.org/italia/onto/gsim-sum#Node
gsim-sum:Node rdf:type owl:Class ;
              rdfs:subClassOf gsim-sum:Concepts ;
              rdfs:comment "A Node is created as a Category, Code or Classification Item for the purpose of defining the situation in which the Category is being used."@en ;
              rdfs:isDefinedBy "A combination of a Category and related attributes."@en .


###  https://w3id.org/italia/onto/gsim-sum#NodeSet
gsim-sum:NodeSet rdf:type owl:Class ;
                 rdfs:subClassOf gsim-sum:Concepts ;
                 rdfs:comment "Node Set is a kind of Concept System. Here are 2 examples: 1 - Sex Categories:  Male,  Female, Other; Sex Codes: <m, male>, <f, female>, <o, other> "@en ;
                 rdfs:isDefinedBy "A set of Nodes."@en .


###  https://w3id.org/italia/onto/gsim-sum#OutputSpecification
gsim-sum:OutputSpecification rdf:type owl:Class ;
                             rdfs:subClassOf gsim-sum:Exchange ;
                             rdfs:comment "The Output Specification specifies Products and defines the Presentations they contain. The Output Specification may be fully defined during the design process (such as in a paper publication or a predefined web report), or may be a combination of designed specification supplemented by user selections (such as in an online data query tool)."@en ;
                             rdfs:isDefinedBy "Defines how Information Sets consumed by a Product are presented to Information Consumers."@en .


###  https://w3id.org/italia/onto/gsim-sum#Population
gsim-sum:Population rdf:type owl:Class ;
                    rdfs:subClassOf gsim-sum:Concept ;
                    rdfs:comment "A Population is used to describe the total membership of a group of people, objects or events based on characteristics, e.g. time and geographic boundaries. Hera are three examples: 1. US adult persons on 13 November 1956; 2. US computer companies at the end of 2012; 3. Universities in the  US 1 January 2011."@en ;
                    rdfs:isDefinedBy "The total membership of a defined class of people, objects or events."@en .


###  https://w3id.org/italia/onto/gsim-sum#Presentation
gsim-sum:Presentation rdf:type owl:Class ;
                      rdfs:subClassOf gsim-sum:Exchange ;
                      rdfs:comment """A Product has one or more Presentations, which present data and referential metadata from Information Sets. A Presentation is defined by an Output Specification. Presentation can be in different forms; e.g. tables, graphs, structured data files. Examples:
- A table of data. Based on a Data Set, the related Data Structure is used to label the column and row headings for the table. The Data Set is used to populate the cells in the table. Reference metadata is used to populate footnotes and cell notes on the table. Confidentiality rules are applied to the Data Set to suppress any disclosive cells.
- A data file based on a standard (e.g. SDMX).
- A PDF document describing a Classification.
- Any structural metadata object expressed in a standard format (e.g. DDI 3.1 XML).
- A list of Products or services (e.g. a product catalogue or a web services description language (WSDL) file).
- A web page containing Classifications, descriptions of Variables, etc."""@en ;
                      rdfs:isDefinedBy "The way data and referential metadata are presented in a Product. "@en .


###  https://w3id.org/italia/onto/gsim-sum#ProcessControl
gsim-sum:ProcessControl rdf:type owl:Class ;
                        rdfs:subClassOf gsim-sum:Business ;
                        rdfs:comment "The typical use of Process Control is to determine what happens next after a Process Step is executed. The possible paths, and the decision criteria, associated with a Process Control are specified as part of designing a production process, captured in a Process Control Design. There is typically a very close relationship between the design of a process and the design of a Process Control."@en ;
                        rdfs:isDefinedBy "A set of decision points which determine the flow between the Process Steps used to perform a Business Process."@en .


###  https://w3id.org/italia/onto/gsim-sum#ProcessControlDesign
gsim-sum:ProcessControlDesign rdf:type owl:Class ;
                              rdfs:subClassOf gsim-sum:Business ;
                              rdfs:comment "The design of a Process Control typically takes place as part of the design of the process itself. This involves determining the conditional routing between the various sub-processes and services used by the executing process associated with the Process Control and specified by the Process Control Design. It is possible to define a Process Control where the next step in the Process Step that will be executed is a fixed value rather than a \"choice\" between two or more possibilities. Where such a design would be appropriate, this feature allows, for example, initiation of a step in the Process Step representing the GSBPM Process Phase (5) to always lead to initiation of GSBPM sub-process Integrate Data (5.1) as the next step. This allows a process designer to divide a Business Process into logical steps (for example, where each step performs a specific Business Function through re-use of a Business Service) even if these process steps will always follow each other in the same order. In all cases, the Process Control Design defines and the Process Control manages the flow between Process Steps, even where the flow is \"trivial\". Process Design is left to focus entirely on the design of the process itself, not sequencing between steps."@en ;
                              rdfs:isDefinedBy "The specification of the decision points required during the execution of a Business Process."@en .


###  https://w3id.org/italia/onto/gsim-sum#ProcessDesign
gsim-sum:ProcessDesign rdf:type owl:Class ;
                       rdfs:subClassOf gsim-sum:Business ;
                       rdfs:comment "A Process Design is the design time specification of a Process Step that is performed as part of a run-time Business Service. A Process Step can be as big or small as the designer of a particular Business Service chooses. From a design perspective, one Process Step can contain \"sub-steps\", each of which is conceptualized as a (smaller) Process Step in its own right. Each of those \"sub-steps\" may contain \"sub-steps\" within them and so on indefinitely. It is a decision for the process designer to what extent to subdivide steps. At some level it will be appropriate to consider a Process Step to be a discrete task (unit of work) without warranting further subdivision. At that level the Process Step is designed to process particular Process Inputs, according to a particular Process Method, to produce particular Process Outputs. The flow between a Process Step and any sub steps is managed via Process Control."@en ;
                       rdfs:isDefinedBy "The specification of how a Process Step will be performed. This includes specifying the types of Process Inputs required and the type of Process Outputs that will be produced."@en .


###  https://w3id.org/italia/onto/gsim-sum#ProcessInput
gsim-sum:ProcessInput rdf:type owl:Class ;
                      rdfs:subClassOf gsim-sum:Business ;
                      rdfs:comment "Process Input might include information that is used as an input that will be transformed (e.g. a Data Set), information that is used to control specific parameters of the process (e.g. a Rule), and information that is used as reference to guide the process (e.g. a Code List)."@en ;
                      rdfs:isDefinedBy "Any instance of an information object which is supplied to a Process Step Instance at the time its execution is initiated."@en .


###  https://w3id.org/italia/onto/gsim-sum#ProcessInputSpecification
gsim-sum:ProcessInputSpecification rdf:type owl:Class ;
                                   rdfs:subClassOf gsim-sum:Business ;
                                   rdfs:comment "The Process Input Specification enumerates the Process Inputs required at the time a Process Design is executed. For example, if five different Process Inputs are required, the Process Input Specification will describe each of the five inputs. For each required Process Input the Process Input Specification will record the type of information object (based on GSIM) which will be used as the Process Input (example types might be a Dimensional Data Set or a Classification). The Process Input to be provided at the time of Process Step execution will then be a specific instance of the type of information object specified by the Process Input Specification. For example, if a Process Input Specification requires a Dimensional Data Set then the corresponding Process Input provided at the time of Process Step execution will be a particular Dimensional Data Set."@en ;
                                   rdfs:isDefinedBy "A record of the types of inputs required for a Process Design."@en .


###  https://w3id.org/italia/onto/gsim-sum#ProcessMethod
gsim-sum:ProcessMethod rdf:type owl:Class ;
                       rdfs:subClassOf gsim-sum:Business ;
                       rdfs:comment "The technique specified by a Process Method is independent from any choice of technologies and/or other tools which will be used to apply that technique in a particular instance. The definition of the technique may, however, intrinsically require the application of specific Rules (for example, mathematical or logical formulas). A Process Method describes a particular method for performing a Process Step."@en ;
                       rdfs:isDefinedBy "A specification of the technique which will be used to perform the unit of work."@en .


###  https://w3id.org/italia/onto/gsim-sum#ProcessOutput
gsim-sum:ProcessOutput rdf:type owl:Class ;
                       rdfs:subClassOf gsim-sum:Business ;
                       rdfs:comment "Process Outputs have an attribute of Process Output Type, which has two possible values: - Transformed Output is the result which provides the \"reason for existence\" of the Process Step. If that output were no longer required then there would be no need for the Process Step in its current form. Typically a Transformed Output is either a Process Input to a subsequent Process Step or it represents the final product from a statistical business process; - A Process Metric records information about the execution of a Process Step. For example, how long it took to complete execution of the Process Step and what percentage of records in the Process Input was updated by the Process Step to produce the Transformed Output."@en ;
                       rdfs:isDefinedBy "Any instance of an information object which is produced by a Process Step as a result of its execution."@en .


###  https://w3id.org/italia/onto/gsim-sum#ProcessOutputSpecification
gsim-sum:ProcessOutputSpecification rdf:type owl:Class ;
                                    rdfs:subClassOf gsim-sum:Business ;
                                    rdfs:comment "The Process Output Specification enumerates the Process Outputs that are expected to be produced at the time a Process Design is executed. For example, if five different Process Outputs expected, the Process Output Specification will describe each of the five outputs. For each expected Process Output the Process Output Specification will record the type of information object (based on GSIM) which will be used as the Process Output (Example types might be a Dimensional Data Set or a Classification). The Process Output to be provided at the time of Process Step execution will then be a specific instance of the type of information object specified by the Process Output Specification. For example, if a Process Output Specification expects a Dimensional Data Set then the corresponding Process Output provided at the time of Process Step execution will be a particular Dimensional Data Set."@en ;
                                    rdfs:isDefinedBy "A record of the types of outputs required for a Process Design."@en .


###  https://w3id.org/italia/onto/gsim-sum#ProcessPattern
gsim-sum:ProcessPattern rdf:type owl:Class ;
                        rdfs:subClassOf gsim-sum:Business ;
                        rdfs:comment "In a particular Business Process, some Process Steps may be unique to that Business Process while others may be applicable to other Business Processes. A Process Pattern can be seen as a reusable template. It is a means to accelerate design processes and to achieve sharing and reuse of design patterns which have proved effective. Reuse of Process Patterns can indicate the possibility to reuse related Business Services. By deciding to reuse a Process Pattern, a designer is actually reusing the pattern of Process Designs and Process Control Designs associated with that Process Pattern. They will receive a new instance of the Process Designs and Process Control Designs. If they then tailor their \"instance\" of the Process Designs and Process Control Designs to better meet their needs they will not change the definition of the reusable Process Pattern."@en ;
                        rdfs:isDefinedBy "A nominated set of Process Designs, and associated Process Control Designs (flow), which have been highlighted for possible reuse."@en .


###  https://w3id.org/italia/onto/gsim-sum#ProcessStep
gsim-sum:ProcessStep rdf:type owl:Class ;
                     rdfs:subClassOf gsim-sum:Business ;
                     rdfs:comment "Each Process Step is the use of a Process Step Design in a particular context (e.g. within a specific Business Process). At the time of execution a Process Step Instance specifies the actual instances of input objects (for example, specific Data Sets, specific Variables) to be supplied."@en ;
                     rdfs:isDefinedBy """A Process Step is a work package that performs a Business Process. A Process Step implements the Process Step Design specified in order to produce the outputs for which the Process Step was designed.
A Process Step can only exist in either the context of a Business Service OR a Business Process, NOT BOTH."""@en .


###  https://w3id.org/italia/onto/gsim-sum#ProcessStepInstance
gsim-sum:ProcessStepInstance rdf:type owl:Class ;
                             rdfs:subClassOf gsim-sum:Business ;
                             rdfs:comment "Each Process Step is the use of a Process Step Design in a particular context (e.g. within a specific Business Process). At the time of execution a Process Step Instance specifies the actual instances of input objects (for example, specific Data Sets, specific Variables) to be supplied. Each Process Step Instance may produce unique results even though the Process Step remains constant. Even when the inputs remain the same, metrics such as the elapsed time to complete execution of process step may vary from execution to execution. For this reason, each Process Step Instance details of inputs and outputs for that instance of implementing the Process Step. In this way it is possible to trace the flow of execution of a Business Process through all the Process Steps which were involved."@en ;
                             rdfs:isDefinedBy "An executed step in a Business Process. A Process Step Instance specifies the actual inputs to and outputs from for an occurrence of a Process Step."@en .


###  https://w3id.org/italia/onto/gsim-sum#ProvisionAgreement
gsim-sum:ProvisionAgreement rdf:type owl:Class ;
                            rdfs:subClassOf gsim-sum:Exchange ;
                            rdfs:comment "The legal or other basis by which two parties agree to exchange data."@en .


###  https://w3id.org/italia/onto/gsim-sum#Question
gsim-sum:Question rdf:type owl:Class ;
                  rdfs:subClassOf gsim-sum:Exchange ;
                  rdfs:comment "Describes the text used to elicit a response for the Concept to be measured. A Question may be a single question used to obtain a response, or may be a multiple question, a construct which links multiple sub-questions, each with their own response."@en .


###  https://w3id.org/italia/onto/gsim-sum#QuestionnaireComponent
gsim-sum:QuestionnaireComponent rdf:type owl:Class ;
                                rdfs:subClassOf gsim-sum:Exchange ;
                                rdfs:comment """Defines the structure of the Questionnaire Specification, as a combination of Questions, Question Blocks and Statements. It is the object which groups together all the components of a Questionnaire.
A Questionnaire Component is recursive, in that it can refer to other Questionnaire Components and accompanying Questionnaire Logic objects at a lower level. It is only at the top level where the Questionnaire Component links to the Questionnaire Specification."""@en ;
                                rdfs:isDefinedBy "A record of the flow of a Questionnaire Specification and its use of Questions, Question Blocks and Statements. "@en .


###  https://w3id.org/italia/onto/gsim-sum#QuestionnaireLogic
gsim-sum:QuestionnaireLogic rdf:type owl:Class ;
                            rdfs:subClassOf gsim-sum:Exchange ;
                            rdfs:isDefinedBy "Governs the sequence of Questions, Question Blocks and Statements based on factors such as the current location, the response to the previous questions etc., invoking navigation and validation rules to apply."@en .


###  https://w3id.org/italia/onto/gsim-sum#QuestionnaireSpecification
gsim-sum:QuestionnaireSpecification rdf:type owl:Class ;
                                    rdfs:subClassOf gsim-sum:Exchange ;
                                    rdfs:comment """This represents the complete questionnaire design, with a relationship to the top level Questionnaire Component.
There may be many different Questionnaire Specifications, for the same surveys, or tailored to individual observation Units (respondents) so that there would be a different Questionnaire Specification for each respondent. The design would also differ depending upon the specific mode of collection the Questionnaire is designed for."""@en ;
                                    rdfs:isDefinedBy "The tool designed to elicit information from observation Units."@en .


###  https://w3id.org/italia/onto/gsim-sum#RecordRelationship
gsim-sum:RecordRelationship rdf:type owl:Class ;
                            rdfs:subClassOf gsim-sum:Structures ;
                            rdfs:comment "Example: Relationship between person and household Logical Records within a Unit Data Set."@en ;
                            rdfs:isDefinedBy "Describes relationships between Logical Records within a Unit Data Structure. It must have both a source Logical Record and a target Logical Record in order to define the relationship."@en .


###  https://w3id.org/italia/onto/gsim-sum#ReferentialMetadataAttribute
gsim-sum:ReferentialMetadataAttribute rdf:type owl:Class ;
                                      rdfs:subClassOf gsim-sum:Structures ;
                                      rdfs:isDefinedBy "The role given to a Represented Variable to supply information in the context of a Referential Metadata Structure."@en .


###  https://w3id.org/italia/onto/gsim-sum#ReferentialMetadataContentItem
gsim-sum:ReferentialMetadataContentItem rdf:type owl:Class ;
                                        rdfs:subClassOf gsim-sum:Structures ;
                                        rdfs:comment "A Referential Metadata Content Item contains the actual content describing a particular characteristic of a Referential Metadata Subject."@en ;
                                        rdfs:isDefinedBy "The content describing a particular characteristic of a Referential Metadata Subject."@en .


###  https://w3id.org/italia/onto/gsim-sum#ReferentialMetadataResource
gsim-sum:ReferentialMetadataResource rdf:type owl:Class ;
                                     rdfs:subClassOf gsim-sum:InformationResource ;
                                     rdfs:comment "Referential Metadata Resources are collections of structured information that may be used by a statistical activity to produce information. This information object is a specialization of an Information Resource."@en ;
                                     rdfs:isDefinedBy "An organized collection of stored information consisting of one or more Referential Metadata Sets."@en .


###  https://w3id.org/italia/onto/gsim-sum#ReferentialMetadataStructure
gsim-sum:ReferentialMetadataStructure rdf:type owl:Class ;
                                      rdfs:subClassOf gsim-sum:Structures ;
                                      rdfs:comment """A Referential Metadata Structure defines a structured list of Referential Metadata Attributes for a given Referential Metadata Subject.
Examples of Referential Metadata Attributes are those that describe quality information and methodologies. Examples of subject are: objects like a Questionnaire or a Classification, or collections of data like a Data Set, or any Data Point or set of Data Points created from a specific Data Structure."""@en ;
                                      rdfs:isDefinedBy "Defines the structure of an organized collection of referential metadata (Referential Metadata Set)."@en .


###  https://w3id.org/italia/onto/gsim-sum#ReferentialMetadataSubject
gsim-sum:ReferentialMetadataSubject rdf:type owl:Class ;
                                    rdfs:subClassOf gsim-sum:Structures ;
                                    rdfs:comment """The Referential Metadata Subject identifies the subject of the metadata that can be reported using this Referential Metadata Structure. These subjects may be any GSIM object type, or any Data Point or set of Data Points created from a specific Data Structure.
Examples: The GSIM object type may be Product for which there is a list specified in a Value Domain. The Value Domain specifies the list of actual Products for which reference metadata can be reported or authored using this Referential Metadata Structure."""@en ;
                                    rdfs:isDefinedBy "Identifies the subject of an organized collection of referential metadata."@en .


###  https://w3id.org/italia/onto/gsim-sum#ReferentialMetadataSubjectItem
gsim-sum:ReferentialMetadataSubjectItem rdf:type owl:Class ;
                                        rdfs:subClassOf gsim-sum:Structures ;
                                        rdfs:comment "Examples are an actual Product such as Balance of Payments and International Investment Position, Australia, June 2013, or a collection of Data Points such as the Data Points for a single region within a Data Set covering all regions for a country."@en ;
                                        rdfs:isDefinedBy "Identifies the actual subject for which referential metadata is reported."@en .


###  https://w3id.org/italia/onto/gsim-sum#RepresentedVariable
gsim-sum:RepresentedVariable rdf:type owl:Class ;
                             rdfs:subClassOf gsim-sum:Concept ;
                             rdfs:comment "Example: the pair (Number of Employees, Integer), where \"Number of Employees\" is the characteristic of the population (Variable) and \"Integer\" is how that measure will be represented (Value Domain)."@en ;
                             rdfs:isDefinedBy "A combination of a characteristic of a population to be measured and how that measure will be represented."@en .


###  https://w3id.org/italia/onto/gsim-sum#Rule
gsim-sum:Rule rdf:type owl:Class ;
              rdfs:subClassOf gsim-sum:Business ;
              rdfs:comment "Rules are of several types: they may be derived from methods to determine the control flow of a process when it is being designed and executed; they may be used as the input parameters of processes (e.g., imputation rules, edit rules); and they may be used to drive the logical flow of a questionnaire. There are many forms of Rules and their purpose, character and expression can vary greatly."@en ;
              rdfs:isDefinedBy "A specific mathematical or logical expression which can be evaluated to determine specific behavior."@en .


###  https://w3id.org/italia/onto/gsim-sum#Statement
gsim-sum:Statement rdf:type owl:Class ;
                   rdfs:subClassOf gsim-sum:Exchange ;
                   rdfs:comment """Statements are often included to provide further explanation to respondents. Example: \"The following questions are about your health\".
The object is also used to represent completion instructions for the interviewer or respondent.
Statement should be designed with re-use in mind as it can be used in numerous Questionnaires."""@en ;
                   rdfs:isDefinedBy "A report of facts in a Questionnaire. "@en .


###  https://w3id.org/italia/onto/gsim-sum#StatisticalClassification
gsim-sum:StatisticalClassification rdf:type owl:Class ;
                                   rdfs:subClassOf gsim-sum:NodeSet ;
                                   rdfs:comment "The Categories are defined with reference to one or more characteristics of a particular population of units of observation. A Statistical Classification may have a flat, linear structure or may be hierarchically structured, such that all Categories at lower Levels are sub-Categories of Categories at the next Level up. Categories in Statistical Classifications are represented in the information model as Classification Items."@en ;
                                   rdfs:isDefinedBy "A Statistical Classification is a set of Categories which may be assigned to one or more variables registered in statistical surveys or administrative files, and used in the production and dissemination of statistics. The Categories at each Level of the classification structure must be mutually exclusive and jointly exhaustive of all objects/units in the population of interest."@en .


###  https://w3id.org/italia/onto/gsim-sum#StatisticalGenericInformationModel
gsim-sum:StatisticalGenericInformationModel rdf:type owl:Class ;
                                            rdfs:subClassOf prov:Entity .


###  https://w3id.org/italia/onto/gsim-sum#StatisticalNeed
gsim-sum:StatisticalNeed rdf:type owl:Class ;
                         rdfs:subClassOf gsim-sum:Business ;
                         rdfs:comment "The Statistical Need is a proposed or imposed requirement, request or other notification as it has been received by an organization. A Statistical Need is a raw expression of a requirement, and is not necessarily well-defined. A related object - Change Definition - is created when a Statistical Need is analyzed by an organization. Change Definition expresses the raw need in well-defined, structured terms. Once a Statistical Need has been received, the first step is to do the conceptual work to establish what it is we are trying to measure. The final output of this conceptual work is the Change Definition. In some cases, the Statistical Need can result from the Assessment of the quality, efficiency, etc. of an existing process. "@en ;
                         rdfs:isDefinedBy "A requirement, request or other notification that will be considered by an organization. A Statistical Need does not necessarily have structure or format - it is a 'raw' need as received by the organization. A Statistical Need may be of a variety of types including Environmental Change or Information Request."@en .


###  https://w3id.org/italia/onto/gsim-sum#StatisticalProgram
gsim-sum:StatisticalProgram rdf:type owl:Class ;
                            rdfs:subClassOf gsim-sum:Business ;
                            rdfs:comment """The Statistical Program is one of a family of objects that provide the environmental context in which activities to produce statistics within a statistical organization are conducted. Statistical Program is the top level object that describes the purpose and objectives of a set of activities. Statistical Program will usually correspond to an ongoing activity such as a survey or output series. Some examples of Statistical Program are:
 Labour Force Survey - Multipurpose Household Survey - National Accounts - Demography - Overseas Arrivals and Departures
Related to the Statistical Program object there are Statistical Program Design and Statistical Program Cycle objects that hold the detailed information about the design and conduct of the Business Process. In the case of the traditional approach, an organization has received a Statistical Need and produced a Change Definition and an approved Business Case. The Business Case will specify either a change to the design or methodology of an existing Statistical Program, which will result in a new Statistical Program Design; or a change to one or more existing Statistical Programs (for example, to add an additional objective to the Statistical Program); or result in a new Statistical Program being created. This does not include statistical support functions such as metadata management, data management (and other overarching GSBPM processes) and design functions. These activities are conducted as part of Statistical Support Programs."""@en ;
                            rdfs:isDefinedBy "A set of activities, which may be repeated, that describes the purpose and context of a set of Business Process within the context of the relevant Statistical Program Cycles."@en .


###  https://w3id.org/italia/onto/gsim-sum#StatisticalProgramCycle
gsim-sum:StatisticalProgramCycle rdf:type owl:Class ;
                                 rdfs:subClassOf gsim-sum:Business ;
                                 rdfs:comment "A Statistical Program Cycle documents the execution of an iteration of a Statistical Program according to the associated Statistical Program Design for a certain reference period. It identifies the activities that are undertaken as a part of the cycle and the specific resources required and processes used and description of relevant methodological information used in this cycle defined by the Statistical Program Design."@en ;
                                 rdfs:isDefinedBy "A set of activities to investigate characteristics of a given Population for a particular reference period."@en .


###  https://w3id.org/italia/onto/gsim-sum#StatisticalProgramDesign
gsim-sum:StatisticalProgramDesign rdf:type owl:Class ;
                                  rdfs:subClassOf gsim-sum:Business ;
                                  rdfs:comment "The Statistical Program Design is an objects that provide the operational context in which a set of Business Processes is conducted. A simple example is where a Statistical Program relates to a single survey, for example, the Labour Force Survey. The Statistical Program will have a series of Statistical Program Design objects that describe the methodology and design used throughout the life of the survey. When a methodological change is made to the survey, a new Statistical Program Design is created to record the details of the new design."@en ;
                                  rdfs:isDefinedBy "The specification of the resources required, processes used and description of relevant methodological information about the set of activities undertaken to investigate characteristics of a given Population."@en .


###  https://w3id.org/italia/onto/gsim-sum#StatisticalSupportActivity
gsim-sum:StatisticalSupportActivity rdf:type owl:Class ;
                                    rdfs:subClassOf gsim-sum:Business ;
                                    rdfs:comment "This type of activity will include such functions as metadata management, data management, methodological research, and design functions. These activities correspond to the overarching processes in the GSBPM, and Corporate Support in GAMSO, as well as activities to create new or change existing Statistical Programmes which are covered by GSBPM phase 1-3, thus creating or updating Statistical Programme Designs."@en ;
                                    rdfs:isDefinedBy "activity that supports statistical production"@en .


###  https://w3id.org/italia/onto/gsim-sum#Structures
gsim-sum:Structures rdf:type owl:Class ;
                    rdfs:subClassOf gsim-sum:IdentifiableArtefact .


###  https://w3id.org/italia/onto/gsim-sum#SubjectField
gsim-sum:SubjectField rdf:type owl:Class ;
                      rdfs:subClassOf gsim-sum:Concepts ;
                      rdfs:comment "A Subject Field is a field of special knowledge under which a set of Concepts and their Designations is used. For example, labour market, environmental expenditure, tourism, etc."@en ;
                      rdfs:isDefinedBy "One or more Concept Systems used for the grouping of Concepts and Categories for the production of statistics."@en .


###  https://w3id.org/italia/onto/gsim-sum#Unit
gsim-sum:Unit rdf:type owl:Class ;
              rdfs:subClassOf gsim-sum:Concepts ;
              rdfs:comment "Here are 3 examples - 1. Individual US person (i.e., Arofan Gregory, Dan Gillman, Barack Obama, etc.) 2. Individual US computer companies (i.e., Microsoft, Apple, IBM, etc.) 3. Individual US universities (i.e., Johns Hopkins, University of Maryland, Yale, etc.)."@en ;
              rdfs:isDefinedBy "The object of interest in a Business Process."@en .


###  https://w3id.org/italia/onto/gsim-sum#UnitDataStructure
gsim-sum:UnitDataStructure rdf:type owl:Class ;
                           rdfs:subClassOf gsim-sum:DataStructure ;
                           rdfs:comment "For example (social security number, country of residence, age, citizenship, country of birth) where the social security number and the country of residence are the identifying components (Identifier Component) and the others are measured variables obtained directly or indirectly from the person (Unit) and are Measure Components of the Logical Record."@en ;
                           rdfs:isDefinedBy "Describes the structure of a Unit Data Set."@en .


###  https://w3id.org/italia/onto/gsim-sum#UnitType
gsim-sum:UnitType rdf:type owl:Class ;
                  rdfs:subClassOf gsim-sum:Concept ;
                  rdfs:comment """A Unit Type is used to describe a class or group of Units based on a single characteristic, but with no specification of time and geography. For example, the Unit Type of “Person” groups together a set of Units based on the characteristic that they are ‘Persons’.
It concerns not only Unit Types used in dissemination, but anywhere in the statistical process. E.g. using administrative data might involve the use of a fiscal unit"""@en ;
                  rdfs:isDefinedBy "A Unit Type is a class of objects of interest. "@en .


###  https://w3id.org/italia/onto/gsim-sum#ValueDomain
gsim-sum:ValueDomain rdf:type owl:Class ;
                     rdfs:subClassOf gsim-sum:Concepts ;
                     rdfs:comment "The values can be described by enumeration or by an expression."@en ;
                     rdfs:isDefinedBy "The permitted range of values for a characteristic of a variable."@en .


###  https://w3id.org/italia/onto/gsim-sum#Variable
gsim-sum:Variable rdf:type owl:Class ;
                  rdfs:subClassOf gsim-sum:Concept ;
                  rdfs:comment """The Variable combines the meaning of a Concept with a Unit Type, to define the characteristic that is to be measured.
Here are 3 examples - 1. Sex of person 2. Number of employees 3. Value of endowment."""@en ;
                  rdfs:isDefinedBy "The use of a Concept as a characteristic of a Population intended to be measured."@en .


###  https://w3id.org/sdp/core#BusinessProcess
:BusinessProcess rdf:type owl:Class .


###  https://w3id.org/sdp/core#CoreInput
:CoreInput rdf:type owl:Class ;
           rdfs:subClassOf :ProcessInput .


###  https://w3id.org/sdp/core#CoreOutput
:CoreOutput rdf:type owl:Class ;
            rdfs:subClassOf :ProcessOutput .


###  https://w3id.org/sdp/core#IdentifiableArtefact
:IdentifiableArtefact rdf:type owl:Class .


###  https://w3id.org/sdp/core#ParameterInput
:ParameterInput rdf:type owl:Class ;
                rdfs:subClassOf :ProcessInput .


###  https://w3id.org/sdp/core#ProcessControlDesign
:ProcessControlDesign rdf:type owl:Class .


###  https://w3id.org/sdp/core#ProcessDesign
:ProcessDesign rdf:type owl:Class .


###  https://w3id.org/sdp/core#ProcessExecutionLog
:ProcessExecutionLog rdf:type owl:Class ;
                     rdfs:subClassOf :ProcessOutput .


###  https://w3id.org/sdp/core#ProcessInput
:ProcessInput rdf:type owl:Class .


###  https://w3id.org/sdp/core#ProcessInputSpecification
:ProcessInputSpecification rdf:type owl:Class .


###  https://w3id.org/sdp/core#ProcessMethod
:ProcessMethod rdf:type owl:Class .


###  https://w3id.org/sdp/core#ProcessMetric
:ProcessMetric rdf:type owl:Class ;
               rdfs:subClassOf :ProcessOutput .


###  https://w3id.org/sdp/core#ProcessOutput
:ProcessOutput rdf:type owl:Class .


###  https://w3id.org/sdp/core#ProcessOutputSpecification
:ProcessOutputSpecification rdf:type owl:Class .


###  https://w3id.org/sdp/core#ProcessStep
:ProcessStep rdf:type owl:Class .


###  https://w3id.org/sdp/core#ProcessSupportInput
:ProcessSupportInput rdf:type owl:Class ;
                     rdfs:subClassOf :ProcessInput .


###  https://w3id.org/sdp/core#Rule
:Rule rdf:type owl:Class .


###  https://w3id.org/sdp/core#StatisticalProgram
:StatisticalProgram rdf:type owl:Class .


###  https://w3id.org/sdp/core#StatisticalProgramCycle
:StatisticalProgramCycle rdf:type owl:Class .


###  https://w3id.org/sdp/core#StatisticalProgramDesign
:StatisticalProgramDesign rdf:type owl:Class .


#################################################################
#    Individuals
#################################################################

###  http://id.unece.org/models/gamso/CapabilityDevelopmentActivity
<http://id.unece.org/models/gamso/CapabilityDevelopmentActivity> rdf:type owl:NamedIndividual ,
                                                                          gamso:StatisticalSupportingActivity ;
                                                                 skos:definition "This activity area includes research, development and innovation activities i.e. the development of capabilities that enable the organisation to undertake new activities, or to improve the efficiency of existing ones. It promotes the re-use and sharing of infrastructure (statistical and technical), both inside the organisation and across organisations, to facilitate harmonisation and to improve the coherence of statistical outputs. Some of these activities may be outsourced to partners in the private or academic sectors, or even to other statistical organisations. When a new capability or a capability improvement is fully integrated in Production, its support is transferred to one or more activities of Corporate Support."@en ;
                                                                 skos:inScheme <http://id.unece.org/models/gamso/GAMSO> ;
                                                                 skos:narrower <http://id.unece.org/models/gamso/DevelopCapabilityImprovementsActivity> ,
                                                                               <http://id.unece.org/models/gamso/MonitorCapabilityImprovementsActivity> ,
                                                                               <http://id.unece.org/models/gamso/PlanCapabilityImprovementsActivity> ,
                                                                               <http://id.unece.org/models/gamso/TransferSupportOfCapabilityImprovementsActivity> ;
                                                                 skos:notation "2" ;
                                                                 skos:prefLabel "Capability Management" ;
                                                                 skos:topConceptOf <http://id.unece.org/models/gamso/GAMSO> .


###  http://id.unece.org/models/gamso/CorporateSupportActivity
<http://id.unece.org/models/gamso/CorporateSupportActivity> rdf:type owl:NamedIndividual ,
                                                                     gamso:StatisticalSupportingActivity ;
                                                            skos:definition "These activities support standardisation. They cover the cross-cutting activities required by the organisation to deliver its work programme efficiently and effectively. When a capability improvement is fully integrated in Production, its support is transferred to one or more activities of Corporate Support."@en ;
                                                            skos:inScheme <http://id.unece.org/models/gamso/GAMSO> ;
                                                            skos:narrower <http://id.unece.org/models/gamso/ManageBuildingsAndPhysicalSpaceActivity> ,
                                                                          <http://id.unece.org/models/gamso/ManageBusinessPerformanceAndLegislationActivity> ,
                                                                          <http://id.unece.org/models/gamso/ManageCustomersActivity> ,
                                                                          <http://id.unece.org/models/gamso/ManageDataSuppliersActivity> ,
                                                                          <http://id.unece.org/models/gamso/ManageFinancesActivity> ,
                                                                          <http://id.unece.org/models/gamso/ManageHumanResourcesActivity> ,
                                                                          <http://id.unece.org/models/gamso/ManageITActivity> ,
                                                                          <http://id.unece.org/models/gamso/ManageInformationAndKnowledgeActivity> ,
                                                                          <http://id.unece.org/models/gamso/ManageQualityActivity> ,
                                                                          <http://id.unece.org/models/gamso/ManageStatisticalMethodologyActivity> ;
                                                            skos:notation "3" ;
                                                            skos:prefLabel "Corporate Support" ;
                                                            skos:topConceptOf <http://id.unece.org/models/gamso/GAMSO> .


###  http://id.unece.org/models/gamso/DefineVisionActivity
<http://id.unece.org/models/gamso/DefineVisionActivity> rdf:type owl:NamedIndividual ,
                                                                 gamso:StrategyAndLeadershipActivity ;
                                                        skos:broader <http://id.unece.org/models/gamso/StrategyAndLeadershipActivity> ;
                                                        skos:definition """These activities ensure that statistical organisations understand the environment in which they operate and the emerging issues they are confronted with, so that it is clear where they can provide independent, evidence-based information, as well as statistical standards and infrastructure, for use by governments and the broader community. 

Based on this, statistical organisations determine their high-level goals and directions, including the values which will guide them, so they set their statistical programmes accordingly. This also includes communicating the mission, values and expectations internally and externally, to lead and inspire staff and to increase government and community trust and confidence in the organisation and in official statistics in general. These include:

• Understand national and international directions and factors
• Determine vision, mission and strategic goals 
• Determine organisational value proposition
• Determine and communicate values and expectations
• Create interest and awareness"""@en ;
                                                        skos:inScheme <http://id.unece.org/models/gamso/GAMSO> ;
                                                        skos:notation "1.1" ;
                                                        skos:prefLabel "Define Vision"@en .


###  http://id.unece.org/models/gamso/DevelopCapabilityImprovementsActivity
<http://id.unece.org/models/gamso/DevelopCapabilityImprovementsActivity> rdf:type owl:NamedIndividual ,
                                                                                  gamso:CapabilityDevelopmentActivity ;
                                                                         skos:broader <http://id.unece.org/models/gamso/CapabilityDevelopmentActivity> ;
                                                                         skos:definition """These activities develop approved improvement projects from the requirements stage through to their completion. The developers will undertake background research, define the detailed requirements, coordinate the design and building, and finalize all aspects of the capabilities being developed, including their deployment for operational use. 

The activities mainly concern the development of capability improvements for multiple statistical business processes, including cases where capability improvements are developed through partnering with other statistical organisation or through implementing reusable infrastructure originally developed by others. Capability improvements in the context of a single statistical business process are included in the Production activity area. 

The activities include:
• Undertake background research
• Define detailed capability requirements
• Design capability solution
• Build/procure and deploy capability solution"""@en ;
                                                                         skos:inScheme <http://id.unece.org/models/gamso/GAMSO> ;
                                                                         skos:notation "2.2" ;
                                                                         skos:prefLabel "Develop Capability Improvement"@en .


###  http://id.unece.org/models/gamso/GAMSO
<http://id.unece.org/models/gamso/GAMSO> rdf:type owl:NamedIndividual ,
                                                  skos:ConceptScheme ;
                                         rdfs:label "Supporting Activity For Statistical Organisations"@en ;
                                         skos:hasTopConcept <http://id.unece.org/models/gamso/CapabilityDevelopmentActivity> ,
                                                            <http://id.unece.org/models/gamso/CorporateSupportActivity> ,
                                                            <http://id.unece.org/models/gamso/StrategyAndLeadershipActivity> .


###  http://id.unece.org/models/gamso/GovernAndLeadActivity
<http://id.unece.org/models/gamso/GovernAndLeadActivity> rdf:type owl:NamedIndividual ,
                                                                  gamso:StrategyAndLeadershipActivity ;
                                                         skos:broader <http://id.unece.org/models/gamso/StrategyAndLeadershipActivity> ;
                                                         skos:definition """These activities cover the development of strategies to achieve the goals and directions set under Define Vision. They include identification and prioritisation of the statistical work programme, prioritisation of the capital investment programme, and the allocation of resources (capital and labour) to implement the agreed programmes defined in the statistical product and service and capability portfolios. 

Under Govern and Lead the need for capability improvements is identified and requested by prioritising the capability portfolio, under Capability Development the requested and prioritized capability improvements are planned in more detail, developed, monitored and after their full integration in Production their support is transferred to Corporate Support. 

Activities under Govern and Lead include:
• Develop strategies for achieving organisational goals
• Prioritise capability portfolio
• Prioritise statistical product and service portfolio
• Define and manage statistical programme
• Allocate project and programme portfolio budgets
• Build and maintain internal statistical and professional excellence  
• Ensure general coordination and alignment
• Define general organisational policies
• Publish policies, guidelines and normative documents"""@en ;
                                                         skos:inScheme <http://id.unece.org/models/gamso/GAMSO> ;
                                                         skos:notation "1.2" ;
                                                         skos:prefLabel "Govern and Lead"@en .


###  http://id.unece.org/models/gamso/ManageBuildingsAndPhysicalSpaceActivity
<http://id.unece.org/models/gamso/ManageBuildingsAndPhysicalSpaceActivity> rdf:type owl:NamedIndividual ,
                                                                                    gamso:CorporateSupportActivity ;
                                                                           skos:broader <http://id.unece.org/models/gamso/CorporateSupportActivity> ;
                                                                           skos:definition """These activities cover maintenance of the building and allocation of physical space the organisation occupies. These include:
• Manage environmental, mechanical, and electrical needs
• Manage arrangement of office space
• Manage distribution of offices within space"""@en ;
                                                                           skos:inScheme <http://id.unece.org/models/gamso/GAMSO> ;
                                                                           skos:notation "3.9" ;
                                                                           skos:prefLabel "Manage Building and Physical Space"@en .


###  http://id.unece.org/models/gamso/ManageBusinessPerformanceAndLegislationActivity
<http://id.unece.org/models/gamso/ManageBusinessPerformanceAndLegislationActivity> rdf:type owl:NamedIndividual ,
                                                                                            gamso:CorporateSupportActivity ;
                                                                                   skos:broader <http://id.unece.org/models/gamso/CorporateSupportActivity> ;
                                                                                   skos:definition """These activities manage how the organisation conducts its business, including agreed changes to the business, in order to achieve planned outputs and outcomes. These include:
• Manage business performance
• Manage change and risk
• Manage legislation & compliance"""@en ;
                                                                                   skos:inScheme <http://id.unece.org/models/gamso/GAMSO> ;
                                                                                   skos:notation "3.1" ;
                                                                                   skos:prefLabel "Manage Business and Performance"@en .


###  http://id.unece.org/models/gamso/ManageCustomersActivity
<http://id.unece.org/models/gamso/ManageCustomersActivity> rdf:type owl:NamedIndividual ,
                                                                    gamso:CorporateSupportActivity ;
                                                           skos:broader <http://id.unece.org/models/gamso/CorporateSupportActivity> ;
                                                           skos:definition """These activities cover the management of communication and exchanges between governmental or international institutions, the public, and other stakeholders in direct or indirect support of organisational services. They therefore deal with the relationships between statistical organisations and the public, including those via the media. This includes general marketing activities and dealing with non-specific consumer feedback. This also includes measures to educate and inform users so that they fully understand statistical outputs, and to promote and improve levels of statistical literacy in society in general. These include:
• Manage communications and media relations
• Manage stakeholder consultations
• Manage cross-product user support"""@en ;
                                                           skos:inScheme <http://id.unece.org/models/gamso/GAMSO> ;
                                                           skos:notation "3.7" ;
                                                           skos:prefLabel "Manage Consumers"@en .


###  http://id.unece.org/models/gamso/ManageDataSuppliersActivity
<http://id.unece.org/models/gamso/ManageDataSuppliersActivity> rdf:type owl:NamedIndividual ,
                                                                        gamso:CorporateSupportActivity ;
                                                               skos:broader <http://id.unece.org/models/gamso/CorporateSupportActivity> ;
                                                               skos:definition """These activities cover the relationships with sub-national governments and private entities that supply data for statistical activities. This includes cross-process burden management, as well as topics such as profiling and management of contact information (and thus has particularly close links with statistical business processes that maintain registers. These include:
• Manage data sharing agreements
• Manage data transfer"""@en ;
                                                               skos:inScheme <http://id.unece.org/models/gamso/GAMSO> ;
                                                               skos:notation "3.8" ;
                                                               skos:prefLabel "Manage Data Supplier"@en .


###  http://id.unece.org/models/gamso/ManageFinancesActivity
<http://id.unece.org/models/gamso/ManageFinancesActivity> rdf:type owl:NamedIndividual ,
                                                                   gamso:CorporateSupportActivity ;
                                                          skos:broader <http://id.unece.org/models/gamso/CorporateSupportActivity> ;
                                                          skos:definition """These activities cover the organisation's ongoing use of financial and accounting information to measure, operate and predict the efficiency and effectiveness of its activities, including procurement and contracts, in relation to the organisation's goals and objectives. Suppliers as referring to commercial provides of goods and services for the statistical organisation. These include:
• Maintain accounts (including assets and liabilities)
• Manage procurement and contracts
• Manage suppliers of equipment, office supplies and services"""@en ;
                                                          skos:inScheme <http://id.unece.org/models/gamso/GAMSO> ;
                                                          skos:notation "3.2" ;
                                                          skos:prefLabel "Manage Finances"@en .


###  http://id.unece.org/models/gamso/ManageHumanResourcesActivity
<http://id.unece.org/models/gamso/ManageHumanResourcesActivity> rdf:type owl:NamedIndividual ,
                                                                         gamso:CorporateSupportActivity ;
                                                                skos:broader <http://id.unece.org/models/gamso/CorporateSupportActivity> ;
                                                                skos:definition """These activities cover employee performance, recruitment, skills development, talent management and succession planning work. These include:
• Manage employee performance
• Manage and develop skills
• Manage talent
• Manage recruitment
• Ensure succession planning"""@en ;
                                                                skos:inScheme <http://id.unece.org/models/gamso/GAMSO> ;
                                                                skos:notation "3.3" ;
                                                                skos:prefLabel "Manage Human Resources"@en .


###  http://id.unece.org/models/gamso/ManageITActivity
<http://id.unece.org/models/gamso/ManageITActivity> rdf:type owl:NamedIndividual ,
                                                             gamso:CorporateSupportActivity ;
                                                    skos:broader <http://id.unece.org/models/gamso/CorporateSupportActivity> ;
                                                    skos:definition """These activities cover coordination and management of information and technology resources and solutions. They include the management of the physical security of data. These include:
• Manage IT assets and services
• Manage IT security
• Manage technological change"""@en ;
                                                    skos:inScheme <http://id.unece.org/models/gamso/GAMSO> ;
                                                    skos:notation "3.4" ;
                                                    skos:prefLabel "Manage IT"@en .


###  http://id.unece.org/models/gamso/ManageInformationAndKnowledgeActivity
<http://id.unece.org/models/gamso/ManageInformationAndKnowledgeActivity> rdf:type owl:NamedIndividual ,
                                                                                  gamso:CorporateSupportActivity ;
                                                                         skos:broader <http://id.unece.org/models/gamso/CorporateSupportActivity> ;
                                                                         skos:definition """These activities cover the ownership or custody of records, documents, information and other intellectual assets held by the organisation and the governance of information collection, arrangement, storage, maintenance, retrieval, dissemination and destruction. They also include maintaining the policies, guidelines and standards regarding information management and governance. These include:
• Manage documents and records, including destruction and archiving
• Manage knowledge
• Manage information standards and rights
• Manage metadata and data"""@en ;
                                                                         skos:inScheme <http://id.unece.org/models/gamso/GAMSO> ;
                                                                         skos:notation "3.6" ;
                                                                         skos:prefLabel "Manage Information and Knowledge"@en .


###  http://id.unece.org/models/gamso/ManageQualityActivity
<http://id.unece.org/models/gamso/ManageQualityActivity> rdf:type owl:NamedIndividual ,
                                                                  gamso:CorporateSupportActivity ;
                                                         skos:broader <http://id.unece.org/models/gamso/CorporateSupportActivity> ;
                                                         skos:definition """These activities cover developing and administering a quality framework and cross-cutting work with tools to assure quality, i.e. compliance with the quality framework that should cover quality linked to the organisational framework, processes and products. Such tools comprise quality indicators (including balancing quality components), user surveys, self-assessments, quality reviews or audits, certification and labelling of statistics. Quality documentation here refers to the organisational level and covers quality declarations, policies and relevant guidelines such as guidelines on handling of errors and revisions. These include:
• Manage quality framework
• Manage quality assurance tools
• Manage quality documentation"""@en ;
                                                         skos:inScheme <http://id.unece.org/models/gamso/GAMSO> ;
                                                         skos:notation "3.10" ;
                                                         skos:prefLabel "Manage Quality"@en .


###  http://id.unece.org/models/gamso/ManageStatisticalMethodologyActivity
<http://id.unece.org/models/gamso/ManageStatisticalMethodologyActivity> rdf:type owl:NamedIndividual ,
                                                                                 gamso:CorporateSupportActivity ;
                                                                        skos:broader <http://id.unece.org/models/gamso/CorporateSupportActivity> ;
                                                                        skos:definition """These activities cover the need to maintain the confidentiality and disclosure of information collected, maintained, or disseminated about individual persons, businesses or other entities. These include:
• Manage cross-cutting statistical methodologies
• Manage confidentiality
• Manage disclosure control"""@en ;
                                                                        skos:inScheme <http://id.unece.org/models/gamso/GAMSO> ;
                                                                        skos:notation "3.5" ;
                                                                        skos:prefLabel "Manage Statistical Methodology"@en .


###  http://id.unece.org/models/gamso/ManageStrategicCollaborationAndCooperationActivity
<http://id.unece.org/models/gamso/ManageStrategicCollaborationAndCooperationActivity> rdf:type owl:NamedIndividual ,
                                                                                               gamso:StrategyAndLeadershipActivity ;
                                                                                      skos:broader <http://id.unece.org/models/gamso/StrategyAndLeadershipActivity> ;
                                                                                      skos:definition """These activities cover collaboration, cooperation and coordination with other statistical organisations and other external stakeholders. They can include coordination within a statistical system, which may be based on a geographical hierarchy of entities (local, regional, national, multi-national), or a split of responsibilities between organisations based upon activities. They include activities undertaken to identify new opportunities for data exchange or integration. They provide the statistical community with opportunities to exchange knowledge, to improve statistical infrastructure and practices and to influence statistical standards. 

These activities contribute to the building and enhancing of shared statistical capabilities managed by partners, leading to increased statistical understanding and improved application and use. They include organisation and coordination of other organisations which produce official statistics as part of a national system. These include:
• Build and maintain strategic relations, nationally and internationally
• Build and maintain external statistical excellence
• Advance inter-agency and international collaborations
• Secure support for statistical product and service and capability portfolio
• Coordinate the national statistical system"""@en ;
                                                                                      skos:inScheme <http://id.unece.org/models/gamso/GAMSO> ;
                                                                                      skos:notation "1.3" ;
                                                                                      skos:prefLabel "Manage Strategic Collaboration and Cooperation"@en .


###  http://id.unece.org/models/gamso/MonitorCapabilityImprovementsActivity
<http://id.unece.org/models/gamso/MonitorCapabilityImprovementsActivity> rdf:type owl:NamedIndividual ,
                                                                                  gamso:CapabilityDevelopmentActivity ;
                                                                         skos:broader <http://id.unece.org/models/gamso/CapabilityDevelopmentActivity> ;
                                                                         skos:definition """These activities aim at monitoring the organisation capabilities, ensuring the organisation reaps maximum benefits from investments. They involve maintaining capabilities, evaluating them or suggesting where improvements are required. Staff members undertaking these activities effectively become the custodians/reference persons for the capabilities, taking responsibility for their fitness for purpose. These include:

• Maintain capability improvements 
• Promote capability improvements
• Evaluate capability improvements"""@en ;
                                                                         skos:inScheme <http://id.unece.org/models/gamso/GAMSO> ;
                                                                         skos:notation "2.3" ;
                                                                         skos:prefLabel "Monitor Capabilities"@en .


###  http://id.unece.org/models/gamso/PlanCapabilityImprovementsActivity
<http://id.unece.org/models/gamso/PlanCapabilityImprovementsActivity> rdf:type owl:NamedIndividual ,
                                                                               gamso:CapabilityDevelopmentActivity ;
                                                                      skos:broader <http://id.unece.org/models/gamso/CapabilityDevelopmentActivity> ;
                                                                      skos:definition """These activities aim at planning the best way forward to develop a new capability or improve an organisation's capabilities. They require a thorough organisational view of change requirements, the prioritisation of options through an efficient, iterative approval process until a work programme for capability improvements is finalised. 

These activities further coordinate the planning and resourcing of cross-cutting/reusable capability improvement projects (both large and small), to ensure key improvement work is integrated across the organisation, with interdependencies understood and the resources optimized across the work programme. 

These activities also monitor the ongoing progress of the work programme and report to the relevant governance fora to ensure all required change requests occur in an efficient and effective manner. 

The activities include:
• Identify disruptions and capability improvements
• Propose capability improvement projects
• Manage capability improvement programmes"""@en ;
                                                                      skos:inScheme <http://id.unece.org/models/gamso/GAMSO> ;
                                                                      skos:notation "2.1" ;
                                                                      skos:prefLabel "Plan Capability Improvements"@en .


###  http://id.unece.org/models/gamso/StatisticalSupportingActivity
<http://id.unece.org/models/gamso/StatisticalSupportingActivity> rdf:type owl:NamedIndividual ,
                                                                          gamso:StatisticalSupportingActivity ;
                                                                 rdfs:label "Supporting Activity For Statistical Organisations"@en ;
                                                                 skos:inScheme <http://id.unece.org/models/gamso/GAMSO> .


###  http://id.unece.org/models/gamso/StrategyAndLeadershipActivity
<http://id.unece.org/models/gamso/StrategyAndLeadershipActivity> rdf:type owl:NamedIndividual ,
                                                                          gamso:StatisticalSupportingActivity ;
                                                                 skos:definition """These activities ensure that statistical organisations understand the environment in which they operate and the emerging issues they are confronted with, so that it is clear where they can provide independent, evidence-based information, as well as statistical standards and infrastructure, for use by governments and the broader community. 

Based on this, statistical organisations determine their high-level goals and directions, including the values which will guide them, so they set their statistical programmes accordingly. This also includes communicating the mission, values and expectations internally and externally, to lead and inspire staff and to increase government and community trust and confidence in the organisation and in official statistics in general. These include:

• Understand national and international directions and factors
• Determine vision, mission and strategic goals 
• Determine organisational value proposition
• Determine and communicate values and expectations
• Create interest and awareness"""@en ;
                                                                 skos:inScheme <http://id.unece.org/models/gamso/GAMSO> ;
                                                                 skos:narrower <http://id.unece.org/models/gamso/DefineVisionActivity> ,
                                                                               <http://id.unece.org/models/gamso/GovernAndLeadActivity> ,
                                                                               <http://id.unece.org/models/gamso/ManageStrategicCollaborationAndCooperationActivity> ;
                                                                 skos:notation "1" ;
                                                                 skos:prefLabel "Strategy and Leadership" ;
                                                                 skos:topConceptOf <http://id.unece.org/models/gamso/GAMSO> .


###  http://id.unece.org/models/gamso/TransferSupportOfCapabilityImprovementsActivity
<http://id.unece.org/models/gamso/TransferSupportOfCapabilityImprovementsActivity> rdf:type owl:NamedIndividual ,
                                                                                            gamso:CapabilityDevelopmentActivity ;
                                                                                   skos:broader <http://id.unece.org/models/gamso/CapabilityDevelopmentActivity> ;
                                                                                   skos:definition """These activities provide the technical hands-on assistance required across the organisation to ensure that the capability improvements are actually used in support of the statistical work programme. These activities also guide the successful operation of individual reusable business processes and transfer of shared infrastructures. When a capability improvement is fully integrated in Production, its support is transferred to one or more activities of Corporate Support. These include:
• Transfer design
• Transfer operations
• Transfer user support"""@en ;
                                                                                   skos:inScheme <http://id.unece.org/models/gamso/GAMSO> ;
                                                                                   skos:notation "2.4" ;
                                                                                   skos:prefLabel "Support Capability Implementation"@en .


###  http://id.unece.org/models/gsbpm/GSBPM
igsbpm:GSBPM rdf:type owl:NamedIndividual ,
                      skos:ConceptScheme ;
             rdfs:label "Generic Statistical Business Process Model"@en ,
                        "Modèle générique de processus métier statistique"@fr ;
             skos:hasTopConcept <http://id.unece.org/models/gsbpm/1> ,
                                <http://id.unece.org/models/gsbpm/2> ,
                                <http://id.unece.org/models/gsbpm/3> ,
                                <http://id.unece.org/models/gsbpm/4> ,
                                <http://id.unece.org/models/gsbpm/5> ,
                                <http://id.unece.org/models/gsbpm/6> ,
                                <http://id.unece.org/models/gsbpm/7> ,
                                <http://id.unece.org/models/gsbpm/8> ;
             foaf:homepage <http://www1.unece.org/stat/platform/display/GSBPM/GSBPM+v5.0> .


###  http://id.unece.org/models/gsbpm/StatisticalProductionProcess
igsbpm:StatisticalProductionProcess rdf:type owl:NamedIndividual ,
                                             gsbpm:StatisticalProductionActivity ;
                                    rdfs:label "Processus de production statistique"@fr ,
                                               "Statistical Production Process"@en ;
                                    skos:inScheme igsbpm:GSBPM .


###  http://id.unece.org/models/gsbpm/1
<http://id.unece.org/models/gsbpm/1> rdf:type owl:NamedIndividual ,
                                              gsbpm:Phase ;
                                     skos:definition """This phase is triggered when a need for new statistics is identified, or feedback about current statistics initiates a review. It includes all activities associated with engaging customers to identify their detailed statistical needs, proposing high level solution options and preparing business cases to meet these needs.
In this phase the organisation:
- identifies the need for the statistics;
- confirms, in more detail, the statistical needs of the stakeholders;
- establishes the high level objectives of the statistical outputs;
- identifies the relevant concepts and variables for which data are required;
- checks the extent to which current data sources can meet these needs;
- prepares the business case to get approval to produce the statistics.
This phase is broken down into six sub-processes. These are generally sequential, from left to right, but can also occur in parallel, and can be iterative. The sub-processes are:
"""@en ;
                                     skos:inScheme igsbpm:GSBPM ;
                                     skos:narrower <http://id.unece.org/models/gsbpm/1.1> ,
                                                   <http://id.unece.org/models/gsbpm/1.2> ,
                                                   <http://id.unece.org/models/gsbpm/1.3> ,
                                                   <http://id.unece.org/models/gsbpm/1.4> ,
                                                   <http://id.unece.org/models/gsbpm/1.5> ,
                                                   <http://id.unece.org/models/gsbpm/1.6> ;
                                     skos:notation "1" ;
                                     skos:prefLabel "Specify Needs"@en ;
                                     skos:topConceptOf igsbpm:GSBPM .


###  http://id.unece.org/models/gsbpm/1.1
<http://id.unece.org/models/gsbpm/1.1> rdf:type owl:NamedIndividual ,
                                                gsbpm:SubProcess ;
                                       skos:broader <http://id.unece.org/models/gsbpm/1> ;
                                       skos:definition """This sub-process includes the initial investigation and identification of what statistics are needed and what is needed of the statistics. It may be triggered by a new information request, an environmental change such as a reduced budget. Action plans from evaluations of previous iterations of the process, or from other processes, might provide an input to this sub-process. It also includes consideration of practice amongst other (national and international) statistical organisations producing similar data, and in particular the methods used by those organisations. It may involve consideration of specific needs of different user communities, such as the disabled, or different ethnic groups.
"""@en ;
                                       skos:inScheme igsbpm:GSBPM ;
                                       skos:notation "1.1" ;
                                       skos:prefLabel "Identify Needs"@en .


###  http://id.unece.org/models/gsbpm/1.2
<http://id.unece.org/models/gsbpm/1.2> rdf:type owl:NamedIndividual ,
                                                gsbpm:SubProcess ;
                                       skos:broader <http://id.unece.org/models/gsbpm/1> ;
                                       skos:definition """This sub-process focuses on consulting with the stakeholders and confirming in detail the needs for the statistics. A good understanding of user needs is required so that the statistical organisation knows not only what it is expected to deliver, but also when, how, and, perhaps most importantly, why. For second and subsequent iterations of this phase, the main focus will be on determining whether previously identified needs have changed. This detailed understanding of user needs is the critical part of this sub-process.
"""@en ;
                                       skos:inScheme igsbpm:GSBPM ;
                                       skos:notation "1.2" ;
                                       skos:prefLabel "Consult and confirm needs"@en .


###  http://id.unece.org/models/gsbpm/1.3
<http://id.unece.org/models/gsbpm/1.3> rdf:type owl:NamedIndividual ,
                                                gsbpm:SubProcess ;
                                       skos:broader <http://id.unece.org/models/gsbpm/1> ;
                                       skos:definition """This sub-process identifies the statistical outputs that are required to meet the user needs identified in sub-process 1.2 (Consult and confirm needs). It includes agreeing the suitability of the proposed outputs and their quality measures with users. Legal frameworks (e.g. relating to confidentiality), and available resources are likely to be constraints when establishing output objectives.
"""@en ;
                                       skos:inScheme igsbpm:GSBPM ;
                                       skos:notation "1.3" ;
                                       skos:prefLabel "Establish output objectives"@en .


###  http://id.unece.org/models/gsbpm/1.4
<http://id.unece.org/models/gsbpm/1.4> rdf:type owl:NamedIndividual ,
                                                gsbpm:SubProcess ;
                                       skos:broader <http://id.unece.org/models/gsbpm/1> ;
                                       skos:definition """This sub-process clarifies the required concepts to be measured by the business process from the point of view of the user. At this stage the concepts identified may not align with existing statistical standards. This alignment, and the choice or definition of the statistical concepts and variables to be used, takes place in sub-process 2.2.
"""@en ;
                                       skos:inScheme igsbpm:GSBPM ;
                                       skos:notation "1.4" ;
                                       skos:prefLabel "Identify concepts"@en .


###  http://id.unece.org/models/gsbpm/1.5
<http://id.unece.org/models/gsbpm/1.5> rdf:type owl:NamedIndividual ,
                                                gsbpm:SubProcess ;
                                       skos:broader <http://id.unece.org/models/gsbpm/1> ;
                                       skos:definition """This sub-process checks whether current data sources could meet user requirements, and the conditions under which they would be available, including any restrictions on their use. An assessment of possible alternatives would normally include research into potential administrative or other non-statistical data sources, to determine whether they would be suitable for use for statistical purposes. When existing sources have been assessed, a strategy for filling any remaining gaps in the data requirement is prepared. This sub-process also includes a more general assessment of the legal framework in which data would be collected and used, and may therefore identify proposals for changes to existing legislation or the introduction of a new legal framework.
"""@en ;
                                       skos:inScheme igsbpm:GSBPM ;
                                       skos:notation "1.5" ;
                                       skos:prefLabel "Check data availability"@en .


###  http://id.unece.org/models/gsbpm/1.6
<http://id.unece.org/models/gsbpm/1.6> rdf:type owl:NamedIndividual ,
                                                gsbpm:SubProcess ;
                                       skos:broader <http://id.unece.org/models/gsbpm/1> ;
                                       skos:definition """This sub-process documents the findings of the other sub-processes in this phase in the form of a business case to get approval to implement the new or modified statistical business process. Such a business case would need to conform to the requirements of the approval body, but would typically include elements such as:
- A description of the \"As-Is\" business process (if it already exists), with information on how the current statistics are produced, highlighting any inefficiencies and issues to be addressed;
- The proposed \"To-Be\" solution, detailing how the statistical business process will be developed to produce the new or revised statistics;
- An assessment of costs and benefits, as well as any external constraints.
"""@en ;
                                       skos:inScheme igsbpm:GSBPM ;
                                       skos:notation "1.6" ;
                                       skos:prefLabel "Prepare business case"@en .


###  http://id.unece.org/models/gsbpm/2
<http://id.unece.org/models/gsbpm/2> rdf:type owl:NamedIndividual ,
                                              gsbpm:Phase ;
                                     skos:definition """This phase describes the development and design activities, and any associated practical research work needed to define the statistical outputs, concepts, methodologies, collection instruments1 and operational processes. It includes all the design elements needed to define or refine the statistical products or services identified in the business case.  This phase specifies all relevant metadata, ready for use later in the statistical business process, as well as quality assurance procedures. For statistical outputs produced on a regular basis, this phase usually occurs for the first iteration, and whenever improvement actions are identified in the Evaluate phase of a previous iteration.
Design activities make substantial use of international and national standards, in order to reduce the length and cost of the design process, and enhance to comparability and usability of outputs. Organisations are also encouraged to reuse or adapt design elements from existing processes. Additionally, outputs of design processes may form the basis for future standards at the organisation, national or international levels.
This phase is broken down into six sub-processes, which are generally sequential, from left to right, but can also occur in parallel, and can be iterative. These sub-processes are:
"""@en ;
                                     skos:inScheme igsbpm:GSBPM ;
                                     skos:narrower <http://id.unece.org/models/gsbpm/2.1> ,
                                                   <http://id.unece.org/models/gsbpm/2.2> ,
                                                   <http://id.unece.org/models/gsbpm/2.3> ,
                                                   <http://id.unece.org/models/gsbpm/2.4> ,
                                                   <http://id.unece.org/models/gsbpm/2.5> ,
                                                   <http://id.unece.org/models/gsbpm/2.6> ;
                                     skos:notation "2" ;
                                     skos:prefLabel "Design"@en ;
                                     skos:topConceptOf igsbpm:GSBPM .


###  http://id.unece.org/models/gsbpm/2.1
<http://id.unece.org/models/gsbpm/2.1> rdf:type owl:NamedIndividual ,
                                                gsbpm:SubProcess ;
                                       skos:broader <http://id.unece.org/models/gsbpm/2> ;
                                       skos:definition """This sub-process contains the detailed design of the statistical outputs, products and services to be produced, including the related development work and preparation of the systems and tools used in the \"Disseminate\" phase. Disclosure control methods, as well as processes governing access to any confidential outputs are also designed here. Outputs should be designed to follow existing standards wherever possible, so inputs to this process may include metadata from similar or previous collections, international standards, and information about practices in other statistical organisations from sub-process 1.1 (Identify needs).
"""@en ;
                                       skos:inScheme igsbpm:GSBPM ;
                                       skos:notation "2.1" ;
                                       skos:prefLabel "Design outputs"@en .


###  http://id.unece.org/models/gsbpm/2.2
<http://id.unece.org/models/gsbpm/2.2> rdf:type owl:NamedIndividual ,
                                                gsbpm:SubProcess ;
                                       skos:broader <http://id.unece.org/models/gsbpm/2> ;
                                       skos:definition """This sub-process defines the statistical variables to be collected via the collection instrument, as well as any other variables that will be derived from them in sub-process 5.5 (Derive new variables and units), and any statistical classifications that will be used. It is expected that existing national and international standards will be followed wherever possible. This sub-process may need to run in parallel with sub-process 2.3 (Design collection), as the definition of the variables to be collected, and the choice of collection instrument may be inter-dependent to some degree. Preparation of metadata descriptions of collected and derived variables and classifications is a necessary precondition for subsequent phases.
"""@en ;
                                       skos:inScheme igsbpm:GSBPM ;
                                       skos:notation "2.2" ;
                                       skos:prefLabel "Design variable descriptions"@en .


###  http://id.unece.org/models/gsbpm/2.3
<http://id.unece.org/models/gsbpm/2.3> rdf:type owl:NamedIndividual ,
                                                gsbpm:SubProcess ;
                                       skos:broader <http://id.unece.org/models/gsbpm/2> ;
                                       skos:definition """This sub-process determines the most appropriate collection method(s) and instrument(s). The actual activities in this sub-process will vary according to the type of collection instruments required, which can include computer assisted interviewing, paper questionnaires, administrative data interfaces and data integration techniques. This sub-process includes the design of collection instruments, questions and response templates (in conjunction with the variables and statistical classifications designed in sub-process 2.2 (Design variable descriptions)). It also includes the design of any formal agreements relating to data supply, such as memoranda of understanding, and confirmation of the legal basis for the data collection. This sub-process is enabled by tools such as question libraries (to facilitate the reuse of questions and related attributes), questionnaire tools (to enable the quick and easy compilation of questions into formats suitable for cognitive testing) and agreement templates (to help standardise terms and conditions). This sub-process also includes the design of process-specific provider management systems.
"""@en ;
                                       skos:inScheme igsbpm:GSBPM ;
                                       skos:notation "2.3" ;
                                       skos:prefLabel "Design collection"@en .


###  http://id.unece.org/models/gsbpm/2.4
<http://id.unece.org/models/gsbpm/2.4> rdf:type owl:NamedIndividual ,
                                                gsbpm:SubProcess ;
                                       skos:broader <http://id.unece.org/models/gsbpm/2> ;
                                       skos:definition """This sub-process only applies to processes which involve data collection based on sampling, such as through statistical surveys. It identifies and specifies the population of interest, defines a sampling frame (and, where necessary, the register from which it is derived), and determines the most appropriate sampling criteria and methodology (which could include complete enumeration). Common sources for a sampling frame are administrative and statistical registers, censuses and information from other sample surveys. This sub-process describes how these sources can be combined if needed. Analysis of whether the frame covers the target population should be performed. A sampling plan should be made: The actual sample is created in sub-process 4.1 (Create frame and select sample), using the methodology, specified in this sub-process.
"""@en ;
                                       skos:inScheme igsbpm:GSBPM ;
                                       skos:notation "2.4" ;
                                       skos:prefLabel "Design frame and sample"@en .


###  http://id.unece.org/models/gsbpm/2.5
<http://id.unece.org/models/gsbpm/2.5> rdf:type owl:NamedIndividual ,
                                                gsbpm:SubProcess ;
                                       skos:broader <http://id.unece.org/models/gsbpm/2> ;
                                       skos:definition """This sub-process designs the statistical processing methodology to be applied during the \"Process\" and \"Analyse\" phases. This can include specification of routines for coding, editing, imputing, estimating, integrating, validating and finalizing data sets.
"""@en ;
                                       skos:inScheme igsbpm:GSBPM ;
                                       skos:notation "2.5" ;
                                       skos:prefLabel "Design processing and analysis"@en .


###  http://id.unece.org/models/gsbpm/2.6
<http://id.unece.org/models/gsbpm/2.6> rdf:type owl:NamedIndividual ,
                                                gsbpm:SubProcess ;
                                       skos:broader <http://id.unece.org/models/gsbpm/2> ;
                                       skos:definition """This sub-process determines the workflow from data collection to dissemination, taking an overview of all the processes required within the whole statistical production process, and ensuring that they fit together efficiently with no gaps or redundancies. Various systems and databases are needed throughout the process. A general principle is to reuse processes and technology across many statistical business processes, so existing production solutions (e.g. services, systems and databases) should be examined first, to determine whether they are fit for purpose for this specific process, then, if any gaps are identified, new solutions should be designed. This sub-process also considers how staff will interact with systems, and who will be responsible for what and when.
"""@en ;
                                       skos:inScheme igsbpm:GSBPM ;
                                       skos:notation "2.6" ;
                                       skos:prefLabel "Design production systems and workflow"@en .


###  http://id.unece.org/models/gsbpm/3
<http://id.unece.org/models/gsbpm/3> rdf:type owl:NamedIndividual ,
                                              gsbpm:Phase ;
                                     skos:definition """This phase builds and tests the production solution to the point where it is ready for use in the \"live\" environment. The outputs of the \"Design\" phase direct the selection of reusable processes, instruments, information, and services that are assembled and configured in this phase to create the complete operational environment to run the process. New services are built by exception, created in response to gaps in the existing catalogue of services sourced from within the organisation and externally. These new services are constructed to be broadly reusable within the statistical production architecture.
For statistical outputs produced on a regular basis, this phase usually occurs for the first iteration, and following a review or a change in methodology or technology, rather than for every iteration.
It is broken down into seven sub-processes, which are generally sequential, from left to right, but can also occur in parallel, and can be iterative. These sub-processes are:
"""@en ;
                                     skos:inScheme igsbpm:GSBPM ;
                                     skos:narrower <http://id.unece.org/models/gsbpm/3.1> ,
                                                   <http://id.unece.org/models/gsbpm/3.2> ,
                                                   <http://id.unece.org/models/gsbpm/3.3> ,
                                                   <http://id.unece.org/models/gsbpm/3.4> ,
                                                   <http://id.unece.org/models/gsbpm/3.5> ,
                                                   <http://id.unece.org/models/gsbpm/3.6> ,
                                                   <http://id.unece.org/models/gsbpm/3.7> ;
                                     skos:notation "3" ;
                                     skos:prefLabel "Build"@en ;
                                     skos:topConceptOf igsbpm:GSBPM .


###  http://id.unece.org/models/gsbpm/3.1
<http://id.unece.org/models/gsbpm/3.1> rdf:type owl:NamedIndividual ,
                                                gsbpm:SubProcess ;
                                       skos:broader <http://id.unece.org/models/gsbpm/3> ;
                                       skos:definition """This sub-process describes the activities to build the collection instruments to be used during the \"Collect\" phase. The collection instrument is generated or built based on the design specifications created during the \"Design\" phase. A collection may use one or more modes to receive the data, e.g. personal or telephone interviews; paper, electronic or web questionnaires; SDMX hubs. Collection instruments may also be data extraction routines used to gather data from existing statistical or administrative data sets. This sub-process also includes preparing and testing the contents and functioning of that instrument (e.g. testing the questions in a questionnaire). It is recommended to consider the direct connection of collection instruments to the statistical metadata system, so that metadata can be more easily captured in the collection phase. Connection of metadata and data at the point of capture can save work in later phases. Capturing the metrics of data collection (paradata) is also an important consideration in this sub-process.
"""@en ;
                                       skos:inScheme igsbpm:GSBPM ;
                                       skos:notation "3.1" ;
                                       skos:prefLabel "Build collection instrument"@en .


###  http://id.unece.org/models/gsbpm/3.2
<http://id.unece.org/models/gsbpm/3.2> rdf:type owl:NamedIndividual ,
                                                gsbpm:SubProcess ;
                                       skos:broader <http://id.unece.org/models/gsbpm/3> ;
                                       skos:definition """This sub-process describes the activities to build new and enhance existing components and services needed for the \"Process\" and \"Analyse\" phases, as designed in the \"Design\" phase. Services may include dashboard functions and features, information services, transformation functions, workflow frameworks, provider and metadata management services.
"""@en ;
                                       skos:inScheme igsbpm:GSBPM ;
                                       skos:notation "3.2" ;
                                       skos:prefLabel "Build or enhance process components"@en .


###  http://id.unece.org/models/gsbpm/3.3
<http://id.unece.org/models/gsbpm/3.3> rdf:type owl:NamedIndividual ,
                                                gsbpm:SubProcess ;
                                       skos:broader <http://id.unece.org/models/gsbpm/3> ;
                                       skos:definition """This sub-process describes the activities to build new and enhance existing components and services needed for the dissemination of statistical products as designed in sub-process 2.1 (Design outputs). All types of dissemination components and services are included, from those that are used to produce traditional paper publications to those that provide web services, open data outputs, or access to micro-data.
"""@en ;
                                       skos:inScheme igsbpm:GSBPM ;
                                       skos:notation "3.3" ;
                                       skos:prefLabel "Build or enhance dissemination components"@en .


###  http://id.unece.org/models/gsbpm/3.4
<http://id.unece.org/models/gsbpm/3.4> rdf:type owl:NamedIndividual ,
                                                gsbpm:SubProcess ;
                                       skos:broader <http://id.unece.org/models/gsbpm/3> ;
                                       skos:definition """This sub-process configures the workflow, systems and transformations used within the statistical business processes, from data collection through to dissemination. It ensures that the workflow specified in sub-process 2.6 (Design production systems and workflow) works in practice.
"""@en ;
                                       skos:inScheme igsbpm:GSBPM ;
                                       skos:notation "3.4" ;
                                       skos:prefLabel "Configure workflows"@en .


###  http://id.unece.org/models/gsbpm/3.5
<http://id.unece.org/models/gsbpm/3.5> rdf:type owl:NamedIndividual ,
                                                gsbpm:SubProcess ;
                                       skos:broader <http://id.unece.org/models/gsbpm/3> ;
                                       skos:definition """This sub-process is concerned with the testing of assembled and configured services and related workflows. It includes technical testing and sign-off of new programmes and routines, as well as confirmation that existing routines from other statistical business processes are suitable for use in this case. Whilst part of this activity concerning the testing of individual components and services could logically be linked with sub-process 3.2 (Build or enhance process components), this sub-process also includes testing of interactions between assembled and configured services, and ensuring that the production solution works as a coherent set processes, information and services.
"""@en ;
                                       skos:inScheme igsbpm:GSBPM ;
                                       skos:notation "3.5" ;
                                       skos:prefLabel "Test production system"@en .


###  http://id.unece.org/models/gsbpm/3.6
<http://id.unece.org/models/gsbpm/3.6> rdf:type owl:NamedIndividual ,
                                                gsbpm:SubProcess ;
                                       skos:broader <http://id.unece.org/models/gsbpm/3> ;
                                       skos:definition """This sub-process describes the activities to manage a field test or pilot of the statistical business process. Typically it includes a small-scale data collection, to test collection instruments, followed by processing and analysis of the collected data, to ensure the statistical business process performs as expected. Following the pilot, it may be necessary to go back to a previous step and make adjustments to instruments, systems or components. For a major statistical business process, e.g. a population census, there may be several iterations until the process is working satisfactorily.
"""@en ;
                                       skos:inScheme igsbpm:GSBPM ;
                                       skos:notation "3.6" ;
                                       skos:prefLabel "Test statistical business process"@en .


###  http://id.unece.org/models/gsbpm/3.7
<http://id.unece.org/models/gsbpm/3.7> rdf:type owl:NamedIndividual ,
                                                gsbpm:SubProcess ;
                                       skos:broader <http://id.unece.org/models/gsbpm/3> ;
                                       skos:definition """This sub-process includes the activities to put the assembled and configured processes and services, including modified and newly-created services into production ready for use by business areas. The activities include:
- producing documentation about the process components, including technical documentation and user manuals
- training the business users on how to operate the process
- moving the process components into the production environment, and ensuring they work as expected in that environment (this activity may also be part of sub-process 3.5 (Test production system)).
"""@en ;
                                       skos:inScheme igsbpm:GSBPM ;
                                       skos:notation "3.7" ;
                                       skos:prefLabel "Finalise production systems"@en .


###  http://id.unece.org/models/gsbpm/4
<http://id.unece.org/models/gsbpm/4> rdf:type owl:NamedIndividual ,
                                              gsbpm:Phase ;
                                     skos:definition """This phase collects or gathers all necessary information (data and metadata), using different collection modes (including extractions from statistical, administrative and other non-statistical registers and databases), and loads them into the appropriate environment for further processing. Whilst it can include validation of data set formats, it does not include any transformations of the data themselves, as these are all done in the \"Process\" phase. For statistical outputs produced regularly, this phase occurs in each iteration.
The \"Collect\" phase is broken down into four sub-processes, which are generally sequential, from left to right, but can also occur in parallel, and can be iterative. These sub-processes are:
"""@en ;
                                     skos:inScheme igsbpm:GSBPM ;
                                     skos:narrower <http://id.unece.org/models/gsbpm/4.1> ,
                                                   <http://id.unece.org/models/gsbpm/4.2> ,
                                                   <http://id.unece.org/models/gsbpm/4.3> ,
                                                   <http://id.unece.org/models/gsbpm/4.4> ;
                                     skos:notation "4" ;
                                     skos:prefLabel "Collect"@en ;
                                     skos:topConceptOf igsbpm:GSBPM .


###  http://id.unece.org/models/gsbpm/4.1
<http://id.unece.org/models/gsbpm/4.1> rdf:type owl:NamedIndividual ,
                                                gsbpm:SubProcess ;
                                       skos:broader <http://id.unece.org/models/gsbpm/4> ;
                                       skos:definition """This sub-process establishes the frame and selects the sample for this iteration of the collection, as specified in sub-process 2.4 (Design frame and sample). It also includes the coordination of samples between instances of the same statistical business process (for example to manage overlap or rotation), and between different processes using a common frame or register (for example to manage overlap or to spread response burden). Quality assurance and approval of the frame and the selected sample are also undertaken in this sub-process, though maintenance of underlying registers, from which frames for several statistical business processes are drawn, is treated as a separate business process. The sampling aspect of this sub-process is not usually relevant for processes based entirely on the use of pre-existing sources (e.g. administrative sources) as such processes generally create frames from the available data and then follow a census approach.
"""@en ;
                                       skos:inScheme igsbpm:GSBPM ;
                                       skos:notation "4.1" ;
                                       skos:prefLabel "Create frame and select sample"@en .


###  http://id.unece.org/models/gsbpm/4.2
<http://id.unece.org/models/gsbpm/4.2> rdf:type owl:NamedIndividual ,
                                                gsbpm:SubProcess ;
                                       skos:broader <http://id.unece.org/models/gsbpm/4> ;
                                       skos:definition """This sub-process ensures that the people, processes and technology are ready to collect data and metadata, in all modes as designed. It takes place over a period of time, as it includes the strategy, planning and training activities in preparation for the specific instance of the statistical business process. Where the process is repeated regularly, some (or all) of these activities may not be explicitly required for each iteration. For one-off and new processes, these activities can be lengthy. This sub-process includes:
- preparing a collection strategy;
- training collection staff;
- ensuring collection resources are available e.g. laptops;
- agreeing terms with any intermediate collection bodies, e.g. sub-contractors for computer assisted telephone interviewing
- configuring collection systems to request and receive the data;
- ensuring the security of data to be collected;
- preparing collection instruments (e.g. printing questionnaires, pre-filling them with existing data, loading questionnaires and data onto interviewers' computers etc.).
For non-survey sources, this sub-process will include ensuring that the necessary processes, systems and confidentiality procedures are in place, to receive or extract the necessary information from the source.
"""@en ;
                                       skos:inScheme igsbpm:GSBPM ;
                                       skos:notation "4.2" ;
                                       skos:prefLabel "Set up collection"@en .


###  http://id.unece.org/models/gsbpm/4.3
<http://id.unece.org/models/gsbpm/4.3> rdf:type owl:NamedIndividual ,
                                                gsbpm:SubProcess ;
                                       skos:broader <http://id.unece.org/models/gsbpm/4> ;
                                       skos:definition """This sub-process is where the collection is implemented, with the different instruments being used to collect or gather the information, which may include raw micro-data or aggregates produced at the source, as well as any associated metadata. It includes the initial contact with providers and any subsequent follow-up or reminder actions. It may include manual data entry at the point of contact, or fieldwork management, depending on the source and collection mode. It records when and how providers were contacted, and whether they have responded. This sub-process also includes the management of the providers involved in the current collection, ensuring that the relationship between the statistical organisation and data providers remains positive, and recording and responding to comments, queries and complaints. For administrative and other non-statistical sources, this process is brief: the provider is either contacted to send the information, or sends it as scheduled. When the collection meets its targets, it is closed and a report on the collection is produced. Some basic validation of the structure and integrity of the information received may take place within this sub-process, e.g. checking that files are in the right format and contain the expected fields. All validation of the content takes place in the Process phase.
"""@en ;
                                       skos:inScheme igsbpm:GSBPM ;
                                       skos:notation "4.3" ;
                                       skos:prefLabel "Run collection"@en .


###  http://id.unece.org/models/gsbpm/4.4
<http://id.unece.org/models/gsbpm/4.4> rdf:type owl:NamedIndividual ,
                                                gsbpm:SubProcess ;
                                       skos:broader <http://id.unece.org/models/gsbpm/4> ;
                                       skos:definition """This sub-process includes loading the collected data and metadata into a suitable electronic environment for further processing. It may include manual or automatic data take-on, for example using clerical staff or optical character recognition tools to extract information from paper questionnaires, or converting the formats of files received from other organisations. It may also include analysis of the process metadata (paradata) associated with collection to ensure the collection activities have met requirements. In cases where there is a physical collection instrument, such as a paper questionnaire, which is not needed for further processing, this sub-process manages the archiving of that material.
"""@en ;
                                       skos:inScheme igsbpm:GSBPM ;
                                       skos:notation "4.4" ;
                                       skos:prefLabel "Finalise collection"@en .


###  http://id.unece.org/models/gsbpm/5
<http://id.unece.org/models/gsbpm/5> rdf:type owl:NamedIndividual ,
                                              gsbpm:Phase ;
                                     skos:definition """This phase describes the cleaning of data and their preparation for analysis. It is made up of sub-processes that check, clean, and transform input data, so that they can be analysed and disseminated as statistical outputs. It may be repeated several times if necessary. For statistical outputs produced regularly, this phase occurs in each iteration. The sub-processes in this phase can apply to data from both statistical and non-statistical sources (with the possible exception of sub-process 5.6 (Calculate weights), which is usually specific to survey data).
The \"Process\" and \"Analyse\" phases can be iterative and parallel. Analysis can reveal a broader understanding of the data, which might make it apparent that additional processing is needed. Activities within the \"Process\" and \"Analyse\" phases may commence before the \"Collect\" phase is completed. This enables the compilation of provisional results where timeliness is an important concern for users, and increases the time available for analysis.
This phase is broken down into eight sub-processes, which may be sequential, from left to right, but can also occur in parallel, and can be iterative. These sub-processes are:
"""@en ;
                                     skos:inScheme igsbpm:GSBPM ;
                                     skos:narrower <http://id.unece.org/models/gsbpm/5.1> ,
                                                   <http://id.unece.org/models/gsbpm/5.2> ,
                                                   <http://id.unece.org/models/gsbpm/5.3> ,
                                                   <http://id.unece.org/models/gsbpm/5.4> ,
                                                   <http://id.unece.org/models/gsbpm/5.5> ,
                                                   <http://id.unece.org/models/gsbpm/5.6> ,
                                                   <http://id.unece.org/models/gsbpm/5.7> ,
                                                   <http://id.unece.org/models/gsbpm/5.8> ;
                                     skos:notation "5" ;
                                     skos:prefLabel "Process"@en ;
                                     skos:topConceptOf igsbpm:GSBPM .


###  http://id.unece.org/models/gsbpm/5.1
<http://id.unece.org/models/gsbpm/5.1> rdf:type owl:NamedIndividual ,
                                                gsbpm:SubProcess ;
                                       skos:broader <http://id.unece.org/models/gsbpm/5> ;
                                       skos:definition """This sub-process integrates data from one or more sources. It is where the results of sub-processes in the \"Collect\" phase are combined. The input data can be from a mixture of external or internal data sources, and a variety of collection modes, including extracts of administrative data. The result is a set of linked data. Data integration can include:
- combining data from multiple sources, as part of the creation of integrated statistics such as national accounts
- matching / record linkage routines, with the aim of linking micro or macro data from different sources
- prioritising, when two or more sources contain data for the same variable, with potentially different values
Data integration may take place at any point in this phase, before or after any of the other sub-processes. There may also be several instances of data integration in any statistical business process. Following integration, depending on data protection requirements, data may be anonymised, that is stripped of identifiers such as name and address, to help to protect confidentiality.
"""@en ;
                                       skos:inScheme igsbpm:GSBPM ;
                                       skos:notation "5.1" ;
                                       skos:prefLabel "Integrate data"@en .


###  http://id.unece.org/models/gsbpm/5.2
<http://id.unece.org/models/gsbpm/5.2> rdf:type owl:NamedIndividual ,
                                                gsbpm:SubProcess ;
                                       skos:broader <http://id.unece.org/models/gsbpm/5> ;
                                       skos:definition """This sub-process classifies and codes the input data. For example automatic (or clerical) coding routines may assign numeric codes to text responses according to a pre-determined classification scheme.
"""@en ;
                                       skos:inScheme igsbpm:GSBPM ;
                                       skos:notation "5.2" ;
                                       skos:prefLabel "Classify and code"@en .


###  http://id.unece.org/models/gsbpm/5.3
<http://id.unece.org/models/gsbpm/5.3> rdf:type owl:NamedIndividual ,
                                                gsbpm:SubProcess ;
                                       skos:broader <http://id.unece.org/models/gsbpm/5> ;
                                       skos:definition """This sub-process examines data to try to identify potential problems, errors and discrepancies such as outliers, item non-response and miscoding. It can also be referred to as input data validation. It may be run iteratively, validating data against predefined edit rules, usually in a set order. It may flag data for automatic or manual inspection or editing. Reviewing and validating can apply to data from any type of source, before and after integration. Whilst validation is treated as part of the \"Process\" phase, in practice, some elements of validation may occur alongside collection activities, particularly for modes such as web collection. Whilst this sub-process is concerned with detection of actual or potential errors, any correction activities that actually change the data are done in sub-process 5.4.
"""@en ;
                                       skos:inScheme igsbpm:GSBPM ;
                                       skos:notation "5.3" ;
                                       skos:prefLabel "Review and validate"@en .


###  http://id.unece.org/models/gsbpm/5.4
<http://id.unece.org/models/gsbpm/5.4> rdf:type owl:NamedIndividual ,
                                                gsbpm:SubProcess ;
                                       skos:broader <http://id.unece.org/models/gsbpm/5> ;
                                       skos:definition """Where data are considered incorrect, missing or unreliable, new values may be inserted in this sub-process. The terms editing and imputation cover a variety of methods to do this, often using a rule-based approach. Specific steps typically include:
- the determination of whether to add or change data;
- the selection of the method to be used;
- adding / changing data values;
- writing the new data values back to the data set, and flagging them as changed;
- the production of metadata on the editing and imputation process.
"""@en ;
                                       skos:inScheme igsbpm:GSBPM ;
                                       skos:notation "5.4" ;
                                       skos:prefLabel "Edit and impute"@en .


###  http://id.unece.org/models/gsbpm/5.5
<http://id.unece.org/models/gsbpm/5.5> rdf:type owl:NamedIndividual ,
                                                gsbpm:SubProcess ;
                                       skos:broader <http://id.unece.org/models/gsbpm/5> ;
                                       skos:definition """This sub-process derives data for variables and units that are not explicitly provided in the collection, but are needed to deliver the required outputs. It derives new variables by applying arithmetic formulae to one or more of the variables that are already present in the dataset, or applying different model assumptions. This activity may need to be iterative, as some derived variables may themselves be based on other derived variables. It is therefore important to ensure that variables are derived in the correct order. New units may be derived by aggregating or splitting data for collection units, or by various other estimation methods. Examples include deriving households where the collection units are persons, or enterprises where the collection units are legal units.
"""@en ;
                                       skos:inScheme igsbpm:GSBPM ;
                                       skos:notation "5.5" ;
                                       skos:prefLabel "Derive new variables and units"@en .


###  http://id.unece.org/models/gsbpm/5.6
<http://id.unece.org/models/gsbpm/5.6> rdf:type owl:NamedIndividual ,
                                                gsbpm:SubProcess ;
                                       skos:broader <http://id.unece.org/models/gsbpm/5> ;
                                       skos:definition """This sub process creates weights for unit data records according to the methodology created in sub-process 2.5 (Design processing and analysis). In the case of sample surveys, weights can be used to \"gross-up\" results to make them representative of the target population, or to adjust for non-response in total enumerations. In other situations, variables may need weighting for normalisation purposes.
"""@en ;
                                       skos:inScheme igsbpm:GSBPM ;
                                       skos:notation "5.6" ;
                                       skos:prefLabel "Calculate weights"@en .


###  http://id.unece.org/models/gsbpm/5.7
<http://id.unece.org/models/gsbpm/5.7> rdf:type owl:NamedIndividual ,
                                                gsbpm:SubProcess ;
                                       skos:broader <http://id.unece.org/models/gsbpm/5> ;
                                       skos:definition """This sub process creates aggregate data and population totals from micro-data or lower-level aggregates. It includes summing data for records sharing certain characteristics, determining measures of average and dispersion, and applying weights from sub-process 5.6 to derive appropriate totals. In the case of sample surveys, sampling errors may also be calculated in this sub-process, and associated to the relevant aggregates.
"""@en ;
                                       skos:inScheme igsbpm:GSBPM ;
                                       skos:notation "5.7" ;
                                       skos:prefLabel "Calculate aggregates"@en .


###  http://id.unece.org/models/gsbpm/5.8
<http://id.unece.org/models/gsbpm/5.8> rdf:type owl:NamedIndividual ,
                                                gsbpm:SubProcess ;
                                       skos:broader <http://id.unece.org/models/gsbpm/5> ;
                                       skos:definition """This sub-process brings together the results of the other sub-processes in this phase and results in a data file (usually of macro-data), which is used as the input to the \"Analyse\" phase. Sometimes this may be an intermediate rather than a final file, particularly for business processes where there are strong time pressures, and a requirement to produce both preliminary and final estimates.
"""@en ;
                                       skos:inScheme igsbpm:GSBPM ;
                                       skos:notation "5.8" ;
                                       skos:prefLabel "Finalise data files"@en .


###  http://id.unece.org/models/gsbpm/6
<http://id.unece.org/models/gsbpm/6> rdf:type owl:NamedIndividual ,
                                              gsbpm:Phase ;
                                     skos:definition """In this phase, statistical outputs are produced, examined in detail and made ready for dissemination. It includes preparing statistical content (including commentary, technical notes, etc.), and ensuring outputs are \"fit for purpose\" prior to dissemination to customers. This phase also includes the sub-processes and activities that enable statistical analysts to understand the statistics produced. For statistical outputs produced regularly, this phase occurs in every iteration. The \"Analyse\" phase and sub-processes are generic for all statistical outputs, regardless of how the data were sourced.
The \"Analyse\" phase is broken down into five sub-processes, which are generally sequential, from left to right, but can also occur in parallel, and can be iterative. The sub-processes are:
"""@en ;
                                     skos:inScheme igsbpm:GSBPM ;
                                     skos:narrower <http://id.unece.org/models/gsbpm/6.1> ,
                                                   <http://id.unece.org/models/gsbpm/6.2> ,
                                                   <http://id.unece.org/models/gsbpm/6.3> ,
                                                   <http://id.unece.org/models/gsbpm/6.4> ,
                                                   <http://id.unece.org/models/gsbpm/6.5> ;
                                     skos:notation "6" ;
                                     skos:prefLabel "Analyse"@en ;
                                     skos:topConceptOf igsbpm:GSBPM .


###  http://id.unece.org/models/gsbpm/6.1
<http://id.unece.org/models/gsbpm/6.1> rdf:type owl:NamedIndividual ,
                                                gsbpm:SubProcess ;
                                       skos:broader <http://id.unece.org/models/gsbpm/6> ;
                                       skos:definition """This sub-process is where the data are transformed into statistical outputs. It includes the production of additional measurements such as indices, trends or seasonally adjusted series, as well as the recording of quality characteristics.
"""@en ;
                                       skos:inScheme igsbpm:GSBPM ;
                                       skos:notation "6.1" ;
                                       skos:prefLabel "Prepare draft outputs"@en .


###  http://id.unece.org/models/gsbpm/6.2
<http://id.unece.org/models/gsbpm/6.2> rdf:type owl:NamedIndividual ,
                                                gsbpm:SubProcess ;
                                       skos:broader <http://id.unece.org/models/gsbpm/6> ;
                                       skos:definition """This sub-process is where statisticians validate the quality of the outputs produced, in accordance with a general quality framework and with expectations. This sub-process also includes activities involved with the gathering of intelligence, with the cumulative effect of building up a body of knowledge about a specific statistical domain. This knowledge is then applied to the current collection, in the current environment, to identify any divergence from expectations and to allow informed analyses. Validation activities can include:
- checking that the population coverage and response rates are as required;
- comparing the statistics with previous cycles (if applicable);
- checking that the associated metadata and paradata (process metadata) are present and in line with expectations
- confronting the statistics against other relevant data (both internal and external);
- investigating inconsistencies in the statistics;
- performing macro editing;
- validating the statistics against expectations and domain intelligence.
"""@en ;
                                       skos:inScheme igsbpm:GSBPM ;
                                       skos:notation "6.2" ;
                                       skos:prefLabel "Validate outputs"@en .


###  http://id.unece.org/models/gsbpm/6.3
<http://id.unece.org/models/gsbpm/6.3> rdf:type owl:NamedIndividual ,
                                                gsbpm:SubProcess ;
                                       skos:broader <http://id.unece.org/models/gsbpm/6> ;
                                       skos:definition """This sub-process is where the in-depth understanding of the outputs is gained by statisticians. They use that understanding to interpret and explain the statistics produced for this cycle by assessing how well the statistics reflect their initial expectations, viewing the statistics from all perspectives using different tools and media, and carrying out in-depth statistical analyses.
"""@en ;
                                       skos:inScheme igsbpm:GSBPM ;
                                       skos:notation "6.3" ;
                                       skos:prefLabel "Interpret and explain outputs"@en .


###  http://id.unece.org/models/gsbpm/6.4
<http://id.unece.org/models/gsbpm/6.4> rdf:type owl:NamedIndividual ,
                                                gsbpm:SubProcess ;
                                       skos:broader <http://id.unece.org/models/gsbpm/6> ;
                                       skos:definition """This sub-process ensures that the data (and metadata) to be disseminated do not breach the appropriate rules on confidentiality. This may include checks for primary and secondary disclosure, as well as the application of data suppression or perturbation techniques. The degree and method of disclosure control may vary for different types of outputs, for example the approach used for micro-data sets for research purposes will be different to that for published tables or maps.
"""@en ;
                                       skos:inScheme igsbpm:GSBPM ;
                                       skos:notation "6.4" ;
                                       skos:prefLabel "Apply disclosure control"@en .


###  http://id.unece.org/models/gsbpm/6.5
<http://id.unece.org/models/gsbpm/6.5> rdf:type owl:NamedIndividual ,
                                                gsbpm:SubProcess ;
                                       skos:broader <http://id.unece.org/models/gsbpm/6> ;
                                       skos:definition """This sub-process ensures the statistics and associated information are fit for purpose and reach the required quality level, and are thus ready for use. It includes:
- completing consistency checks;
- determining the level of release, and applying caveats;
- collating supporting information, including interpretation, commentary, technical notes, briefings, measures of uncertainty and any other necessary metadata;
- producing the supporting internal documents;
- pre-release discussion with appropriate internal subject matter experts;
- approving the statistical content for release.
"""@en ;
                                       skos:inScheme igsbpm:GSBPM ;
                                       skos:notation "6.5" ;
                                       skos:prefLabel "Finalise outputs"@en .


###  http://id.unece.org/models/gsbpm/7
<http://id.unece.org/models/gsbpm/7> rdf:type owl:NamedIndividual ,
                                              gsbpm:Phase ;
                                     skos:definition """This phase manages the release of the statistical products to customers. It includes all activities associated with assembling and releasing a range of static and dynamic products via a range of channels. These activities support customers to access and use the outputs released by the statistical organisation.
For statistical outputs produced regularly, this phase occurs in each iteration. It is made up of five sub-processes, which are generally sequential, from left to right, but can also occur in parallel, and can be iterative. These sub-processes are:
"""@en ;
                                     skos:inScheme igsbpm:GSBPM ;
                                     skos:narrower <http://id.unece.org/models/gsbpm/7.1> ,
                                                   <http://id.unece.org/models/gsbpm/7.2> ,
                                                   <http://id.unece.org/models/gsbpm/7.3> ,
                                                   <http://id.unece.org/models/gsbpm/7.4> ,
                                                   <http://id.unece.org/models/gsbpm/7.5> ;
                                     skos:notation "7" ;
                                     skos:prefLabel "Disseminate"@en ;
                                     skos:topConceptOf igsbpm:GSBPM .


###  http://id.unece.org/models/gsbpm/7.1
<http://id.unece.org/models/gsbpm/7.1> rdf:type owl:NamedIndividual ,
                                                gsbpm:SubProcess ;
                                       skos:broader <http://id.unece.org/models/gsbpm/7> ;
                                       skos:definition """This sub-process manages the update of systems where data and metadata are stored ready for dissemination purposes, including:
- formatting data and metadata ready to be put into output databases;
- loading data and metadata into output databases;
- ensuring data are linked to the relevant metadata.
Formatting, loading and linking of metadata should preferably mostly take place in earlier phases, but this sub-process includes a final check that all of the necessary metadata are in place ready for dissemination.
"""@en ;
                                       skos:inScheme igsbpm:GSBPM ;
                                       skos:notation "7.1" ;
                                       skos:prefLabel "Update output systems"@en .


###  http://id.unece.org/models/gsbpm/7.2
<http://id.unece.org/models/gsbpm/7.2> rdf:type owl:NamedIndividual ,
                                                gsbpm:SubProcess ;
                                       skos:broader <http://id.unece.org/models/gsbpm/7> ;
                                       skos:definition """This sub-process produces the products, as previously designed (in sub-process 2.1), to meet user needs. They could include printed publications, press releases and web sites. The products can take many forms including interactive graphics, tables, public-use micro-data sets and downloadable files. Typical steps include:
- preparing the product components (explanatory text, tables, charts, quality statements etc.);
- assembling the components into products;
- editing the products and checking that they meet publication standards.
"""@en ;
                                       skos:inScheme igsbpm:GSBPM ;
                                       skos:notation "7.2" ;
                                       skos:prefLabel "Produce dissemination products"@en .


###  http://id.unece.org/models/gsbpm/7.3
<http://id.unece.org/models/gsbpm/7.3> rdf:type owl:NamedIndividual ,
                                                gsbpm:SubProcess ;
                                       skos:broader <http://id.unece.org/models/gsbpm/7> ;
                                       skos:definition """This sub-process ensures that all elements for the release are in place including managing the timing of the release. It includes briefings for specific groups such as the press or ministers, as well as the arrangements for any pre-release embargoes. It also includes the provision of products to subscribers, and managing access to confidential data by authorised user groups, such as researchers. Sometimes an organisation may need to retract a product, for example if an error is discovered. This is also included in this sub-process.
"""@en ;
                                       skos:inScheme igsbpm:GSBPM ;
                                       skos:notation "7.3" ;
                                       skos:prefLabel "Manage release of dissemination products"@en .


###  http://id.unece.org/models/gsbpm/7.4
<http://id.unece.org/models/gsbpm/7.4> rdf:type owl:NamedIndividual ,
                                                gsbpm:SubProcess ;
                                       skos:broader <http://id.unece.org/models/gsbpm/7> ;
                                       skos:definition """Whilst marketing in general can be considered to be an over-arching process, this sub-process concerns the active promotion of the statistical products produced in a specific statistical business process, to help them reach the widest possible audience. It includes the use of customer relationship management tools, to better target potential users of the products, as well as the use of tools including web sites, wikis and blogs to facilitate the process of communicating statistical information to users.
"""@en ;
                                       skos:inScheme igsbpm:GSBPM ;
                                       skos:notation "7.4" ;
                                       skos:prefLabel "Promote dissemination products"@en .


###  http://id.unece.org/models/gsbpm/7.5
<http://id.unece.org/models/gsbpm/7.5> rdf:type owl:NamedIndividual ,
                                                gsbpm:SubProcess ;
                                       skos:broader <http://id.unece.org/models/gsbpm/7> ;
                                       skos:definition """This sub-process ensures that customer queries and requests for services such as micro-data access are recorded, and that responses are provided within agreed deadlines. These queries and requests should be regularly reviewed to provide an input to the over-arching quality management process, as they can indicate new or changing user needs.
"""@en ;
                                       skos:inScheme igsbpm:GSBPM ;
                                       skos:notation "7.5" ;
                                       skos:prefLabel "Manage user support"@en .


###  http://id.unece.org/models/gsbpm/8
<http://id.unece.org/models/gsbpm/8> rdf:type owl:NamedIndividual ,
                                              gsbpm:Phase ;
                                     skos:definition """This phase manages the evaluation of a specific instance of a statistical business process, as opposed to the more general over-arching process of statistical quality management described in Section VI. It logically takes place at the end of the instance of the process, but relies on inputs gathered throughout the different phases. It includes evaluating the success of a specific instance of the statistical business process, drawing on a range of quantitative and qualitative inputs, and identifying and prioritising potential improvements.
For statistical outputs produced regularly, evaluation should, at least in theory occur for each iteration, determining whether future iterations should take place, and if so, whether any improvements should be implemented. However, in some cases, particularly for regular and well established statistical business processes, evaluation may not be formally carried out for each iteration. In such cases, this phase can be seen as providing the decision as to whether the next iteration should start from the Specify Needs phase, or from some later phase (often the Collect phase).
This phase is made up of three sub-processes, which are generally sequential, from left to right, but which can overlap to some extent in practice. These sub-processes are:
"""@en ;
                                     skos:inScheme igsbpm:GSBPM ;
                                     skos:narrower <http://id.unece.org/models/gsbpm/8.1> ,
                                                   <http://id.unece.org/models/gsbpm/8.2> ,
                                                   <http://id.unece.org/models/gsbpm/8.3> ;
                                     skos:notation "8" ;
                                     skos:prefLabel "Evaluate"@en ;
                                     skos:topConceptOf igsbpm:GSBPM .


###  http://id.unece.org/models/gsbpm/8.1
<http://id.unece.org/models/gsbpm/8.1> rdf:type owl:NamedIndividual ,
                                                gsbpm:SubProcess ;
                                       skos:broader <http://id.unece.org/models/gsbpm/8> ;
                                       skos:definition """Evaluation material can be produced in any other phase or sub-process. It may take many forms, including feedback from users, process metadata (paradata), system metrics, and staff suggestions. Reports of progress against an action plan agreed during a previous iteration may also form an input to evaluations of subsequent iterations. This sub-process gathers all of these inputs, and makes them available for the person or team producing the evaluation.
"""@en ;
                                       skos:inScheme igsbpm:GSBPM ;
                                       skos:notation "8.1" ;
                                       skos:prefLabel "Gather evaluation inputs"@en .


###  http://id.unece.org/models/gsbpm/8.2
<http://id.unece.org/models/gsbpm/8.2> rdf:type owl:NamedIndividual ,
                                                gsbpm:SubProcess ;
                                       skos:broader <http://id.unece.org/models/gsbpm/8> ;
                                       skos:definition """This sub-process analyses the evaluation inputs and synthesises them into an evaluation report. The resulting report should note any quality issues specific to this iteration of the statistical business process, and should make recommendations for changes if appropriate. These recommendations can cover changes to any phase or sub-process for future iterations of the process, or can suggest that the process is not repeated.
"""@en ;
                                       skos:inScheme igsbpm:GSBPM ;
                                       skos:notation "8.2" ;
                                       skos:prefLabel "Conduct evaluation"@en .


###  http://id.unece.org/models/gsbpm/8.3
<http://id.unece.org/models/gsbpm/8.3> rdf:type owl:NamedIndividual ,
                                                gsbpm:SubProcess ;
                                       skos:broader <http://id.unece.org/models/gsbpm/8> ;
                                       skos:definition """This sub-process brings together the necessary decision-making power to form and agree an action plan based on the evaluation report. It should also include consideration of a mechanism for monitoring the impact of those actions, which may, in turn, provide an input to evaluations of future iterations of the process.
"""@en ;
                                       skos:inScheme igsbpm:GSBPM ;
                                       skos:notation "8.3" ;
                                       skos:prefLabel "Agree an action plan"@en .


###  https://www.bps.go.id/survey/population-census#PopulationCensusBusinessProcess2020ShortForm
id-ps:PopulationCensusBusinessProcess2020ShortForm rdf:type owl:NamedIndividual ,
                                                            :BusinessProcess ;
                                                   :hasBP-PS id-ps:SP2020DesignCollectionProcess ,
                                                             id-ps:SP2020DesignOutputProcess ,
                                                             id-ps:SP2020DesignProcessingAndAnalysisProcess ,
                                                             id-ps:SP2020DesignVariableDescriptionsProcess ;
                                                   rdfs:label "Population Census Business Process SP2020 Short Form"@en .


###  https://www.bps.go.id/survey/population-census#PopulationCensusProgram
id-ps:PopulationCensusProgram rdf:type owl:NamedIndividual ,
                                       :StatisticalProgram ;
                              :hasSP-SPC id-ps:PopulationCensusProgramCycle2010 ,
                                         id-ps:PopulationCensusProgramCycle2020 ,
                                         id-ps:PopulationCensusProgramCycle2020LongForm ;
                              :usesSP-SPD id-ps:SP2020DesignOutputStatisticalProgramDesign ;
                              gsim-sum:hasDateInitiated-SP "1961-10-01T00:00:00"^^xsd:dateTime ;
                              gsim-sum:hasDescription-IA "SP menyediakan data karakteristik pokok dan rinci terhadap seluruh penduduk baik yang bertempat tinggal tetap maupun yang tidak mempunyai tempat tinggal tetap (tuna wisma, anak buah kapal Indonesia, manusia/orang perahu, dan suku terasing). Sensus ini dilaksanakan sepuluh tahunan pada tahun berakhiran '0'." ;
                              gsim-sum:hasLegalFramework-SP """- Undang-Undang Nomor 16 tahun 1997 tentang Statistik; 
- Undang-Undang Nomor 23 tahun 2006 tentang Administrasi Kependudukan; 
- Undang-Undang Nomor 24 tahun 2013 tentang perubahan atas Undang-Undang Nomor 23 tahun 2006 tentang Administrasi Kependudukan; 
- Undang-Undang Nomor 52 tahun 2009 tentang Perkembangan Kependudukan dan Pembangunan Keluarga; 
- Peraturan Pemerintah Nomor 51 Tahun 1999 tentang Penyelenggaraan Statistik; 
- Peraturan Presiden Nomor 39 Tahun 2019 tentang Satu Data Indonesia.""" ;
                              gsim-sum:hasLegislativeReference-SN "Sebagaimana tertuang dalam Undang-Undang No. 16 Tahun 1997 tentang Statistik, Badan Pusat Statistik (BPS) diamanatkan untuk melaksanakan sensus penduduk sekurang-kurangnya sekali dalam sepuluh tahun." ;
                              gsim-sum:hasName-IA "Sensus Penduduk" ;
                              gsim-sum:hasStatus-SP "Active" ;
                              gsim-sum:hasValue-IA """History: 
Dalam perjalanannya, sensus penduduk di Indonesia sudah dilaksanakan sebanyak tujuh kali sejak Indonesia merdeka, yaitu pada tahun 1961, 1971, 1980, 1990, 2000, 2010, dan 2020.

Benefit:
Tersedianya data jumlah, komposisi, distribusi, dan karakteristik penduduk Indonesia.

Objective2:
(1) Mengumpulkan dan menyajikan data dasar kependudukan sampai wilayah administrasi terkecil.; 
(2) Membentuk Kerangka Sampel Induk (KSI) untuk kepentingan survei-survei lain yang dilakukan dengan pendekatan rumah tangga. ; 
(3) Memperkirakan berbagai parameter kependudukan sampai wilayah administrasi tertentu.; 
(4) Mengumpulkan informasi kependudukan yang dapat digunakan/dimanfaatkan untuk penyusunan basis data kependudukan.""" ;
                              rdfs:label "Population Census Program"@en .


###  https://www.bps.go.id/survey/population-census#PopulationCensusProgramCycle2010
id-ps:PopulationCensusProgramCycle2010 rdf:type owl:NamedIndividual ,
                                                :StatisticalProgramCycle ;
                                       gsim-sum:hasReferencePeriodEnd-SPC "2012-12-31T00:00:00"^^xsd:dateTime ;
                                       gsim-sum:hasReferencePeriodStart-SPC "2007-01-01T00:00:00"^^xsd:dateTime ;
                                       rdfs:label "Population Census Program Cycle 2010 (SP2010)"@en .


###  https://www.bps.go.id/survey/population-census#PopulationCensusProgramCycle2020
id-ps:PopulationCensusProgramCycle2020 rdf:type owl:NamedIndividual ,
                                                :StatisticalProgramCycle ;
                                       :includesSPC-BP id-ps:PopulationCensusBusinessProcess2020ShortForm ;
                                       gsim-sum:hasReferencePeriodEnd-SPC "2021-01-21T00:00:00"^^xsd:dateTime ;
                                       gsim-sum:hasReferencePeriodStart-SPC "2018-01-01T00:00:00"^^xsd:dateTime ;
                                       rdfs:label "Population Census Program Cycle 2020 (SP2020 Short Form)"@en .


###  https://www.bps.go.id/survey/population-census#PopulationCensusProgramCycle2020LongForm
id-ps:PopulationCensusProgramCycle2020LongForm rdf:type owl:NamedIndividual ,
                                                        :StatisticalProgramCycle ;
                                               gsim-sum:hasReferencePeriodEnd-SPC "2023-12-31T00:00:00"^^xsd:dateTime ;
                                               gsim-sum:hasReferencePeriodStart-SPC "2021-01-01T00:00:00"^^xsd:dateTime ;
                                               rdfs:label "Population Census Program Cycle 2020 Long Form (SP2020 Long Form)"@en .


###  https://www.bps.go.id/survey/population-census#SP2020DesignCollectionProcess
id-ps:SP2020DesignCollectionProcess rdf:type owl:NamedIndividual ,
                                             :ProcessStep ;
                                    :createsPS-PO id-ps:SP2020DesignCollectionProcessCoreOutput ,
                                                  id-ps:SP2020DesignCollectionProcessExecutionLog ;
                                    :hasPS-PI id-ps:SP2020DesignCollectionProcessCoreInput ;
                                    :hasEndTime-PS "2018-09-12T00:00:00"^^xsd:dateTime ;
                                    :hasStartTime-PS "2018-08-01T00:00:00"^^xsd:dateTime ;
                                    rdfs:label "SP2020 - Design Collection - Process"@en .


###  https://www.bps.go.id/survey/population-census#SP2020DesignCollectionProcessControlDesign
id-ps:SP2020DesignCollectionProcessControlDesign rdf:type owl:NamedIndividual ,
                                                          :ProcessControlDesign ;
                                                 gsim-sum:hasValue-IA """Has all the information from the business case and statistical program design been described in the collection method that will be produced?
- If no, go to back to the beginning of the Process Step and run again 
- If yes, go to the next Process Step""" ;
                                                 rdfs:label "SP2020 - Design Collection - Process Control Design"@en .


###  https://www.bps.go.id/survey/population-census#SP2020DesignCollectionProcessCoreInput
id-ps:SP2020DesignCollectionProcessCoreInput rdf:type owl:NamedIndividual ,
                                                      :CoreInput ;
                                             :correspondsToPI-PIS id-ps:SP2020DesignCollectionProcessInputSpecification ;
                                             :refersToCI-IA id-ps:SP2020DesignOutputBusinessCase ,
                                                            id-ps:SP2020DesignOutputStatisticalProgramDesign ;
                                             rdfs:label "SP2020 - Design Collection - Process Input (Core Input)"@en .


###  https://www.bps.go.id/survey/population-census#SP2020DesignCollectionProcessCoreOutput
id-ps:SP2020DesignCollectionProcessCoreOutput rdf:type owl:NamedIndividual ,
                                                       :CoreOutput ;
                                              :correspondsToPO-POS id-ps:SP2020DesignCollectionProcessOutputSpecification ;
                                              :refersToCO-IA id-ps:SP2020DesignCollectionProcessMethodCollection ;
                                              rdfs:label "SP2020 - Design Collection - Process Output (Core Output)"@en .


###  https://www.bps.go.id/survey/population-census#SP2020DesignCollectionProcessDesign
id-ps:SP2020DesignCollectionProcessDesign rdf:type owl:NamedIndividual ,
                                                   :ProcessDesign ;
                                          :classifiedAs <http://id.unece.org/models/gsbpm/3.2> ;
                                          :hasPD-PCD id-ps:SP2020DesignCollectionProcessControlDesign ;
                                          :hasPD-PIS id-ps:SP2020DesignCollectionProcessInputSpecification ;
                                          :hasPD-POS id-ps:SP2020DesignCollectionProcessOutputSpecification ;
                                          :implementsPD-PM id-ps:SP2020DesignCollectionProcessMethod ;
                                          :specifiesPD-PS id-ps:SP2020DesignCollectionProcess ;
                                          rdfs:label "SP2020 - Design Collection - Process Design"@en .


###  https://www.bps.go.id/survey/population-census#SP2020DesignCollectionProcessExecutionLog
id-ps:SP2020DesignCollectionProcessExecutionLog rdf:type owl:NamedIndividual ,
                                                         :ProcessExecutionLog ;
                                                gsim-sum:hasExecutionLog """- All information from the business case and statistical program design been described in the collection method
- There needs to be deeper testing of each collection mode
- There is a need to organize collection modes based on the characteristics of residents' residences, for example residents who live in apartments or condominiums.""" ;
                                                rdfs:label "SP2020 - Design Collection - Execution Log" .


###  https://www.bps.go.id/survey/population-census#SP2020DesignCollectionProcessInputSpecification
id-ps:SP2020DesignCollectionProcessInputSpecification rdf:type owl:NamedIndividual ,
                                                               :ProcessInputSpecification ;
                                                      :coreInputType "Business Case" ,
                                                                     "Statistical Program Design" ;
                                                      rdfs:label "SP2020 - Design Collection - Process Input Specification"@en .


###  https://www.bps.go.id/survey/population-census#SP2020DesignCollectionProcessMethod
id-ps:SP2020DesignCollectionProcessMethod rdf:type owl:NamedIndividual ,
                                                   :ProcessMethod ;
                                          gsim-sum:hasValue-IA """- Check the business case and statistical program design received
- Analyze requirement and review collection method from reference metadata
- Produce collection method""" ;
                                          rdfs:label "SP2020 - Design Collection - Process Method"@en .


###  https://www.bps.go.id/survey/population-census#SP2020DesignCollectionProcessMethodCollection
id-ps:SP2020DesignCollectionProcessMethodCollection rdf:type owl:NamedIndividual ,
                                                             :ProcessMethod ;
                                                    gsim-sum:hasName-IA "Desain Pengumpulan Data Sensus Penduduk" ;
                                                    gsim-sum:hasValue-IA """DOES CONDUCT OFFICER TRAINING
Yes

NUMBER OF Enumerators
208038

TYPE OF DATA COLLECTION AREA COVERAGE
All Indonesian Territory

DATA COLLECTION FREQUENCY
More than Two Years

MINIMUM EDUCATIONAL LEVEL OF OFFICERS
SMA/SMK


DATA COLLECTION MODE
Paper-Assisted Personal Interviewing (PAPI), Computer-Assisted Personal Interviewing (CAPI), Computer-Aided Web Interviewing (CAWI)

METHOD OF COLLECTING DATA
- Interview (PAPI)
- Data Input (CAPI)
- Data Input (CAWI)

DATA COLLECTION OFFICER
Organizing Agency Staff and Partners/Contract Personnel

RESPONSIBLE DIVISION
Subdirectorate of Demographic Statistics""" ;
                                                    rdfs:label "SP2020 - Design Collection - Process Method (Collection)"@en .


###  https://www.bps.go.id/survey/population-census#SP2020DesignCollectionProcessOutputSpecification
id-ps:SP2020DesignCollectionProcessOutputSpecification rdf:type owl:NamedIndividual ,
                                                                :ProcessOutputSpecification ;
                                                       :coreOutputType "Process Method of Collection" ;
                                                       rdfs:label "SP2020 - Design Collection - Process Output Specification"@en .


###  https://www.bps.go.id/survey/population-census#SP2020DesignOutputBusinessCase
id-ps:SP2020DesignOutputBusinessCase rdf:type owl:NamedIndividual ,
                                              gsim-sum:BusinessCase ;
                                     gsim-sum:hasOutputs-BC """To calculate serveral indicator related to Indonesian population in 2020, including:
- Total population
- Total population by administration
- Total population migration
- Total population by generation""" ;
                                     rdfs:label "SP2020 - Design Output - Business Case"@en .


###  https://www.bps.go.id/survey/population-census#SP2020DesignOutputCoreInput
id-ps:SP2020DesignOutputCoreInput rdf:type owl:NamedIndividual ,
                                           :CoreInput ;
                                  :correspondsToPI-PIS id-ps:SP2020DesignOutputProcessInputSpecification ;
                                  :refersToCI-IA id-ps:SP2020DesignOutputBusinessCase ;
                                  rdfs:label "SP2020 - Design Output - Process Input (Core Input)"@en .


###  https://www.bps.go.id/survey/population-census#SP2020DesignOutputCoreOutput
id-ps:SP2020DesignOutputCoreOutput rdf:type owl:NamedIndividual ,
                                            :CoreOutput ;
                                   :correspondsToPO-POS id-ps:SP2020DesignOutputProcessOutputSpecification ;
                                   :refersToCO-IA id-ps:SP2020DesignOutputOutputSpecification ,
                                                  id-ps:SP2020DesignOutputStatisticalProgramDesign ;
                                   rdfs:label "SP2020 - Design Output - Process Output (Core Output)"@en .


###  https://www.bps.go.id/survey/population-census#SP2020DesignOutputOutputSpecification
id-ps:SP2020DesignOutputOutputSpecification rdf:type owl:NamedIndividual ,
                                                     gsim-sum:OutputSpecification ;
                                            gsim-sum:hasValue-IA """Indicator #1
Name: Total Population
Definition: The absolute measure of population, expressed in persons
Unit: Person
Calculation Mechanism: Summation of each individual
Benefit: Serves as the basis for development planning in various fields
Interpretation: The higher the figure, the greater the total population 
Update Frequency: Biennial or more frequent
Reference: Statistics Indonesia
Subject: Population and migration
Measure: Total
Concept: Population includes all individuals residing within the territory of the Unitary State of the Republic of Indonesia for 1 year or more, or those residing for less than 1 year but with the intention to settle for 1 year or more

Indicator #2
Name: Total Population by Population Administration
Definition: The absolute measure of population according to Population Administration records, expressed in persons
Unit: Person
Calculation Mechanism: Summation of each individual
Benefit: 
- Basis for utilization in:
  (1) Public services;
  (2) Development planning;
  (3) Budget allocation;
  (4) Democracy development;
  (5) Law enforcement and crime prevention.
Interpretation: The higher the figure, the greater the total population 
Update Frequency: Semiannual
Reference: Ministry of Home Affairs
Subject: Population and migration
Measure: Total
Concept: Population according to the address stated on population documents, including both Indonesian citizens and foreigners residing within the territory of the Republic of Indonesia and fulfilling the requirements of applicable laws and regulations

Indicator #3
Name: Total Population Migration
Definition: The absolute measure of migrating population, expressed in persons
Unit: Person
Calculation Mechanism: Summation of each individual
Benefit: Serves as the basis for development planning in various fields, especially regarding migration and population mobility
Interpretation: The higher the figure, the greater the total population migration 
Update Frequency: Biennial or more frequent
Reference: Statistics Indonesia
Subject: Population and migration
Measure: Total
Concept: Migrating Population:
  Individuals recorded in the initial Civil Registry data as residents of a particular Village/Subdistrict but are no longer present in that Village/Subdistrict during the SP2020

Indicator #4
Name: Total Population by Generation
Definition: The absolute measure of population by generation, expressed in persons
Unit: Person
Calculation Mechanism: Summation of each individual
Benefit: Serves as the basis for development planning in various fields
Interpretation: The higher the figure, the greater the total population 
Update Frequency: Biennial or more frequent
Reference: Central Statistics Agency
Subject: Population and migration
Measure: Total
Concept: Population by Generation:
  Categorization of population by generation. Classification source: William H. Frey analysis of Census Bureau Population Estimates (25 June 2020)""" ;
                                            rdfs:label "SP2020 - Design Output - Output Specification"@en .


###  https://www.bps.go.id/survey/population-census#SP2020DesignOutputProcess
id-ps:SP2020DesignOutputProcess rdf:type owl:NamedIndividual ,
                                         :ProcessStep ;
                                :createsPS-PO id-ps:SP2020DesignOutputCoreOutput ,
                                              id-ps:SP2020DesignOutputProcessExecutionLog ;
                                :hasPS-PI id-ps:SP2020DesignOutputCoreInput ;
                                :hasEndTime-PS "2018-06-29T20:00:00"^^xsd:dateTime ;
                                :hasStartTime-PS "2018-05-02T08:00:00"^^xsd:dateTime ;
                                rdfs:label "SP2020 - Design Output - Process"@en .


###  https://www.bps.go.id/survey/population-census#SP2020DesignOutputProcessControlDesign
id-ps:SP2020DesignOutputProcessControlDesign rdf:type owl:NamedIndividual ,
                                                      :ProcessControlDesign ;
                                             gsim-sum:hasValue-IA """Has all the information from the business case been described in the statistical indicators and statistical program design that will be produced?
- If no, go to back to the beginning of the Process Step and run again 
- If yes, go to the next Process Step""" ;
                                             rdfs:label "SP2020 - Design Output - Process Control Design"@en .


###  https://www.bps.go.id/survey/population-census#SP2020DesignOutputProcessDesign
id-ps:SP2020DesignOutputProcessDesign rdf:type owl:NamedIndividual ,
                                               :ProcessDesign ;
                                      :classifiedAs <http://id.unece.org/models/gsbpm/2.1> ;
                                      :hasPD-PCD id-ps:SP2020DesignOutputProcessControlDesign ;
                                      :hasPD-PIS id-ps:SP2020DesignOutputProcessInputSpecification ;
                                      :hasPD-POS id-ps:SP2020DesignOutputProcessOutputSpecification ;
                                      :implementsPD-PM id-ps:SP2020DesignOutputProcessMethod ;
                                      :specifiesPD-PS id-ps:SP2020DesignOutputProcess ;
                                      rdfs:label "SP2020 - Design Output - Process Design"@en .


###  https://www.bps.go.id/survey/population-census#SP2020DesignOutputProcessExecutionLog
id-ps:SP2020DesignOutputProcessExecutionLog rdf:type owl:NamedIndividual ,
                                                     :ProcessExecutionLog ;
                                            gsim-sum:hasExecutionLog """- All the information from the business case been described in the statistical indicators and statistical program
- Requests for additional indicators by stackholders can be accommodated during the Longform Population Census
- It is necessary to further refine the mechanism for calculating the resulting indicators""" ;
                                            rdfs:label "SP2020 - Design Output - Execution Log" .


###  https://www.bps.go.id/survey/population-census#SP2020DesignOutputProcessInputSpecification
id-ps:SP2020DesignOutputProcessInputSpecification rdf:type owl:NamedIndividual ,
                                                           :ProcessInputSpecification ;
                                                  :coreInputType "Business Case" ;
                                                  rdfs:label "SP2020 - Design Output - Process Input Specification"@en .


###  https://www.bps.go.id/survey/population-census#SP2020DesignOutputProcessMethod
id-ps:SP2020DesignOutputProcessMethod rdf:type owl:NamedIndividual ,
                                               :ProcessMethod ;
                                      gsim-sum:hasValue-IA """- Check the business case received
- Analyze definitions, units, units of observation, types of units of observation, types of observational studies, measures, calculation methods, interpretations, and related concepts from existing reference metadata
- Produce output specifications and statistical program design""" ;
                                      rdfs:label "SP2020 - Design Output - Process Method"@en .


###  https://www.bps.go.id/survey/population-census#SP2020DesignOutputProcessOutputSpecification
id-ps:SP2020DesignOutputProcessOutputSpecification rdf:type owl:NamedIndividual ,
                                                            :ProcessOutputSpecification ;
                                                   :coreOutputType "Output Specification: Provides general information about statistical indicator (name, definition, unit, calculate mechanism, benefit, etc.)" ,
                                                                   "Process Method" ,
                                                                   "Statistical Program Design" ;
                                                   rdfs:label "SP2020 - Design Output - Process Output Specification"@en .


###  https://www.bps.go.id/survey/population-census#SP2020DesignOutputStatisticalProgramDesign
id-ps:SP2020DesignOutputStatisticalProgramDesign rdf:type owl:NamedIndividual ,
                                                          gsim-sum:StatisticalProgramDesign ;
                                                 gsim-sum:hasName-IA "General Design of Population Census" ;
                                                 gsim-sum:hasValue-IA """UNIT OF OBSERVATION
All individuals (Indonesian citizens and foreigners) residing in the territory of the Unitary State of the Republic of Indonesia for one year or more, or those residing for less than one year but intending to settle for more than one year.

TYPE OF OBSERVATIONAL STUDY
Cross-Sectional

TYPE OF UNIT OF OBSERVATION
Individuals""" ;
                                                 rdfs:label "SP2020 - Design Output - Statistical Program Design"@en .


###  https://www.bps.go.id/survey/population-census#SP2020DesignProcessingAndAnalysisProcess
id-ps:SP2020DesignProcessingAndAnalysisProcess rdf:type owl:NamedIndividual ,
                                                        :ProcessStep ;
                                               :createsPS-PO id-ps:SP2020DesignProcessingAndAnalysisProcessCoreOutput ,
                                                             id-ps:SP2020DesignProcessingAndAnalysisProcessExecutionLog ;
                                               :hasPS-PI id-ps:SP2020DesignProcessingAndAnalysisProcessCoreInput ;
                                               :hasEndTime-PS "2018-10-17T00:00:00"^^xsd:dateTime ;
                                               :hasStartTime-PS "2018-09-03T00:00:00"^^xsd:dateTime ;
                                               rdfs:label "SP2020 - Design Processing And Analysis - Process"@en .


###  https://www.bps.go.id/survey/population-census#SP2020DesignProcessingAndAnalysisProcessControlDesign
id-ps:SP2020DesignProcessingAndAnalysisProcessControlDesign rdf:type owl:NamedIndividual ,
                                                                     :ProcessControlDesign ;
                                                            gsim-sum:hasValue-IA """Has all the information from the business case and statistical program design been described in the statistical indicators that will be produced?
- If no, go to back to the beginning of the Process Step and run again 
- If yes, go to the next Process Step""" ;
                                                            rdfs:label "SP2020 - Design Processing And Analysis - Process Control Design"@en .


###  https://www.bps.go.id/survey/population-census#SP2020DesignProcessingAndAnalysisProcessCoreInput
id-ps:SP2020DesignProcessingAndAnalysisProcessCoreInput rdf:type owl:NamedIndividual ,
                                                                 :CoreInput ;
                                                        :correspondsToPI-PIS id-ps:SP2020DesignProcessingAndAnalysisProcessInputSpecification ;
                                                        :refersToCI-IA id-ps:SP2020DesignOutputBusinessCase ,
                                                                       id-ps:SP2020DesignOutputStatisticalProgramDesign ;
                                                        rdfs:label "SP2020 - Design Processing And Analysis - Process Input (Core Input)"@en .


###  https://www.bps.go.id/survey/population-census#SP2020DesignProcessingAndAnalysisProcessCoreOutput
id-ps:SP2020DesignProcessingAndAnalysisProcessCoreOutput rdf:type owl:NamedIndividual ,
                                                                  :CoreOutput ;
                                                         :correspondsToPO-POS id-ps:SP2020DesignProcessingAndAnalysisProcessOutputSpecification ;
                                                         :refersToCO-IA id-ps:SP2020DesignProcessingAndAnalysisProcessMethodAnalysis ,
                                                                        id-ps:SP2020DesignProcessingAndAnalysisProcessMethodProcessing ;
                                                         rdfs:label "SP2020 - Design Processing And Analysis - Process Output (Core Output)"@en .


###  https://www.bps.go.id/survey/population-census#SP2020DesignProcessingAndAnalysisProcessDesign
id-ps:SP2020DesignProcessingAndAnalysisProcessDesign rdf:type owl:NamedIndividual ,
                                                              :ProcessDesign ;
                                                     :classifiedAs <http://id.unece.org/models/gsbpm/2.5> ;
                                                     :hasPD-PCD id-ps:SP2020DesignProcessingAndAnalysisProcessControlDesign ;
                                                     :hasPD-PIS id-ps:SP2020DesignProcessingAndAnalysisProcessInputSpecification ;
                                                     :hasPD-POS id-ps:SP2020DesignProcessingAndAnalysisProcessOutputSpecification ;
                                                     :implementsPD-PM id-ps:SP2020DesignProcessingAndAnalysisProcessMethod ;
                                                     :specifiesPD-PS id-ps:SP2020DesignProcessingAndAnalysisProcess ;
                                                     rdfs:label "SP2020 - Design Processing And Analysis - Process Design"@en .


###  https://www.bps.go.id/survey/population-census#SP2020DesignProcessingAndAnalysisProcessExecutionLog
id-ps:SP2020DesignProcessingAndAnalysisProcessExecutionLog rdf:type owl:NamedIndividual ,
                                                                    :ProcessExecutionLog ;
                                                           gsim-sum:hasExecutionLog """- All information from the business case and statistical program design have been described in the design processing and analysis
- Processing tools will adapt to the resulting questionnaire. Because there is a multi-modal collection process, preparation for making tools must be done long before the dress rehearsal.
- Analysis tools will use cloud computing that has been provided, so that the data processed does not leave the analysis environment.""" ;
                                                           rdfs:label "SP2020 - Design Processing And Analysis - Execution Log" .


###  https://www.bps.go.id/survey/population-census#SP2020DesignProcessingAndAnalysisProcessInputSpecification
id-ps:SP2020DesignProcessingAndAnalysisProcessInputSpecification rdf:type owl:NamedIndividual ,
                                                                          :ProcessInputSpecification ;
                                                                 :coreInputType "Business Case" ,
                                                                                "Statistical Program Design" ;
                                                                 rdfs:label "SP2020 - Design Processing And Analysis - Process Input Specification"@en .


###  https://www.bps.go.id/survey/population-census#SP2020DesignProcessingAndAnalysisProcessMethod
id-ps:SP2020DesignProcessingAndAnalysisProcessMethod rdf:type owl:NamedIndividual ,
                                                              :ProcessMethod ;
                                                     gsim-sum:hasValue-IA """- Check the business case and statistical program design received
- Analyze the requirements
- Review processing and analysis methods from reference metadata
- Produce processing and analysis method""" ;
                                                     rdfs:label "SP2020 - Design Processing And Analysis - Process Method"@en .


###  https://www.bps.go.id/survey/population-census#SP2020DesignProcessingAndAnalysisProcessMethodAnalysis
id-ps:SP2020DesignProcessingAndAnalysisProcessMethodAnalysis rdf:type owl:NamedIndividual ,
                                                                      :ProcessMethod ;
                                                             gsim-sum:hasName-IA "Desain Analisis Data Sensus Penduduk" ;
                                                             gsim-sum:hasValue-IA """ANALYSIS UNITS
individual, household

DOES IT USE SECONDARY DATA
Yes

SECONDARY DATASET NAME
Population Administration Data

LEVEL OF PRESENTATION OF ANALYSIS RESULTS
Subdistrict

RESPONSIBLE DIVISION
Subdirectorate of Demographic Statistics

TYPE OF ANALYSIS UNIT
People, Households, Households

ANALYSIS METHODS
Descriptive Analysis""" ;
                                                             rdfs:label "SP2020 - Design Processing And Analysis - Process Method (Analysis)" .


###  https://www.bps.go.id/survey/population-census#SP2020DesignProcessingAndAnalysisProcessMethodProcessing
id-ps:SP2020DesignProcessingAndAnalysisProcessMethodProcessing rdf:type owl:NamedIndividual ,
                                                                        :ProcessMethod ;
                                                               gsim-sum:hasName-IA "Desain Pemrosesan Data Sensus Penduduk" ;
                                                               gsim-sum:hasValue-IA """WHETHER TO DO SAMPLING ERROR CALCULATIONS
No

REASONS FOR NOT COUNTING SAMPLING ERROR
Because it is a census activity

DOES IDENTIFY NONSAMPLING ERROR
Yes

TECHNOLOGY
The 2020 Population Census in Indonesia implemented multi-mode data collection, consisting of Computer-Aided Web Interviewing (CAWI), Computer-Assisted Personal Interviewing (CAPI), and Paper and Pencil Interviewing (PAPI)

DATA COMPARABILITY
Between Regions and Between Times

DATA PROCESSING STAGES
Batching, Editing, Editing, Coding, Coding, Data Input (Data Entry), Data Input (Data Entry), Validation, Validation, Verification, Verification, Tabulation, Tabulation

TREATMENT OF OUTLIERS
Imputation""" ;
                                                               rdfs:label "SP2020 - Design Processing And Analysis - Process Method (Processing)" .


###  https://www.bps.go.id/survey/population-census#SP2020DesignProcessingAndAnalysisProcessOutputSpecification
id-ps:SP2020DesignProcessingAndAnalysisProcessOutputSpecification rdf:type owl:NamedIndividual ,
                                                                           :ProcessOutputSpecification ;
                                                                  :coreOutputType "Process Method of Analysis" ,
                                                                                  "Process Method of Processing" ;
                                                                  rdfs:label "SP2020 - Design Processing And Analysis - Process Output Specification"@en .


###  https://www.bps.go.id/survey/population-census#SP2020DesignVariableDescriptionsProcess
id-ps:SP2020DesignVariableDescriptionsProcess rdf:type owl:NamedIndividual ,
                                                       :ProcessStep ;
                                              :createsPS-PO id-ps:SP2020DesignVariableDescriptionsProcessCoreOutput ,
                                                            id-ps:SP2020DesignVariableDescriptionsProcessExecutionLog ;
                                              :hasPS-PI id-ps:SP2020DesignVariableDescriptionsProcessCoreInput ;
                                              :hasEndTime-PS "2018-07-13T23:00:00"^^xsd:dateTime ;
                                              :hasStartTime-PS "2018-05-14T07:00:00"^^xsd:dateTime ;
                                              rdfs:label "SP2020 - Design Variable Descriptions - Process"@en .


###  https://www.bps.go.id/survey/population-census#SP2020DesignVariableDescriptionsProcessConceptAddress
id-ps:SP2020DesignVariableDescriptionsProcessConceptAddress rdf:type owl:NamedIndividual ,
                                                                     gsim-sum:Concept ;
                                                            gsim-sum:hasDescription-IA "The current residence address is the domicile or usual address of residence, namely the legal residence of the legal subject (person or business entity) or is defined as the official residence. The term comes from domicile which means residence or place of residence." ;
                                                            rdfs:label "SP2020 - Design Variable Descriptions - Concept - Address" .


###  https://www.bps.go.id/survey/population-census#SP2020DesignVariableDescriptionsProcessConceptBuilding
id-ps:SP2020DesignVariableDescriptionsProcessConceptBuilding rdf:type owl:NamedIndividual ,
                                                                      gsim-sum:Concept ;
                                                             rdfs:label "SP2020 - Design Variable Descriptions - Concept - Building" .


###  https://www.bps.go.id/survey/population-census#SP2020DesignVariableDescriptionsProcessConceptFamilyCardNumber
id-ps:SP2020DesignVariableDescriptionsProcessConceptFamilyCardNumber rdf:type owl:NamedIndividual ,
                                                                              gsim-sum:Concept ;
                                                                     gsim-sum:hasDescription-IA "Family Card is a family identity card which contains data about the name, structure and relationships within the family, as well as the identity of family members." ;
                                                                     rdfs:label "SP2020 - Design Variable Descriptions - Concept - Family Card Number"@en .


###  https://www.bps.go.id/survey/population-census#SP2020DesignVariableDescriptionsProcessConceptFamilyRelationshipStatus
id-ps:SP2020DesignVariableDescriptionsProcessConceptFamilyRelationshipStatus rdf:type owl:NamedIndividual ,
                                                                                      gsim-sum:Concept ;
                                                                             gsim-sum:hasDescription-IA "Family relationship status is information that shows the relationship between family members and the head of the family." ;
                                                                             rdfs:label "SP2020 - Design Variable Descriptions - Concept - Family Relationship Status" .


###  https://www.bps.go.id/survey/population-census#SP2020DesignVariableDescriptionsProcessConceptIDNumber
id-ps:SP2020DesignVariableDescriptionsProcessConceptIDNumber rdf:type owl:NamedIndividual ,
                                                                      gsim-sum:Concept ;
                                                             gsim-sum:hasDescription-IA "ID Number is a Population Identity Number which is unique or distinctive, single and attached to a person who is registered as an Indonesian Resident." ;
                                                             rdfs:label "SP2020 - Design Variable Descriptions - Concept - ID Number" .


###  https://www.bps.go.id/survey/population-census#SP2020DesignVariableDescriptionsProcessConceptName
id-ps:SP2020DesignVariableDescriptionsProcessConceptName rdf:type owl:NamedIndividual ,
                                                                  gsim-sum:Concept ;
                                                         gsim-sum:hasDescription-IA "A name is a word to refer to or call a person or can also be interpreted as a word that functions as a term that identifies a person or as a marker of someone's identity." ;
                                                         rdfs:label "SP2020 - Design Variable Descriptions - Concept - Name" .


###  https://www.bps.go.id/survey/population-census#SP2020DesignVariableDescriptionsProcessConceptSex
id-ps:SP2020DesignVariableDescriptionsProcessConceptSex rdf:type owl:NamedIndividual ,
                                                                 gsim-sum:Concept ;
                                                        gsim-sum:hasDescription-IA "The differences between women and men are biologically marked by certain physical characteristics. Gender is divided into women and men" ;
                                                        rdfs:label "SP2020 - Design Variable Descriptions - Concept - Sex" .


###  https://www.bps.go.id/survey/population-census#SP2020DesignVariableDescriptionsProcessControlDesign
id-ps:SP2020DesignVariableDescriptionsProcessControlDesign rdf:type owl:NamedIndividual ,
                                                                    :ProcessControlDesign ;
                                                           gsim-sum:hasValue-IA """Has all the information from the business case and statistical program design been described into variables that will be used?
- If no, go to back to the beginning of the Process Step and run again 
- If yes, go to the next Process Step""" ;
                                                           rdfs:label "SP2020 - Design Variable Descriptions - Process Control Design"@en .


###  https://www.bps.go.id/survey/population-census#SP2020DesignVariableDescriptionsProcessCoreInput
id-ps:SP2020DesignVariableDescriptionsProcessCoreInput rdf:type owl:NamedIndividual ,
                                                                :CoreInput ;
                                                       :correspondsToPI-PIS id-ps:SP2020DesignVariableDescriptionsProcessInputSpecification ;
                                                       :refersToCI-IA id-ps:SP2020DesignOutputBusinessCase ,
                                                                      id-ps:SP2020DesignOutputStatisticalProgramDesign ;
                                                       rdfs:label "SP2020 - Design Variable Descriptions - Process Input (Core Input)"@en .


###  https://www.bps.go.id/survey/population-census#SP2020DesignVariableDescriptionsProcessCoreOutput
id-ps:SP2020DesignVariableDescriptionsProcessCoreOutput rdf:type owl:NamedIndividual ,
                                                                 :CoreOutput ;
                                                        :correspondsToPO-POS id-ps:SP2020DesignVariableDescriptionsProcessOutputSpecification ;
                                                        :refersToCO-IA id-ps:SP2020DesignVariableDescriptionsProcessVariableAddress ,
                                                                       id-ps:SP2020DesignVariableDescriptionsProcessVariableBuildingSerialNumber ,
                                                                       id-ps:SP2020DesignVariableDescriptionsProcessVariableFamilyNumber ,
                                                                       id-ps:SP2020DesignVariableDescriptionsProcessVariableFamilyRelationshipStatus ,
                                                                       id-ps:SP2020DesignVariableDescriptionsProcessVariableIDNumber ,
                                                                       id-ps:SP2020DesignVariableDescriptionsProcessVariableName ,
                                                                       id-ps:SP2020DesignVariableDescriptionsProcessVariableSex ;
                                                        rdfs:label "SP2020 - Design Variable Descriptions - Process Output (Core Output)"@en .


###  https://www.bps.go.id/survey/population-census#SP2020DesignVariableDescriptionsProcessDesign
id-ps:SP2020DesignVariableDescriptionsProcessDesign rdf:type owl:NamedIndividual ,
                                                             :ProcessDesign ;
                                                    :classifiedAs <http://id.unece.org/models/gsbpm/2.2> ;
                                                    :hasPD-PCD id-ps:SP2020DesignVariableDescriptionsProcessControlDesign ;
                                                    :hasPD-PIS id-ps:SP2020DesignVariableDescriptionsProcessInputSpecification ;
                                                    :hasPD-POS id-ps:SP2020DesignVariableDescriptionsProcessOutputSpecification ;
                                                    :implementsPD-PM id-ps:SP2020DesignVariableDescriptionsProcessMethod ;
                                                    :specifiesPD-PS id-ps:SP2020DesignVariableDescriptionsProcess ;
                                                    rdfs:label "SP2020 - Design Variable Descriptions - Process Design"@en .


###  https://www.bps.go.id/survey/population-census#SP2020DesignVariableDescriptionsProcessExecutionLog
id-ps:SP2020DesignVariableDescriptionsProcessExecutionLog rdf:type owl:NamedIndividual ,
                                                                   :ProcessExecutionLog ;
                                                          gsim-sum:hasExecutionLog """All information from the business case and statistical program design have been described into variables. Has all the information from the business case and statistical program design been described into variables that will be used?
- If no, go to back to the beginning of the Process Step and run again 
- If yes, go to the next Process Step""" ;
                                                          rdfs:label "SP2020 - Design Variable Descriptions - Execution Log" .


###  https://www.bps.go.id/survey/population-census#SP2020DesignVariableDescriptionsProcessInputSpecification
id-ps:SP2020DesignVariableDescriptionsProcessInputSpecification rdf:type owl:NamedIndividual ,
                                                                         :ProcessInputSpecification ;
                                                                :coreInputType "Business Case" ,
                                                                               "Statistical Program Design" ;
                                                                rdfs:label "SP2020 - Design Variable Descriptions - Process Input Specification"@en .


###  https://www.bps.go.id/survey/population-census#SP2020DesignVariableDescriptionsProcessMethod
id-ps:SP2020DesignVariableDescriptionsProcessMethod rdf:type owl:NamedIndividual ,
                                                             :ProcessMethod ;
                                                    gsim-sum:hasValue-IA """- Check the business case and statistical program design received
- Analyze requirement and review existing concept from reference metadata
- Produce variables""" ;
                                                    rdfs:label "SP2020 - Design Variable Descriptions - Process Method"@en .


###  https://www.bps.go.id/survey/population-census#SP2020DesignVariableDescriptionsProcessOutputSpecification
id-ps:SP2020DesignVariableDescriptionsProcessOutputSpecification rdf:type owl:NamedIndividual ,
                                                                          :ProcessOutputSpecification ;
                                                                 :coreOutputType "Address Variables" ,
                                                                                 "Building Serial Number Variables" ,
                                                                                 "Family Card Number Variables" ,
                                                                                 "Family Relationship Status Variables" ,
                                                                                 "ID Number Variables" ,
                                                                                 "Name Variables" ,
                                                                                 "Sex Variables" ;
                                                                 rdfs:label "SP2020 - Design Variable Descriptions - Process Output Specification"@en .


###  https://www.bps.go.id/survey/population-census#SP2020DesignVariableDescriptionsProcessUnitTypePerson
id-ps:SP2020DesignVariableDescriptionsProcessUnitTypePerson rdf:type owl:NamedIndividual ,
                                                                     gsim-sum:UnitType ;
                                                            rdfs:label "SP2020 - Design Variable Descriptions - Unit Type - Person"@en .


###  https://www.bps.go.id/survey/population-census#SP2020DesignVariableDescriptionsProcessUnitTypeVillage
id-ps:SP2020DesignVariableDescriptionsProcessUnitTypeVillage rdf:type owl:NamedIndividual ,
                                                                      gsim-sum:UnitType ;
                                                             rdfs:label "SP2020 - Design Variable Descriptions - Unit Type - Village"@en .


###  https://www.bps.go.id/survey/population-census#SP2020DesignVariableDescriptionsProcessVariableAddress
id-ps:SP2020DesignVariableDescriptionsProcessVariableAddress rdf:type owl:NamedIndividual ,
                                                                      gsim-sum:Variable ;
                                                             gsim-sum:measuresV-C id-ps:SP2020DesignVariableDescriptionsProcessConceptAddress ;
                                                             gsim-sum:measuresV-UT id-ps:SP2020DesignVariableDescriptionsProcessUnitTypePerson ;
                                                             gsim-sum:hasDescription-IA "Location that shows where the respondent lived when the census was carried out." ;
                                                             gsim-sum:hasName-IA "Address" ;
                                                             rdfs:label "SP2020 - Design Variable Descriptions - Variable - Address"@en .


###  https://www.bps.go.id/survey/population-census#SP2020DesignVariableDescriptionsProcessVariableBuildingSerialNumber
id-ps:SP2020DesignVariableDescriptionsProcessVariableBuildingSerialNumber rdf:type owl:NamedIndividual ,
                                                                                   gsim-sum:Variable ;
                                                                          gsim-sum:measuresV-C id-ps:SP2020DesignVariableDescriptionsProcessConceptBuilding ;
                                                                          gsim-sum:measuresV-UT id-ps:SP2020DesignVariableDescriptionsProcessUnitTypeVillage ;
                                                                          gsim-sum:hasDescription-IA "Number that shows the location/position of the census building sequence in a Local Environmental Unit." ;
                                                                          gsim-sum:hasName-IA "Building Serial Number" ;
                                                                          rdfs:label "SP2020 - Design Variable Descriptions - Variable - Building Serial Number"@en .


###  https://www.bps.go.id/survey/population-census#SP2020DesignVariableDescriptionsProcessVariableFamilyNumber
id-ps:SP2020DesignVariableDescriptionsProcessVariableFamilyNumber rdf:type owl:NamedIndividual ,
                                                                           gsim-sum:Variable ;
                                                                  gsim-sum:measuresV-C id-ps:SP2020DesignVariableDescriptionsProcessConceptFamilyCardNumber ;
                                                                  gsim-sum:measuresV-UT id-ps:SP2020DesignVariableDescriptionsProcessUnitTypeVillage ;
                                                                  gsim-sum:hasDescription-IA "The Family Card Number consists of 16 (sixteen) digits and the compilation code consists of the first 6 (six) digits of province, district/city and sub-district." ;
                                                                  gsim-sum:hasName-IA "Family Card Number" ;
                                                                  rdfs:label "SP2020 - Design Variable Descriptions - Variable - Family Card Number"@en .


###  https://www.bps.go.id/survey/population-census#SP2020DesignVariableDescriptionsProcessVariableFamilyRelationshipStatus
id-ps:SP2020DesignVariableDescriptionsProcessVariableFamilyRelationshipStatus rdf:type owl:NamedIndividual ,
                                                                                       gsim-sum:Variable ;
                                                                              gsim-sum:measuresV-C id-ps:SP2020DesignVariableDescriptionsProcessConceptFamilyRelationshipStatus ;
                                                                              gsim-sum:measuresV-UT id-ps:SP2020DesignVariableDescriptionsProcessUnitTypePerson ;
                                                                              gsim-sum:hasDescription-IA "The relationship status of family members with the head of the family is needed to see the composition of family members, living arrangements and child rearing patterns." ;
                                                                              gsim-sum:hasName-IA "Family Relationship Status" ;
                                                                              rdfs:label "SP2020 - Design Variable Descriptions - Variable - Family Relationship Status"@en .


###  https://www.bps.go.id/survey/population-census#SP2020DesignVariableDescriptionsProcessVariableIDNumber
id-ps:SP2020DesignVariableDescriptionsProcessVariableIDNumber rdf:type owl:NamedIndividual ,
                                                                       gsim-sum:Variable ;
                                                              gsim-sum:measuresV-C id-ps:SP2020DesignVariableDescriptionsProcessConceptIDNumber ;
                                                              gsim-sum:measuresV-UT id-ps:SP2020DesignVariableDescriptionsProcessUnitTypePerson ;
                                                              gsim-sum:hasDescription-IA "The ID Number consists of 16 (sixteen) digits and the compilation code consists of the first 6 (six) digits of the province, district/city and sub-district, the second 6 (six) digits are the date, month, year of birth and the last 4 (four) digits are the number. ID Number issuance sequence which is processed automatically with SIAK (Population Administration Information System)." ;
                                                              gsim-sum:hasName-IA "ID Number" ;
                                                              rdfs:label "SP2020 - Design Variable Descriptions - Variable - ID Number"@en .


###  https://www.bps.go.id/survey/population-census#SP2020DesignVariableDescriptionsProcessVariableName
id-ps:SP2020DesignVariableDescriptionsProcessVariableName rdf:type owl:NamedIndividual ,
                                                                   gsim-sum:Variable ;
                                                          gsim-sum:measuresV-C id-ps:SP2020DesignVariableDescriptionsProcessConceptName ;
                                                          gsim-sum:measuresV-UT id-ps:SP2020DesignVariableDescriptionsProcessUnitTypePerson ;
                                                          gsim-sum:hasDescription-IA "Identity to call or refer to someone." ;
                                                          gsim-sum:hasName-IA "Name" ;
                                                          rdfs:label "SP2020 - Design Variable Descriptions - Variable - Name"@en .


###  https://www.bps.go.id/survey/population-census#SP2020DesignVariableDescriptionsProcessVariableSex
id-ps:SP2020DesignVariableDescriptionsProcessVariableSex rdf:type owl:NamedIndividual ,
                                                                  gsim-sum:Variable ;
                                                         gsim-sum:measuresV-C id-ps:SP2020DesignVariableDescriptionsProcessConceptSex ;
                                                         gsim-sum:measuresV-UT id-ps:SP2020DesignVariableDescriptionsProcessUnitTypePerson ;
                                                         gsim-sum:hasDescription-IA "Gender is the biological difference between men and women. These biological differences can be seen from genitals and genetic differences." ;
                                                         gsim-sum:hasName-IA "Sex" ;
                                                         rdfs:label "SP2020 - Design Variable Descriptions - Variable - Sex"@en .


###  https://www.ksh.hu/survey/retail-trade-statistics#CheckDataAvailabilityProcess
kshrts:CheckDataAvailabilityProcess rdf:type owl:NamedIndividual ,
                                             :ProcessStep ;
                                    rdfs:label "RTS - Check Data Availability - Process"@en .


###  https://www.ksh.hu/survey/retail-trade-statistics#CheckDataAvailabilityProcessControlDesign
kshrts:CheckDataAvailabilityProcessControlDesign rdf:type owl:NamedIndividual ,
                                                          :ProcessControlDesign ;
                                                 gsim-sum:hasValue-IA """Has all relevant information been analysed and assessed to produce Assessment?
- If no, go back to the beginning of the Process Step and run again 
- If yes, go to the Consult and Confirm Needs Process Step""" ;
                                                 rdfs:label "RTS - Check Data Availability - Process Control Design"@en .


###  https://www.ksh.hu/survey/retail-trade-statistics#CheckDataAvailabilityProcessDesign
kshrts:CheckDataAvailabilityProcessDesign rdf:type owl:NamedIndividual ,
                                                   :ProcessDesign ;
                                          :classifiedAs <http://id.unece.org/models/gsbpm/1.5> ;
                                          :hasPD-PCD kshrts:CheckDataAvailabilityProcessControlDesign ;
                                          :hasPD-PIS kshrts:CheckDataAvailabilityProcessInputSpecification ;
                                          :hasPD-POS kshrts:CheckDataAvailabilityProcessOutputSpecification ;
                                          :implementsPD-PM kshrts:CheckDataAvailabilityProcessDesign ;
                                          :specifiesPD-PS kshrts:CheckDataAvailabilityProcess ;
                                          rdfs:label "RTS - Check Data Availability - Process Design"@en .


###  https://www.ksh.hu/survey/retail-trade-statistics#CheckDataAvailabilityProcessInputSpecification
kshrts:CheckDataAvailabilityProcessInputSpecification rdf:type owl:NamedIndividual ,
                                                               :ProcessInputSpecification ;
                                                      :coreInputType "Change Definitions containing structured, detailed information about user needs and specification of Concepts to be measured" ,
                                                                     "Information Resources (e.g., collections of Data Sets) available or accessible by the Organisation" ,
                                                                     "Provision Agreements associated with the Information Resources" ;
                                                      :processSupportInputType "Policies or guidelines to be followed on how to assess the data availability internally and externally" ;
                                                      rdfs:label "RTS - Check Data Availability - Process Input Specification"@en .


###  https://www.ksh.hu/survey/retail-trade-statistics#CheckDataAvailabilityProcessMethod
kshrts:CheckDataAvailabilityProcessMethod rdf:type owl:NamedIndividual ,
                                                   :ProcessMethod ;
                                          gsim-sum:hasValue-IA """- Check whether exiting Information Resources in the Organisation or alternative Information Resources outside the Organisation could meet user needs or be used to measure Concepts or Variables as specified in Change Definition, with consideration with any restriction in Provision Agreements
- Assess the division of responsibilities between different Agents and Data Providers within or outside the Organisation and any ICT resources needed to acquire or transfer the data""" ;
                                          rdfs:label "RTS - Check Data Availability - Process Method"@en .


###  https://www.ksh.hu/survey/retail-trade-statistics#CheckDataAvailabilityProcessOutputSpecification
kshrts:CheckDataAvailabilityProcessOutputSpecification rdf:type owl:NamedIndividual ,
                                                                :ProcessOutputSpecification ;
                                                       :coreOutputType "Assessments on Information Resources (e.g., how they could meet user needs, how alternative Information Resources could be used) including division of work and responsibilities and ICT resources required for data acquisition / collection" ;
                                                       :processExecutionLogType """Execution logs such as
- Time that Process Step started
- Time that Process Step ended""" ;
                                                       :processMetricType """Quality measures (e.g., extent to which current data sources meet user requirements, taking into consideration the conditions under which they would be available and any restrictions on their use)
Quality measures of the Process Step such as:
- Time spent to complete the Process Step (derived from Process Execution Log)
- Cost spent to complete the Process Step""" ;
                                                       rdfs:label "RTS - Check Data Availability - Process Output Specification"@en .


###  https://www.ksh.hu/survey/retail-trade-statistics#ConsultAndConfirmNeeds
kshrts:ConsultAndConfirmNeeds rdf:type owl:NamedIndividual ,
                                       :ProcessStep ;
                              :createsPS-PO kshrts:ConsultAndConfirmNeedsCoreOutput ;
                              :hasPS-PI kshrts:ConsultAndConfirmNeedsCoreInput ;
                              :hasEndTime-PS "2018-02-16T20:00:00"^^xsd:dateTime ;
                              :hasStartTime-PS "2018-01-22T08:00:00"^^xsd:dateTime ;
                              rdfs:label "RTS - Consult and Confirm Needs - Process"@en .


###  https://www.ksh.hu/survey/retail-trade-statistics#ConsultAndConfirmNeedsChangeDefinition
kshrts:ConsultAndConfirmNeedsChangeDefinition rdf:type owl:NamedIndividual ,
                                                       gsim-sum:ChangeDefinition ;
                                              gsim-sum:hasValue-IA """- Investigate the new potential data source (electronic fiscal devices) for the production of retail trade statistics and build a business case
- Provide aggregated data on retail sales on a quarterly basis; broken down by classification of major commodity groups
- Provide aggregated data on retail sales on a monthly basis; broken down by the nomenclature of type of shop
- Produce unadjusted, calendar-effect adjusted, seasonal and calendar-effect adjusted time series data on volume indices on sales in retail shops
- Update the descriptive metadata templates for time series data and test the clarity of the information provided
- Prepare volume indices on sales on a monthly basis, broken down by: food, non-food, fuel""" ;
                                              rdfs:label "RTS - Consult and Confirm Needs - Change Definition"@en .


###  https://www.ksh.hu/survey/retail-trade-statistics#ConsultAndConfirmNeedsCoreInput
kshrts:ConsultAndConfirmNeedsCoreInput rdf:type owl:NamedIndividual ,
                                                :CoreInput ;
                                       :correspondsToPI-PIS kshrts:ConsultAndConfirmNeedsProcessInputSpecification ;
                                       :refersToCI-IA kshrts:IdentifyNeedsStatisticalNeed ;
                                       rdfs:label "RTS - Consult and Confirm Needs - Process Input (Core Input)"@en .


###  https://www.ksh.hu/survey/retail-trade-statistics#ConsultAndConfirmNeedsCoreOutput
kshrts:ConsultAndConfirmNeedsCoreOutput rdf:type owl:NamedIndividual ,
                                                 :CoreOutput ;
                                        :correspondsToPO-POS kshrts:ConsultAndConfirmNeedsProcessOutputSpecification ;
                                        :refersToCO-IA kshrts:ConsultAndConfirmNeedsChangeDefinition ;
                                        rdfs:label "RTS - Consult and Confirm Needs - Process Output (Core Output)"@en .


###  https://www.ksh.hu/survey/retail-trade-statistics#ConsultAndConfirmNeedsProcessControlDesign
kshrts:ConsultAndConfirmNeedsProcessControlDesign rdf:type owl:NamedIndividual ,
                                                           :ProcessControlDesign ;
                                                  gsim-sum:hasValue-IA """Have all Statistical Needs been incorporated into the Change Definition?
- If no, go back to the beginning of the Process Step and run again 
- If yes, go to the next Process Step""" ;
                                                  rdfs:label "RTS - Consult and Confirm Needs - Process Control Design"@en .


###  https://www.ksh.hu/survey/retail-trade-statistics#ConsultAndConfirmNeedsProcessDesign
kshrts:ConsultAndConfirmNeedsProcessDesign rdf:type owl:NamedIndividual ,
                                                    :ProcessDesign ;
                                           :classifiedAs <http://id.unece.org/models/gsbpm/1.2> ;
                                           :hasPD-PCD kshrts:ConsultAndConfirmNeedsProcessControlDesign ;
                                           :hasPD-PIS kshrts:ConsultAndConfirmNeedsProcessInputSpecification ;
                                           :hasPD-POS kshrts:ConsultAndConfirmNeedsProcessOutputSpecification ;
                                           :implementsPD-PM kshrts:ConsultAndConfirmNeedsProcessMethod ;
                                           :specifiesPD-PS kshrts:ConsultAndConfirmNeeds ;
                                           rdfs:label "RTS - Consult and Confirm Needs - Process Design"@en .


###  https://www.ksh.hu/survey/retail-trade-statistics#ConsultAndConfirmNeedsProcessInputSpecification
kshrts:ConsultAndConfirmNeedsProcessInputSpecification rdf:type owl:NamedIndividual ,
                                                                :ProcessInputSpecification ;
                                                       :coreInputType "Statistical Needs: all statistical needs collected (but not necessarily well-defined)" ;
                                                       :processSupportInputType "Policies or guidelines to be followed during consultation with internal and external stakeholders" ;
                                                       rdfs:label "RTS - Consult and Confirm Needs - Process Input Specification"@en .


###  https://www.ksh.hu/survey/retail-trade-statistics#ConsultAndConfirmNeedsProcessMethod
kshrts:ConsultAndConfirmNeedsProcessMethod rdf:type owl:NamedIndividual ,
                                                    :ProcessMethod ;
                                           gsim-sum:hasValue-IA """- Consult the Statistical Needs with internal and external stakeholders to confirm in detail the needs for the statistics
- Produce the Change Definitions specifying the needs in detail""" ;
                                           rdfs:label "RTS - Consult and Confirm Needs - Process Method"@en .


###  https://www.ksh.hu/survey/retail-trade-statistics#ConsultAndConfirmNeedsProcessOutputSpecification
kshrts:ConsultAndConfirmNeedsProcessOutputSpecification rdf:type owl:NamedIndividual ,
                                                                 :ProcessOutputSpecification ;
                                                        :coreOutputType "Change Definitions describing the confirmed, more detailed and structured version of the initial Statistical Needs" ;
                                                        :processExecutionLogType """Execution logs such as
- Time that Process Step started
- Time that Process Step ended
- Log (e.g., time, place, notes) from stakeholder consultations conducted""" ;
                                                        :processMetricType """Quality measures (e.g., extent to which all Statistical Needs are consulted and confirmed)
Quality measures of the Process Step such as:
- Time spent to complete the Process Step (derived from Process Execution Log)
- Cost spent to complete the Process Step""" ;
                                                        rdfs:label "RTS - Consult and Confirm Needs - Process Output Specification"@en .


###  https://www.ksh.hu/survey/retail-trade-statistics#DesignCollectionProcess
kshrts:DesignCollectionProcess rdf:type owl:NamedIndividual ,
                                        :ProcessStep ;
                               rdfs:label "RTS - Design Collection - Process"@en .


###  https://www.ksh.hu/survey/retail-trade-statistics#DesignCollectionProcessControlDesign
kshrts:DesignCollectionProcessControlDesign rdf:type owl:NamedIndividual ,
                                                     :ProcessControlDesign ;
                                            gsim-sum:hasValue-IA """Are all Represented Variables needs to be collected covered by at least one collection instrument?
- If no, go to back to the beginning of the Process Step and run again 
- If yes, go to the next Process Step""" ;
                                            rdfs:label "RTS - Design Collection - Process Control Design"@en .


###  https://www.ksh.hu/survey/retail-trade-statistics#DesignCollectionProcessDesign
kshrts:DesignCollectionProcessDesign rdf:type owl:NamedIndividual ,
                                              :ProcessDesign ;
                                     :classifiedAs <http://id.unece.org/models/gsbpm/2.3> ;
                                     :hasPD-PCD kshrts:DesignCollectionProcessControlDesign ;
                                     :hasPD-PIS kshrts:DesignCollectionProcessInputSpecification ;
                                     :hasPD-POS kshrts:DesignCollectionProcessOutputSpecification ;
                                     :implementsPD-PM kshrts:DesignCollectionProcessMethod ;
                                     :specifiesPD-PS kshrts:DesignCollectionProcess ;
                                     rdfs:label "RTS - Design Collection - Process Design"@en .


###  https://www.ksh.hu/survey/retail-trade-statistics#DesignCollectionProcessInputSpecification
kshrts:DesignCollectionProcessInputSpecification rdf:type owl:NamedIndividual ,
                                                          :ProcessInputSpecification ;
                                                 :coreInputType """- Business Cases containing proposed solutions and approved decisions regarding what Information Resources to be used, including Assessments of cost benefit, risks, etc. 
- Statistical Program Designs that containing information on Represented Variables to be collected and associated information (e.g., Unit Type, Statistical Classifications)""" ;
                                                 :processSupportInputType """Standards, policies or guidelines to be followed during the design of collection instruments.
Repository or inventory of templates available from previous Statistical Program Cycle or similar Statistical Program that can be used as reference such as:
- Questionnaire Specification
- Questionnaire Component
- Data Harvest
- Provision Agreement
- Data Structure
- Process Method""" ;
                                                 rdfs:label "RTS - Design Collection - Process Input Specification"@en .


###  https://www.ksh.hu/survey/retail-trade-statistics#DesignCollectionProcessMethod
kshrts:DesignCollectionProcessMethod rdf:type owl:NamedIndividual ,
                                              :ProcessMethod ;
                                     gsim-sum:hasValue-IA """- Review Business Cases and Represented Variables
- Consult repository or inventory of Exchange Channels, Questionnaire Specification, Data Structure, etc. and relevant guidelines as well as available information from previous Statistical Program Cycle or similar Statistical Program
- Determines Exchange Channels to be used for data collection
- Design collection instrument (e.g., Questionnaire Specification for direct data collection; data transmission mechanism for third party data collection) and Provision Agreement as needed
- Design Process Method to be used for data collection
- Prepare metadata description of Process Method, etc.""" ;
                                     rdfs:label "RTS - Design Collection - Process Method"@en .


###  https://www.ksh.hu/survey/retail-trade-statistics#DesignCollectionProcessOutputSpecification
kshrts:DesignCollectionProcessOutputSpecification rdf:type owl:NamedIndividual ,
                                                           :ProcessOutputSpecification ;
                                                  :coreOutputType """Statistical Program Designs that containing 
- Specification of Exchange Channel (e.g., Questionnaire Specifications, Questionnaire Components, etc. when collecting data directly, e.g., via survey, design of Data Harvest (a tool to be used to pass information between sources, usually by a machine to machine mechanism) when collecting data indirectly, e.g., via survey)
- Data Structures: structure of the Data Sets to be collected by data transmissions, web-scrapping or any other indirect means of data collection
- Provision Agreements: confirmation of any formal agreements to collect or acquire the Data Sets
- Process Methods to be used during data collection (e.g., point of entry validation methods) including quality criteria to be fulfilled during data collection
- Designs of other supporting materials to be used during data collection (e.g., nonresponse Code Lists, response templates, guide to complete questionnaires, training material, schedules, other guides).
- Referential Metadata Set: specifications of the design of the data""" ;
                                                  :processExecutionLogType """Execution logs such as
- Time that Process Step started
- Time that Process Step ended""" ;
                                                  :processMetricType """Quality measures such as (e.g., how well does the collection method suit the nature and volume of the information to be gathered? Is the process re-suing known methods and collection, systems, e.g., according to guidelines/recommendations?)
Quality measures of the Process Step such as:
- Time spent to complete the Process Step (derived from Process Execution Log)
- Cost spent to complete the Process Step""" ;
                                                  rdfs:label "RTS - Design Collection - Process Output Specification"@en .


###  https://www.ksh.hu/survey/retail-trade-statistics#DesignFrameAndSampleProcess
kshrts:DesignFrameAndSampleProcess rdf:type owl:NamedIndividual ,
                                            :ProcessStep ;
                                   rdfs:label "RTS - Design Frame And Sample - Process"@en .


###  https://www.ksh.hu/survey/retail-trade-statistics#DesignFrameAndSampleProcessControlDesign
kshrts:DesignFrameAndSampleProcessControlDesign rdf:type owl:NamedIndividual ,
                                                         :ProcessControlDesign ;
                                                gsim-sum:hasValue-IA """Have all quality criteria been met (e.g., is coverage level acceptable? is population accessible? all required variable covered? is the specified sample statistically efficient)?
- If no, go to back to the beginning of the Process Step and run again 
- If yes, go to the next Process Step""" ;
                                                rdfs:label "RTS - Design Frame And Sample - Process Control Design"@en .


###  https://www.ksh.hu/survey/retail-trade-statistics#DesignFrameAndSampleProcessDesign
kshrts:DesignFrameAndSampleProcessDesign rdf:type owl:NamedIndividual ,
                                                  :ProcessDesign ;
                                         :classifiedAs <http://id.unece.org/models/gsbpm/2.4> ;
                                         :hasPD-PCD kshrts:DesignFrameAndSampleProcessControlDesign ;
                                         :hasPD-PIS kshrts:DesignFrameAndSampleProcessInputSpecification ;
                                         :hasPD-POS kshrts:DesignFrameAndSampleProcessOutputSpecification ;
                                         :implementsPD-PM kshrts:DesignFrameAndSampleProcessMethod ;
                                         :specifiesPD-PS kshrts:DesignFrameAndSampleProcess ;
                                         rdfs:label "RTS - Design Frame And Sample - Process Design"@en .


###  https://www.ksh.hu/survey/retail-trade-statistics#DesignFrameAndSampleProcessInputSpecification
kshrts:DesignFrameAndSampleProcessInputSpecification rdf:type owl:NamedIndividual ,
                                                              :ProcessInputSpecification ;
                                                     :coreInputType """- Business Cases containing proposed solutions and approved decisions regarding target Population
- Data Sets to be used to design frame and sample (e.g., census data, Administrative Register, Statistical Register, geospatial data)
- Data Structures describing the structure of the Data Sets 
- Represented Variables and Statistical Classifications for specification for the frame""" ;
                                                     :processSupportInputType """- Standards, policies or guidelines to be followed during the design of frame and sample
- Data Sets from sample survey of previous Statistical Program Cycle or similar Statistical Program as reference""" ;
                                                     rdfs:label "RTS - Design Frame And Sample - Process Input Specification"@en .


###  https://www.ksh.hu/survey/retail-trade-statistics#DesignFrameAndSampleProcessMethod
kshrts:DesignFrameAndSampleProcessMethod rdf:type owl:NamedIndividual ,
                                                  :ProcessMethod ;
                                         gsim-sum:hasValue-IA """- Review Business Case regarding target Population
- Define Process Methods to be used for creating frame and sample and for calculating relevant measures (e.g., response burden, quality indicators)
- Identify survey Population based on the frame specification""" ;
                                         rdfs:label "RTS - Design Frame And Sample - Process Method"@en .


###  https://www.ksh.hu/survey/retail-trade-statistics#DesignFrameAndSampleProcessOutputSpecification
kshrts:DesignFrameAndSampleProcessOutputSpecification rdf:type owl:NamedIndividual ,
                                                               :ProcessOutputSpecification ;
                                                      :coreInputType """Statistical Program Designs that containing 
- Process Methods such as sample methodology specification (e.g., accuracy level, sample size, weight design, methods to spread response burden and manage overlap or rotation, methods for data integration from multiple sources, if required, for example, in cases when frame drawn is not sufficient) as well as associated Rules 
- Data Structure: frame specification
- Represented Variables (e.g., for linkage if the frame is needed to be extended, stratification if needed)
- Survey Population 
- Referential Metadata Set to be passed along with Process Methods documenting relevance of the frame (how accessible is the population? coverage level of the population), its timeliness (when was the frame updated?), its accuracy (are all variables covered?), its cost (does the frame cost exceed the survey cost?)""" ;
                                                      :processExecutionLogType """Execution logs such as
- Time that Process Step started
- Time that Process Step ended""" ;
                                                      :processMetricType """Quality measures (e.g., extent to which the survey Population matches with the target Population)
Quality measures of the Process Step such as:
- Time spent to complete the Process Step (derived from Process Execution Log)
- Cost spent to complete the Process Step""" ;
                                                      rdfs:label "RTS - Design Frame And Sample - Process Output Specification"@en .


###  https://www.ksh.hu/survey/retail-trade-statistics#DesignOutputProcess
kshrts:DesignOutputProcess rdf:type owl:NamedIndividual ,
                                    :ProcessStep ;
                           rdfs:label "RTS - Design Output - Process"@en .


###  https://www.ksh.hu/survey/retail-trade-statistics#DesignOutputProcessControlDesign
kshrts:DesignOutputProcessControlDesign rdf:type owl:NamedIndividual ,
                                                 :ProcessControlDesign ;
                                        gsim-sum:hasValue-IA """Have all user needs been considered in the design of the output?
- If no, go back to the beginning of the Process Step and run again 
- If yes, go to the next Process Step""" ;
                                        rdfs:label "RTS - Design Output - Process Control Design"@en .


###  https://www.ksh.hu/survey/retail-trade-statistics#DesignOutputProcessDesign
kshrts:DesignOutputProcessDesign rdf:type owl:NamedIndividual ,
                                          :ProcessDesign ;
                                 :classifiedAs <http://id.unece.org/models/gsbpm/2.1> ;
                                 :hasPD-PCD kshrts:DesignOutputProcessControlDesign ;
                                 :hasPD-PIS kshrts:DesignOutputProcessInputSpecification ;
                                 :hasPD-POS kshrts:DesignOutputProcessOutputSpecification ;
                                 :implementsPD-PM kshrts:DesignOutputProcessDesign ;
                                 :specifiesPD-PS kshrts:DesignOutputProcess ;
                                 rdfs:label "RTS - Design Output - Process Design"@en .


###  https://www.ksh.hu/survey/retail-trade-statistics#DesignOutputProcessInputSpecification
kshrts:DesignOutputProcessInputSpecification rdf:type owl:NamedIndividual ,
                                                      :ProcessInputSpecification ;
                                             :coreInputType "Business Cases containing proposed solutions and approved decisions regarding Products and services to be produced" ;
                                             :processSupportInputType """- Legal frameworks and regulations that influence the content and quality of the outputs
- Policies or guidelines to be followed regarding dissemination (e.g., data protection provisions, quality policies)
- Output Specifications, Process Methods, quality criteria or any other referential metadata available from previous Statistical Program Cycles or similar Statistical Programs that can be used as reference""" ;
                                             rdfs:label "RTS - Design Output - Process Input Specification"@en .


###  https://www.ksh.hu/survey/retail-trade-statistics#DesignOutputProcessMethod
kshrts:DesignOutputProcessMethod rdf:type owl:NamedIndividual ,
                                          :ProcessMethod ;
                                 gsim-sum:hasValue-IA """- Review Business Cases regarding outputs and output objectives
- Design outputs such as Products (e.g., Data Sets and its Data Structures) and services in consideration of relevant regulations, polices and guidelines as well as referential metadata available from previous cycle 
- Design Process Methods and system to be used for dissemination""" ;
                                 rdfs:label "RTS - Design Output - Process Method"@en .


###  https://www.ksh.hu/survey/retail-trade-statistics#DesignOutputProcessOutputSpecification
kshrts:DesignOutputProcessOutputSpecification rdf:type owl:NamedIndividual ,
                                                       :ProcessOutputSpecification ;
                                              :coreOutputType """Statistical Program Designs* that containing 
- Output Specifications: specification of Products, (e.g., Data Set and its Data Structure) and quality criteria
- Process Methods: specifications for creating the draft outputs and the dissemination Product 

* Statistical Program Design is used as an umbrella object that rolls up the design specifications in Phase 2""" ;
                                              :processExecutionLogType """Execution logs such as
- Time that Process Step started
- Time that Process Step ended""" ;
                                              :processMetricType """Quality measures (e.g., extent to which user needs are incorporated into the designed outputs)
Quality measures of the Process Step such as:
- Time spent to complete the Process Step (derived from Process Execution Log)
- Cost spent to complete the Process Step""" ;
                                              rdfs:label "RTS - Design Output - Process Output Specification"@en .


###  https://www.ksh.hu/survey/retail-trade-statistics#DesignVariableDescriptionsProcess
kshrts:DesignVariableDescriptionsProcess rdf:type owl:NamedIndividual ,
                                                  :ProcessStep ;
                                         rdfs:label "RTS - Design Variable Descriptions - Process"@en .


###  https://www.ksh.hu/survey/retail-trade-statistics#DesignVariableDescriptionsProcessControlDesign
kshrts:DesignVariableDescriptionsProcessControlDesign rdf:type owl:NamedIndividual ,
                                                               :ProcessControlDesign ;
                                                      gsim-sum:hasValue-IA """Have all Represented Variables been designed?
- If no, go to back to the beginning of the Process Step and run again 
- If yes, go to the next Process Step 
Are there any duplications for Represented Variables descriptions as the result of the Process Step?
- If no, go to back to the beginning of the Process Step and run again 
- If yes, go to the next Process Step""" ;
                                                      rdfs:label "RTS - Design Variable Descriptions - Process Control Design"@en .


###  https://www.ksh.hu/survey/retail-trade-statistics#DesignVariableDescriptionsProcessDesign
kshrts:DesignVariableDescriptionsProcessDesign rdf:type owl:NamedIndividual ,
                                                        :ProcessDesign ;
                                               :classifiedAs <http://id.unece.org/models/gsbpm/2.2> ;
                                               :hasPD-PCD kshrts:DesignVariableDescriptionsProcessControlDesign ;
                                               :hasPD-PIS kshrts:DesignVariableDescriptionsProcessInputSpecification ;
                                               :hasPD-POS kshrts:DesignVariableDescriptionsProcessOutputSpecification ;
                                               :implementsPD-PM kshrts:DesignVariableDescriptionsProcessMethod ;
                                               :specifiesPD-PS kshrts:DesignVariableDescriptionsProcess ;
                                               rdfs:label "RTS - Design Variable Descriptions - Process Design"@en .


###  https://www.ksh.hu/survey/retail-trade-statistics#DesignVariableDescriptionsProcessInputSpecification
kshrts:DesignVariableDescriptionsProcessInputSpecification rdf:type owl:NamedIndividual ,
                                                                    :ProcessInputSpecification ;
                                                           :coreInputType "Business Cases containing proposed solutions and approved decisions regarding Concept to be measured" ;
                                                           :processSupportInputType """Standards, policies or guidelines to be followed on how to design Variables to be collected and write metadata description 
Repository or inventory of
- Variable, Unit Type (e.g., persons, households, enterprises), Measurement Type (e.g., currencies, capita)
- Value Domain, Measurement Unit
- Statistical Classification, Code List
that are agreed and approved in the Organisation to be used as reference
Represented Variables, Process Methods, Statistical Classification or any other referential metadata available from previous Statistical Program Cycles or similar Statistical Programs that can be used as reference""" ;
                                                           rdfs:label "RTS - Design Variable Descriptions - Process Input Specification"@en .


###  https://www.ksh.hu/survey/retail-trade-statistics#DesignVariableDescriptionsProcessMethod
kshrts:DesignVariableDescriptionsProcessMethod rdf:type owl:NamedIndividual ,
                                                        :ProcessMethod ;
                                               gsim-sum:hasValue-IA """- Review Business Case regarding Concepts and Variables
- Consult repository or inventory of Variables, Statistical Classifications, etc., relevant standards, guidelines and any available information from previous Statistical Program Cycles or similar Statistical Programs
- Design Represented Variables (Variables, Value Domains)
- Design Statistical Classifications* if needed
- Design Process Methods to be used for derivation and calculation of Represented Variables
- Prepare metadata descriptions of Represented Variables, Process Methods, etc.

* Version local to the current business process, the maintenance of Statistical Classification that is used across the Organization takes place as a separate business process.""" ;
                                               rdfs:label "RTS - Design Variable Descriptions - Process Method"@en .


###  https://www.ksh.hu/survey/retail-trade-statistics#DesignVariableDescriptionsProcessOutputSpecification
kshrts:DesignVariableDescriptionsProcessOutputSpecification rdf:type owl:NamedIndividual ,
                                                                     :ProcessOutputSpecification ;
                                                            :coreOutputType """Statistical Program Designs that containing 
- Represented Variables (Variables, Value Domains) to be used for collection and to be derived
- Process Methods specifying how to derive and calculate the Represented Variables 
- Statistical Classifications: description of the statistical classification (geospatial) structure and content.
- Referential Metadata Set describing any relevant information about Process Methods, Statistical Classification, etc.""" ;
                                                            :processMetricType """Quality measures regarding designing such as:
- Percentage of Represented Variables and classifications that have metadata descriptions
- Percentage of definitions and classifications associated to (key) Represented Variables and Populations that follow international and national standards
Quality measures of the Process Step such as:
- Time spent to complete the Process Step (derived from Process Execution Log)
- Cost spent to complete the Process Step""" ;
                                                            :processSupportInputType """Execution logs such as
- Time that Process Step started
- Time that Process Step ended""" ;
                                                            rdfs:label "RTS - Design Variable Descriptions - Process Output Specification"@en .


###  https://www.ksh.hu/survey/retail-trade-statistics#EstablishOutputObjectivesChangeDefinition
kshrts:EstablishOutputObjectivesChangeDefinition rdf:type owl:NamedIndividual ,
                                                          gsim-sum:ChangeDefinition ;
                                                 gsim-sum:hasValue-IA """*Produce the following products for retail trade statistics:
- Changes in the volume of sales in retail shops adjusted for calendar effects compared to the same period of the previous year
- Changes in the volume of sales in retail shops adjusted for seasonal and calendar effects compared to the monthly average of 2015
- Volume indices on sales of food, drinks and tobacco in retail shops adjusted for calendar effects, the same period of the previous year = 100.0
- Volume indices on sales of non-food products in retail shops adjusted for calendar effects, the same period of the previous year = 100.0
- Volume indices on sales of automotive fuel in retail shops adjusted for calendar effects, the same period of the previous year = 100.0
- Volume indices on total sales in retail shops adjusted for calendar effects, the same period of the previous year = 100.0;
- Volume indices on total retail sales without adjustment, the same period of the previous year = 100.0.

* NACE Rev.2 classification (Statistical Classification of Economic Activities in the European Community) is to be used for all the STS indicators
* All of the time series required by the STS regulation are to be transmitted to Eurostat. 
* The first estimates of the retail trade data is to be published not later than 35 days after the end of the reference month
* The TRAMO/SEATS method with JDemetra+ is to be used for seasonal adjustment of retail trade data, in accordance with the ESS guidelines on seasonal adjustment
* Aggregated data with less than 3 statistical units shall not be disseminated and secondary cell suppression shall be used to ensure the protection of all retail trade statistics tables.
* Retail trade statistics data shall be forwarded to Eurostat in SDMX format.""" ;
                                                 rdfs:label "RTS - Establish Output Objectives - Change Definition"@en .


###  https://www.ksh.hu/survey/retail-trade-statistics#EstablishOutputObjectivesCoreInput
kshrts:EstablishOutputObjectivesCoreInput rdf:type owl:NamedIndividual ,
                                                   :CoreInput ;
                                          :correspondsToPI-PIS kshrts:EstablishOutputObjectivesProcessInputSpecification ;
                                          :refersToCI-IA kshrts:ConsultAndConfirmNeedsChangeDefinition ;
                                          rdfs:label "RTS - Establish Output Objectives - Process Input (Core Input)"@en .


###  https://www.ksh.hu/survey/retail-trade-statistics#EstablishOutputObjectivesCoreOutput
kshrts:EstablishOutputObjectivesCoreOutput rdf:type owl:NamedIndividual ,
                                                    :CoreOutput ;
                                           :correspondsToPO-POS kshrts:EstablishOutputObjectivesProcessOutputSpecification ;
                                           :refersToCO-IA kshrts:EstablishOutputObjectivesChangeDefinition ;
                                           rdfs:label "RTS - Establish Output Objectives - Process Output (Core Output)"@en .


###  https://www.ksh.hu/survey/retail-trade-statistics#EstablishOutputObjectivesProcess
kshrts:EstablishOutputObjectivesProcess rdf:type owl:NamedIndividual ,
                                                 :ProcessStep ;
                                        :createsPS-PO kshrts:EstablishOutputObjectivesCoreOutput ;
                                        :hasPS-PI kshrts:EstablishOutputObjectivesCoreInput ,
                                                  kshrts:EstablishOutputObjectivesProcessSupportInput ;
                                        :hasEndTime-PS "2018-03-09T20:00:00"^^xsd:dateTime ;
                                        :hasStartTime-PS "2018-02-19T08:00:00"^^xsd:dateTime ;
                                        rdfs:label "RTS - Establish Output Objectives - Process"@en .


###  https://www.ksh.hu/survey/retail-trade-statistics#EstablishOutputObjectivesProcessControlDesign
kshrts:EstablishOutputObjectivesProcessControlDesign rdf:type owl:NamedIndividual ,
                                                              :ProcessControlDesign ;
                                                     gsim-sum:hasValue-IA """Have all relevant needs in Change Definitions been used to produce the output objectives in the form of Change Definitions?
- If no, go back to the beginning of the Process Step and run again 
- If yes, go to the Consult and Confirm Needs Process Step""" ;
                                                     rdfs:label "RTS - Establish Output Objectives - Process Control Design"@en .


###  https://www.ksh.hu/survey/retail-trade-statistics#EstablishOutputObjectivesProcessDesign
kshrts:EstablishOutputObjectivesProcessDesign rdf:type owl:NamedIndividual ,
                                                       :ProcessDesign ;
                                              :classifiedAs <http://id.unece.org/models/gsbpm/1.3> ;
                                              :hasPD-PCD kshrts:EstablishOutputObjectivesProcessControlDesign ;
                                              :hasPD-PIS kshrts:EstablishOutputObjectivesProcessInputSpecification ;
                                              :hasPD-POS kshrts:EstablishOutputObjectivesProcessOutputSpecification ;
                                              :implementsPD-PM kshrts:EstablishOutputObjectivesProcessMethod ;
                                              :specifiesPD-PS kshrts:EstablishOutputObjectivesProcess ;
                                              rdfs:label "RTS - Establish Output Objectives - Process Design"@en .


###  https://www.ksh.hu/survey/retail-trade-statistics#EstablishOutputObjectivesProcessInputSpecification
kshrts:EstablishOutputObjectivesProcessInputSpecification rdf:type owl:NamedIndividual ,
                                                                   :ProcessInputSpecification ;
                                                          :coreInputType "Change Definitions: confirmed, more detailed and structured version of the initial Statistical Needs" ;
                                                          :processSupportInputType "Legal frameworks and regulations that influence the content and quality of the outputs" ;
                                                          rdfs:label "RTS - Establish Output Objectives - Process Input Specification"@en .


###  https://www.ksh.hu/survey/retail-trade-statistics#EstablishOutputObjectivesProcessMethod
kshrts:EstablishOutputObjectivesProcessMethod rdf:type owl:NamedIndividual ,
                                                       :ProcessMethod ;
                                              gsim-sum:hasValue-IA """- Check all user needs in Change Definitions that are relevant for identification of output objectives
- Analyse the needs and identifies the output objectives while considering the legal frameworks and guidelines
- Agree on the quality measures for the output with users
- Update Change Definition with output objectives established""" ;
                                              rdfs:label "RTS - Establish Output Objectives - Process Method"@en .


###  https://www.ksh.hu/survey/retail-trade-statistics#EstablishOutputObjectivesProcessOutputSpecification
kshrts:EstablishOutputObjectivesProcessOutputSpecification rdf:type owl:NamedIndividual ,
                                                                    :ProcessOutputSpecification ;
                                                           :coreOutputType "Change Definitions describing the objectives of output (e.g., Products and services) to be produced, including their quality measures" ;
                                                           :processExecutionLogType """Execution logs such as
- Time that Process Step started
- Time that Process Step ended""" ;
                                                           :processMetricType """Quality measures (e.g., extent to which all needs are included in the process)
Quality measures of the Process Step such as:
- Time spent to complete the Process Step (derived from Process Execution Log)
- Cost spent to complete the Process Step""" ;
                                                           rdfs:label "RTS - Establish Output Objectives - Process Output Specification"@en .


###  https://www.ksh.hu/survey/retail-trade-statistics#EstablishOutputObjectivesProcessSupportInput
kshrts:EstablishOutputObjectivesProcessSupportInput rdf:type owl:NamedIndividual ,
                                                             :ProcessSupportInput ;
                                                    gsim-sum:hasValue-IA """Legal frameworks and regulations that influence the content and quality of the outputs
- Regulation (EC) No 223/2009 of the European Parliament of the Council on European statistics
- Act CLV of 2016 on Official Statistics regulating development, production and dissemination of official statistics at national level
- Council Regulation (EC) No 1165/98 of 19 May 1998 concerning short-term statistics
- Regulation (EC) No 1158/2005 of the European Parliament and of the Council of 6 July 2005 amending Council Regulation (EC) No 1165/98 concerning short-term statistics
- Methodology of short-term business statistics: guidelines on recommended breakdown, quality aspects and data and metadata structures
- Dissemination policy of the Hungarian Central Statistical Office""" ;
                                                    rdfs:label "RTS - Establish Output Objectives - Process Input (Process Support Input)"@en .


###  https://www.ksh.hu/survey/retail-trade-statistics#IdentifyConceptChangeDefinition
kshrts:IdentifyConceptChangeDefinition rdf:type owl:NamedIndividual ,
                                                gsim-sum:ChangeDefinition ;
                                       gsim-sum:hasValue-IA """Change Definitions describing Concepts reflecting user needs concerning what to be measured:
- Retail sales: the purchases of finished goods and services by consumers and businesses
- Nomenclature of type of shops: different types of shops, based on their specialisation
- Major commodity group: commodities distinguished by their main characteristics. Minimum user need is to distinguish food, non-food and fuel groups""" ;
                                       rdfs:label "RTS - Identify Concepts - Change Definition"@en .


###  https://www.ksh.hu/survey/retail-trade-statistics#IdentifyConceptCoreInput
kshrts:IdentifyConceptCoreInput rdf:type owl:NamedIndividual ,
                                         :CoreInput ;
                                :correspondsToPI-PIS kshrts:IdentifyConceptProcessInputSpecification ;
                                :refersToCI-IA kshrts:ConsultAndConfirmNeedsChangeDefinition ;
                                rdfs:label "RTS - Identify Concepts - Process Input (Core Input)"@en .


###  https://www.ksh.hu/survey/retail-trade-statistics#IdentifyConceptCoreOutput
kshrts:IdentifyConceptCoreOutput rdf:type owl:NamedIndividual ,
                                          :CoreOutput ;
                                 :correspondsToPO-POS kshrts:IdentifyConceptProcessOutputSpecification ;
                                 :refersToCO-IA kshrts:IdentifyConceptChangeDefinition ;
                                 rdfs:label "RTS - Identify Concepts - Process Output (Core Output)"@en .


###  https://www.ksh.hu/survey/retail-trade-statistics#IdentifyConceptProcess
kshrts:IdentifyConceptProcess rdf:type owl:NamedIndividual ,
                                       :ProcessStep ;
                              :createsPS-PO kshrts:IdentifyConceptCoreOutput ;
                              :hasPS-PI kshrts:IdentifyConceptCoreInput ,
                                        kshrts:IdentifyConceptProcessSupportInput ;
                              :hasEndTime-PS "2018-03-16T20:00:00"^^xsd:dateTime ;
                              :hasStartTime-PS "2018-02-19T08:00:00"^^xsd:dateTime ;
                              rdfs:label "RTS - Identify Concepts - Process"@en .


###  https://www.ksh.hu/survey/retail-trade-statistics#IdentifyConceptProcessControlDesign
kshrts:IdentifyConceptProcessControlDesign rdf:type owl:NamedIndividual ,
                                                    :ProcessControlDesign ;
                                           gsim-sum:hasValue-IA """Have all available needs in Change Definitions been used to identify the Concepts?
- If no, go back to the beginning of the Process Step and run again 
- • If yes, go to the next Process Step""" ;
                                           rdfs:label "RTS - Identify Concepts - Process Control Design"@en .


###  https://www.ksh.hu/survey/retail-trade-statistics#IdentifyConceptProcessDesign
kshrts:IdentifyConceptProcessDesign rdf:type owl:NamedIndividual ,
                                             :ProcessDesign ;
                                    :classifiedAs <http://id.unece.org/models/gsbpm/1.4> ;
                                    :hasPD-PCD kshrts:IdentifyConceptProcessControlDesign ;
                                    :hasPD-PIS kshrts:IdentifyConceptProcessInputSpecification ;
                                    :hasPD-POS kshrts:IdentifyConceptProcessOutputSpecification ;
                                    :implementsPD-PM kshrts:IdentifyConceptProcessMethod ;
                                    :specifiesPD-PS kshrts:IdentifyConceptProcess ;
                                    rdfs:label "RTS - Identify Concepts - Process Design"@en .


###  https://www.ksh.hu/survey/retail-trade-statistics#IdentifyConceptProcessInputSpecification
kshrts:IdentifyConceptProcessInputSpecification rdf:type owl:NamedIndividual ,
                                                         :ProcessInputSpecification ;
                                                :coreInputType "Change Definitions: confirmed, more detailed and structured version of the initial Statistical Needs" ;
                                                :processSupportInputType """- Policies or guidelines to be followed on how to identify and describe initial Concepts for the development, production and dissemination of statistics
- Repository or inventory of Concept that are agreed and approved in the Organisation to be used as a reference""" ;
                                                rdfs:label "RTS - Identify Concepts - Process Input Specification"@en .


###  https://www.ksh.hu/survey/retail-trade-statistics#IdentifyConceptProcessMethod
kshrts:IdentifyConceptProcessMethod rdf:type owl:NamedIndividual ,
                                             :ProcessMethod ;
                                    gsim-sum:hasValue-IA """- Check all user needs available in Change Definitions that are relevant for the identification of Concepts
- Consult repository or inventory of Concepts and relevant guidelines
- Identify all Concepts to be measured by statistics""" ;
                                    rdfs:label "RTS - Identify Concepts - Process Method"@en .


###  https://www.ksh.hu/survey/retail-trade-statistics#IdentifyConceptProcessOutputSpecification
kshrts:IdentifyConceptProcessOutputSpecification rdf:type owl:NamedIndividual ,
                                                          :ProcessOutputSpecification ;
                                                 :coreOutputType "Change Definitions describing Concepts reflecting user needs concerning what to be measured (e.g., target Population, Variable)" ;
                                                 :processExecutionLogType """Execution logs such as
- Time that Process Step started
- Time that Process Step ended""" ;
                                                 :processMetricType """Quality measures (e.g., extent to which needs are transformed into Concepts)
Quality measures of the Process Step such as:
- Time spent to complete the Process Step (derived from Process Execution Log)
- Cost spent to complete the Process Step""" ;
                                                 rdfs:label "RTS - Identify Concepts - Process Output Specification"@en .


###  https://www.ksh.hu/survey/retail-trade-statistics#IdentifyConceptProcessSupportInput
kshrts:IdentifyConceptProcessSupportInput rdf:type owl:NamedIndividual ,
                                                   :ProcessSupportInput ;
                                          gsim-sum:hasValue-IA "Dissemination policies" ;
                                          rdfs:label "RTS - Identify Concepts - Process Input (Process Support Input)"@en .


###  https://www.ksh.hu/survey/retail-trade-statistics#IdentifyNeedsAssessment
kshrts:IdentifyNeedsAssessment rdf:type owl:NamedIndividual ,
                                        gsim-sum:Assessment ;
                               gsim-sum:hasIssues-Ass """Have all Information Requests, Environment Changes and Assessments checked and analysed for the identification of Statistical Needs?
- If no, go back to the beginning of the Process Step and run again 
- If yes, go to the Consult and Confirm Needs Process Step""" ;
                               rdfs:label "RTS - Identify Needs - Assessment"@en .


###  https://www.ksh.hu/survey/retail-trade-statistics#IdentifyNeedsCoreInput
kshrts:IdentifyNeedsCoreInput rdf:type owl:NamedIndividual ,
                                       :CoreInput ;
                              :correspondsToPI-PIS kshrts:IdentifyNeedsProcessInputSpecification ;
                              :refersToCI-IA kshrts:IdentifyNeedsAssessment ,
                                             kshrts:IdentifyNeedsEnvironmentChanges ,
                                             kshrts:IdentifyNeedsInformationRequest ;
                              rdfs:label "RTS - Identify Needs - Process Input (Core Input)"@en .


###  https://www.ksh.hu/survey/retail-trade-statistics#IdentifyNeedsCoreOutput
kshrts:IdentifyNeedsCoreOutput rdf:type owl:NamedIndividual ,
                                        :CoreOutput ;
                               :correspondsToPO-POS kshrts:IdentifyNeedsProcessOutputSpecification ;
                               :refersToCO-IA kshrts:IdentifyNeedsStatisticalNeed ;
                               rdfs:label "RTS - Identify Needs - Process Output (Core Output)"@en .


###  https://www.ksh.hu/survey/retail-trade-statistics#IdentifyNeedsEnvironmentChanges
kshrts:IdentifyNeedsEnvironmentChanges rdf:type owl:NamedIndividual ,
                                                gsim-sum:EnvironmentChange ;
                                       gsim-sum:hasChangeOrigin-EC "NSI has access to retail trade data generated by electronic fiscal devices" ;
                                       rdfs:label "RTS - Identify Needs - Environment Changes"@en .


###  https://www.ksh.hu/survey/retail-trade-statistics#IdentifyNeedsInformationRequest
kshrts:IdentifyNeedsInformationRequest rdf:type owl:NamedIndividual ,
                                                gsim-sum:InformationRequest ;
                                       gsim-sum:hasInformationRequest-IR """- Need to provide information on retail sales on a regular basis
- Retail sales statistics need to be broken down by major commodity groups
- Users are also interested in sales of retails shops by type of shop
- Users need time series data and infra-annual data
- Eurostat needs volume indices on sales on a monthly basis, broken down by: food, non-food, fuel""" ;
                                       rdfs:label "RTS - Identify Needs - Information Request"@en .


###  https://www.ksh.hu/survey/retail-trade-statistics#IdentifyNeedsMethod
kshrts:IdentifyNeedsMethod rdf:type owl:NamedIndividual ,
                                    gsim-sum:ProcessMethod ;
                           gsim-sum:hasValue-IA """- Check all Information Requests, Environment Changes and Assessments received 
- Conduct an initial analysis of Information Requests, Environment Changes and Assessments, e.g., by comparing with practice amongst other statistical Organisations
- Produce the Statistical Needs""" ;
                           rdfs:label "RTS - Identify Needs - Process Method"@en .


###  https://www.ksh.hu/survey/retail-trade-statistics#IdentifyNeedsProcess
kshrts:IdentifyNeedsProcess rdf:type owl:NamedIndividual ,
                                     :ProcessStep ;
                            :createsPS-PO kshrts:IdentifyNeedsCoreOutput ;
                            :hasPS-PI kshrts:IdentifyNeedsCoreInput ;
                            :hasEndTime-PS "2018-01-19T20:00:00"^^xsd:dateTime ;
                            :hasStartTime-PS "2018-01-02T08:00:00"^^xsd:dateTime ;
                            rdfs:label "RTS - Identify Needs - Process"@en .


###  https://www.ksh.hu/survey/retail-trade-statistics#IdentifyNeedsProcessControlDesign
kshrts:IdentifyNeedsProcessControlDesign rdf:type owl:NamedIndividual ,
                                                  :ProcessControlDesign ;
                                         gsim-sum:hasValue-IA """Have all Information Requests, Environment Changes and Assessments checked and analysed for the identification of Statistical Needs?
- If no, go back to the beginning of the Process Step and run again 
- If yes, go to the Consult and Confirm Needs Process Step""" ;
                                         rdfs:label "RTS - Identify Needs - Process Control Design"@en .


###  https://www.ksh.hu/survey/retail-trade-statistics#IdentifyNeedsProcessDesign
kshrts:IdentifyNeedsProcessDesign rdf:type owl:NamedIndividual ,
                                           :ProcessDesign ;
                                  :classifiedAs <http://id.unece.org/models/gsbpm/1.1> ;
                                  :hasPD-PCD kshrts:IdentifyNeedsProcessControlDesign ;
                                  :hasPD-PIS kshrts:IdentifyNeedsProcessInputSpecification ;
                                  :hasPD-POS kshrts:IdentifyNeedsProcessOutputSpecification ;
                                  :implementsPD-PM kshrts:IdentifyNeedsMethod ;
                                  :specifiesPD-PS kshrts:IdentifyNeedsProcess ;
                                  rdfs:label "RTS - Identify Needs - Process Design"@en .


###  https://www.ksh.hu/survey/retail-trade-statistics#IdentifyNeedsProcessInputSpecification
kshrts:IdentifyNeedsProcessInputSpecification rdf:type owl:NamedIndividual ,
                                                       :ProcessInputSpecification ;
                                              :coreInputType """- Information Requests: needs for new statistical information 
- Environment Changes: change that originates from the operating environment of the statistical organisation
- Assessments: analysis of the quality and effectiveness of any activity undertaken by a statistical organisation and recommendations on how these can be improved (action plans and lessons learnt from previous iterations), e.g., from previous Statistical Program Cycles""" ;
                                              rdfs:label "RTS - Identify Needs - Process Input Specification"@en .


###  https://www.ksh.hu/survey/retail-trade-statistics#IdentifyNeedsProcessOutputSpecification
kshrts:IdentifyNeedsProcessOutputSpecification rdf:type owl:NamedIndividual ,
                                                        :ProcessOutputSpecification ;
                                               :coreOutputType "Statistical Needs: expression of all needs (but not necessarily well-defined) after initial investigation" ;
                                               :processExecutionLogType """Execution logs such as
- Time that Process Step started
- Time that Process Step ended
- Time that Information Requests were received""" ;
                                               :processMetricType """Quality measures (e.g., extent to which all needs from Information Requests, Environment Changes and Assessments are included in the identification process)
Quality measures of the Process Step such as:
- Time spent to complete the Process Step (derived from Process Execution Log)
- Cost spent to complete the Process Step""" ;
                                               rdfs:label "RTS - Identify Needs - Process Output Specification"@en .


###  https://www.ksh.hu/survey/retail-trade-statistics#IdentifyNeedsStatisticalNeed
kshrts:IdentifyNeedsStatisticalNeed rdf:type owl:NamedIndividual ,
                                             gsim-sum:StatisticalNeed ;
                                    gsim-sum:hasStatus-SN "Approved" ;
                                    gsim-sum:hasValue-IA """- Provide aggregated data on retail sales on a regular basis; broken down by major commodities and by type of shop
- Investigate how the new data source (electronic fiscal devices) can be used for the production of retail trade statistics
- Provide infra-annual and time series data
- For time series data, the comparability of data over time should be explained in more detail and in an easily understandable manner
- Prepare volume indices on sales on a monthly basis, broken down by: food, non-food, fuel and prepare the datasets to be sent to Eurostat regularly""" ;
                                    rdfs:label "RTS - Identify Needs - Statistical Need"@en .


###  https://www.ksh.hu/survey/retail-trade-statistics#PrepareAndSubmitBusinessCaseProcess
kshrts:PrepareAndSubmitBusinessCaseProcess rdf:type owl:NamedIndividual ,
                                                    :ProcessStep ;
                                           rdfs:label "RTS - Prepare And Submit Business Case - Process"@en .


###  https://www.ksh.hu/survey/retail-trade-statistics#PrepareAndSubmitBusinessCaseProcessControlDesign
kshrts:PrepareAndSubmitBusinessCaseProcessControlDesign rdf:type owl:NamedIndividual ,
                                                                 :ProcessControlDesign ;
                                                        gsim-sum:hasValue-IA """Does Business Case meet requirements and follow guidelines of approving body? 
•   If no, go back to the beginning of Process Step and run again
•   If yes, submit Business Case""" ;
                                                        rdfs:label "RTS - Prepare And Submit Business Case - Process Control Design"@en .


###  https://www.ksh.hu/survey/retail-trade-statistics#PrepareAndSubmitBusinessCaseProcessDesign
kshrts:PrepareAndSubmitBusinessCaseProcessDesign rdf:type owl:NamedIndividual ,
                                                          :ProcessDesign ;
                                                 :classifiedAs <http://id.unece.org/models/gsbpm/1.6> ;
                                                 :hasPD-PCD kshrts:PrepareAndSubmitBusinessCaseProcessControlDesign ;
                                                 :hasPD-PIS kshrts:PrepareAndSubmitBusinessCaseProcessInputSpecification ;
                                                 :hasPD-POS kshrts:PrepareAndSubmitBusinessCaseProcessOutputSpecification ;
                                                 :implementsPD-PM kshrts:PrepareAndSubmitBusinessCaseProcessMethod ;
                                                 :specifiesPD-PS kshrts:PrepareAndSubmitBusinessCaseProcess ;
                                                 rdfs:label "RTS - Prepare And Submit Business Case - Process Design"@en .


###  https://www.ksh.hu/survey/retail-trade-statistics#PrepareAndSubmitBusinessCaseProcessInputSpecification
kshrts:PrepareAndSubmitBusinessCaseProcessInputSpecification rdf:type owl:NamedIndividual ,
                                                                      :ProcessInputSpecification ;
                                                             :coreInputType """Change Definitions containing information about
- Confirmed, more detailed and structured version of user needs 
- Objectives of output (e.g., Products and services) to be produced, including their quality measures
- Specification of Concepts reflecting user needs concerning what to be measured, collected and produced

Assessments on
- Information Resources (data availability)
- Other resources (e.g., IT, human resources) within the Organisation required for data acquisition / collection as well as for meeting user needs of the outputs""" ;
                                                             :processSupportInputType "Policies or guidelines of approving body on how to prepare Business Case" ;
                                                             rdfs:label "RTS - Prepare And Submit Business Case - Process Input Specification"@en .


###  https://www.ksh.hu/survey/retail-trade-statistics#PrepareAndSubmitBusinessCaseProcessMethod
kshrts:PrepareAndSubmitBusinessCaseProcessMethod rdf:type owl:NamedIndividual ,
                                                          :ProcessMethod ;
                                                 gsim-sum:hasValue-IA """- Check whether exiting Information Resources in the Organisation or alternative Information Resources outside the Organisation could meet user needs or be used to measure Concepts or Variables as specified in Change Definition, with consideration with any restriction in Provision Agreements
- Assess the division of responsibilities between different Agents and Data Providers within or outside the Organisation and any ICT resources needed to acquire or transfer the data""" ;
                                                 rdfs:label "RTS - Prepare And Submit Business Case - Process Method"@en .


###  https://www.ksh.hu/survey/retail-trade-statistics#PrepareAndSubmitBusinessCaseProcessOutputSpecification
kshrts:PrepareAndSubmitBusinessCaseProcessOutputSpecification rdf:type owl:NamedIndividual ,
                                                                       :ProcessOutputSpecification ;
                                                              :coreOutputType """Business Cases containing information on 
- Proposed changes and solutions in consideration with user needs and proposals in Change Definitions
- Assessments of required resources (e.g., budget, human resources), cost-benefit of implementing the changes as well as risks""" ;
                                                              :processExecutionLogType """Execution logs such as
- Time that Process Step started
- Time that Process Step ended""" ;
                                                              :processMetricType """Quality measures (e.g., to what extent does Business Case reflect the findings, recommendations and proposals from previous Process Steps)


Quality measures of the Process Step such as:
- Time spent to complete the Process Step (derived from Process Execution Log)
- Cost spent to complete the Process Step""" ;
                                                              rdfs:label "RTS - Prepare And Submit Business Case - Process Output Specification"@en .


###  https://www.ksh.hu/survey/retail-trade-statistics#RetailTradeStatistics
kshrts:RetailTradeStatistics rdf:type owl:NamedIndividual ,
                                      :StatisticalProgram ;
                             :hasSP-SPC kshrts:RetailTradeStatisticsProgramCycle ;
                             gsim-sum:hasDateInitiated-SP "2020-01-15T00:00:00+07:00"^^xsd:dateTime ;
                             gsim-sum:hasDescription-IA "Statistical activities that present data related to retail trade such as the number of retail traders and trade value per group of goods presented every quarter." ;
                             gsim-sum:hasName-IA "Retail Trade Statistics" ;
                             gsim-sum:hasSourceOfFunding-SP "Government budget" ;
                             gsim-sum:hasStatus-SP "New Proposal" ;
                             rdfs:label "Retail Trade Statistics (RTS) Program"@en .


###  https://www.ksh.hu/survey/retail-trade-statistics#RetailTradeStatisticsBusinessProcess
kshrts:RetailTradeStatisticsBusinessProcess rdf:type owl:NamedIndividual ,
                                                     :BusinessProcess ;
                                            :hasBP-PS kshrts:CheckDataAvailabilityProcess ,
                                                      kshrts:ConsultAndConfirmNeeds ,
                                                      kshrts:DesignCollectionProcess ,
                                                      kshrts:DesignFrameAndSampleProcess ,
                                                      kshrts:DesignOutputProcess ,
                                                      kshrts:DesignVariableDescriptionsProcess ,
                                                      kshrts:EstablishOutputObjectivesProcess ,
                                                      kshrts:IdentifyConceptProcess ,
                                                      kshrts:IdentifyNeedsProcess ,
                                                      kshrts:PrepareAndSubmitBusinessCaseProcess ;
                                            gsim-sum:hasName-IA "Retail Trade Statistics Business Process" ;
                                            rdfs:label "Retail Trade Statistics (RTS) Business Process"@en .


###  https://www.ksh.hu/survey/retail-trade-statistics#RetailTradeStatisticsProgramCycle
kshrts:RetailTradeStatisticsProgramCycle rdf:type owl:NamedIndividual ,
                                                  :StatisticalProgramCycle ;
                                         :includesSPC-BP kshrts:RetailTradeStatisticsBusinessProcess ;
                                         gsim-sum:hasDescription-IA "Retail Trade activities presented every quarter." ;
                                         gsim-sum:hasName-IA "Retail Trade Statistics Cycle" ;
                                         rdfs:label "Retail Trade Statistics (RTS) Program Cycle"@en .


#################################################################
#    Annotations
#################################################################

cspa:label rdfs:label "Label" .


###  Generated by the OWL API (version 4.5.26.2023-07-17T20:34:13Z) https://github.com/owlcs/owlapi
